QCP_examples/humaneval/spec_logic_rewrite_c_files/C_140_goal.v
@@ -1,0 +1,2208 @@
+Require Import Coq.ZArith.ZArith.
+Require Import Coq.Bool.Bool.
+Require Import Coq.Strings.String.
+Require Import Coq.Strings.Ascii.
+Require Import Coq.Lists.List.
+Require Import Coq.Classes.RelationClasses.
+Require Import Coq.Classes.Morphisms.
+Require Import Coq.micromega.Psatz.
+Require Import Coq.Sorting.Permutation.
+From AUXLib Require Import int_auto Axioms Feq Idents ListLib VMap.
+Require Import SetsClass.SetsClass. Import SetsNotation.
+From SimpleC.SL Require Import Mem SeparationLogic.
+Require Import Logic.LogicGenerator.demo932.Interface.
+Local Open Scope Z_scope.
+Local Open Scope sets.
+Local Open Scope string_scope.
+Local Open Scope list.
+Import naive_C_Rules.
+Require Import SimpleC.StdLib.string_lib.
+Require Import coins_140.
+Local Open Scope sac.
+From SimpleC.EE.QCP_demos_LLM Require Import char_array_strategy_goal.
+From SimpleC.EE.QCP_demos_LLM Require Import char_array_strategy_proof.
+From SimpleC.StdLib Require Import string_strategy_goal.
+From SimpleC.StdLib Require Import string_strategy_proof.
+
+(*----- Function fix_spaces -----*)
+
+Definition fix_spaces_safety_wit_1 := 
+forall (text_pre: Z) (input: (@list Z)) (retval: Z) (PreH1 : (retval = (string_length (input)))) (PreH2 : (0 <= ((string_length (input)) + 1 ))) (PreH3 : (valid_string input )) (PreH4 : (problem_140_pre_z input )) (PreH5 : (ascii_range_z input )) (PreH6 : ((string_length (input)) < INT_MAX)) ,
+  ((( &( "out" ) )) # Ptr  |->_)
+  **  (store_string text_pre input )
+  **  ((( &( "n" ) )) # Int  |-> retval)
+  **  ((( &( "text" ) )) # Ptr  |-> text_pre)
+|--
+  “ ((retval + 1 ) <= INT_MAX) ” 
+  &&  “ ((INT_MIN) <= (retval + 1 )) ”
+.
+
+Definition fix_spaces_safety_wit_2 := 
+forall (text_pre: Z) (input: (@list Z)) (retval: Z) (PreH1 : (retval = (string_length (input)))) (PreH2 : (0 <= ((string_length (input)) + 1 ))) (PreH3 : (valid_string input )) (PreH4 : (problem_140_pre_z input )) (PreH5 : (ascii_range_z input )) (PreH6 : ((string_length (input)) < INT_MAX)) ,
+  ((( &( "out" ) )) # Ptr  |->_)
+  **  (store_string text_pre input )
+  **  ((( &( "n" ) )) # Int  |-> retval)
+  **  ((( &( "text" ) )) # Ptr  |-> text_pre)
+|--
+  “ (1 <= INT_MAX) ” 
+  &&  “ ((INT_MIN) <= 1) ”
+.
+
+Definition fix_spaces_safety_wit_3 := 
+forall (text_pre: Z) (input: (@list Z)) (retval: Z) (retval_2: Z) (PreH1 : (retval_2 <> 0)) (PreH2 : (retval = (string_length (input)))) (PreH3 : (0 <= ((string_length (input)) + 1 ))) (PreH4 : (valid_string input )) (PreH5 : (problem_140_pre_z input )) (PreH6 : (ascii_range_z input )) (PreH7 : ((string_length (input)) < INT_MAX)) ,
+  (CharArray.undef_full retval_2 (retval + 1 ) )
+  **  (CharArray.full text_pre ((string_length (input)) + 1 ) (c_string (input)) )
+  **  ((( &( "out" ) )) # Ptr  |-> retval_2)
+  **  ((( &( "n" ) )) # Int  |-> retval)
+  **  ((( &( "text" ) )) # Ptr  |-> text_pre)
+|--
+  “ (0 <= INT_MAX) ” 
+  &&  “ ((INT_MIN) <= 0) ”
+.
+
+Definition fix_spaces_safety_wit_4 := 
+forall (text_pre: Z) (input: (@list Z)) (retval: Z) (retval_2: Z) (PreH1 : (retval_2 = 0)) (PreH2 : (retval_2 <> 0)) (PreH3 : (retval = (string_length (input)))) (PreH4 : (0 <= ((string_length (input)) + 1 ))) (PreH5 : (valid_string input )) (PreH6 : (problem_140_pre_z input )) (PreH7 : (ascii_range_z input )) (PreH8 : ((string_length (input)) < INT_MAX)) ,
+  (CharArray.undef_full retval_2 (retval + 1 ) )
+  **  (CharArray.full text_pre ((string_length (input)) + 1 ) (c_string (input)) )
+  **  ((( &( "out" ) )) # Ptr  |-> retval_2)
+  **  ((( &( "n" ) )) # Int  |-> retval)
+  **  ((( &( "text" ) )) # Ptr  |-> text_pre)
+|--
+  “ False ”
+.
+
+Definition fix_spaces_safety_wit_5 := 
+forall (text_pre: Z) (input: (@list Z)) (retval: Z) (retval_2: Z) (PreH1 : (retval_2 <> 0)) (PreH2 : (retval_2 <> 0)) (PreH3 : (retval = (string_length (input)))) (PreH4 : (0 <= ((string_length (input)) + 1 ))) (PreH5 : (valid_string input )) (PreH6 : (problem_140_pre_z input )) (PreH7 : (ascii_range_z input )) (PreH8 : ((string_length (input)) < INT_MAX)) ,
+  ((( &( "k" ) )) # Int  |->_)
+  **  (CharArray.undef_full retval_2 (retval + 1 ) )
+  **  (CharArray.full text_pre ((string_length (input)) + 1 ) (c_string (input)) )
+  **  ((( &( "out" ) )) # Ptr  |-> retval_2)
+  **  ((( &( "n" ) )) # Int  |-> retval)
+  **  ((( &( "text" ) )) # Ptr  |-> text_pre)
+|--
+  “ (0 <= INT_MAX) ” 
+  &&  “ ((INT_MIN) <= 0) ”
+.
+
+Definition fix_spaces_safety_wit_6 := 
+forall (text_pre: Z) (input: (@list Z)) (retval: Z) (retval_2: Z) (PreH1 : (retval_2 <> 0)) (PreH2 : (retval_2 <> 0)) (PreH3 : (retval = (string_length (input)))) (PreH4 : (0 <= ((string_length (input)) + 1 ))) (PreH5 : (valid_string input )) (PreH6 : (problem_140_pre_z input )) (PreH7 : (ascii_range_z input )) (PreH8 : ((string_length (input)) < INT_MAX)) ,
+  ((( &( "spacelen" ) )) # Int  |->_)
+  **  ((( &( "k" ) )) # Int  |-> 0)
+  **  (CharArray.undef_full retval_2 (retval + 1 ) )
+  **  (CharArray.full text_pre ((string_length (input)) + 1 ) (c_string (input)) )
+  **  ((( &( "out" ) )) # Ptr  |-> retval_2)
+  **  ((( &( "n" ) )) # Int  |-> retval)
+  **  ((( &( "text" ) )) # Ptr  |-> text_pre)
+|--
+  “ (0 <= INT_MAX) ” 
+  &&  “ ((INT_MIN) <= 0) ”
+.
+
+Definition fix_spaces_safety_wit_7 := 
+forall (text_pre: Z) (input: (@list Z)) (retval: Z) (retval_2: Z) (PreH1 : (retval_2 <> 0)) (PreH2 : (retval_2 <> 0)) (PreH3 : (retval = (string_length (input)))) (PreH4 : (0 <= ((string_length (input)) + 1 ))) (PreH5 : (valid_string input )) (PreH6 : (problem_140_pre_z input )) (PreH7 : (ascii_range_z input )) (PreH8 : ((string_length (input)) < INT_MAX)) ,
+  ((( &( "i" ) )) # Int  |->_)
+  **  ((( &( "spacelen" ) )) # Int  |-> 0)
+  **  ((( &( "k" ) )) # Int  |-> 0)
+  **  (CharArray.undef_full retval_2 (retval + 1 ) )
+  **  (CharArray.full text_pre ((string_length (input)) + 1 ) (c_string (input)) )
+  **  ((( &( "out" ) )) # Ptr  |-> retval_2)
+  **  ((( &( "n" ) )) # Int  |-> retval)
+  **  ((( &( "text" ) )) # Ptr  |-> text_pre)
+|--
+  “ (0 <= INT_MAX) ” 
+  &&  “ ((INT_MIN) <= 0) ”
+.
+
+Definition fix_spaces_safety_wit_8 := 
+forall (text_pre: Z) (input: (@list Z)) (out: Z) (output: (@list Z)) (spacelen: Z) (k: Z) (i: Z) (n: Z) (PreH1 : (i < n)) (PreH2 : (n = (string_length (input)))) (PreH3 : (0 <= i)) (PreH4 : (i <= n)) (PreH5 : (0 <= k)) (PreH6 : (0 <= spacelen)) (PreH7 : ((k + spacelen ) <= i)) (PreH8 : (k = (Zlength (output)))) (PreH9 : (fix_spaces_state_z_140 input output i spacelen )) (PreH10 : (valid_string input )) (PreH11 : (problem_140_pre_z input )) (PreH12 : (ascii_range_z input )) (PreH13 : ((string_length (input)) < INT_MAX)) ,
+  ((( &( "text" ) )) # Ptr  |-> text_pre)
+  **  ((( &( "n" ) )) # Int  |-> n)
+  **  ((( &( "i" ) )) # Int  |-> i)
+  **  ((( &( "k" ) )) # Int  |-> k)
+  **  ((( &( "spacelen" ) )) # Int  |-> spacelen)
+  **  (store_string text_pre input )
+  **  ((( &( "out" ) )) # Ptr  |-> out)
+  **  (CharArray.full out k output )
+  **  (CharArray.undef_seg out k (n + 1 ) )
+|--
+  “ (32 <= INT_MAX) ” 
+  &&  “ ((INT_MIN) <= 32) ”
+.
+
+Definition fix_spaces_safety_wit_9 := 
+forall (text_pre: Z) (input: (@list Z)) (out: Z) (output: (@list Z)) (spacelen: Z) (k: Z) (i: Z) (n: Z) (PreH1 : ((Znth i (c_string (input)) 0) = 32)) (PreH2 : (i < n)) (PreH3 : (n = (string_length (input)))) (PreH4 : (0 <= i)) (PreH5 : (i <= n)) (PreH6 : (0 <= k)) (PreH7 : (0 <= spacelen)) (PreH8 : ((k + spacelen ) <= i)) (PreH9 : (k = (Zlength (output)))) (PreH10 : (fix_spaces_state_z_140 input output i spacelen )) (PreH11 : (valid_string input )) (PreH12 : (problem_140_pre_z input )) (PreH13 : (ascii_range_z input )) (PreH14 : ((string_length (input)) < INT_MAX)) ,
+  ((( &( "text" ) )) # Ptr  |-> text_pre)
+  **  ((( &( "n" ) )) # Int  |-> n)
+  **  ((( &( "i" ) )) # Int  |-> i)
+  **  ((( &( "k" ) )) # Int  |-> k)
+  **  ((( &( "spacelen" ) )) # Int  |-> spacelen)
+  **  (store_string text_pre input )
+  **  ((( &( "out" ) )) # Ptr  |-> out)
+  **  (CharArray.full out k output )
+  **  (CharArray.undef_seg out k (n + 1 ) )
+|--
+  “ ((spacelen + 1 ) <= INT_MAX) ” 
+  &&  “ ((INT_MIN) <= (spacelen + 1 )) ”
+.
+
+Definition fix_spaces_safety_wit_10 := 
+forall (text_pre: Z) (input: (@list Z)) (out: Z) (output: (@list Z)) (spacelen: Z) (k: Z) (i: Z) (n: Z) (PreH1 : ((Znth i (c_string (input)) 0) = 32)) (PreH2 : (i < n)) (PreH3 : (n = (string_length (input)))) (PreH4 : (0 <= i)) (PreH5 : (i <= n)) (PreH6 : (0 <= k)) (PreH7 : (0 <= spacelen)) (PreH8 : ((k + spacelen ) <= i)) (PreH9 : (k = (Zlength (output)))) (PreH10 : (fix_spaces_state_z_140 input output i spacelen )) (PreH11 : (valid_string input )) (PreH12 : (problem_140_pre_z input )) (PreH13 : (ascii_range_z input )) (PreH14 : ((string_length (input)) < INT_MAX)) ,
+  ((( &( "text" ) )) # Ptr  |-> text_pre)
+  **  ((( &( "n" ) )) # Int  |-> n)
+  **  ((( &( "i" ) )) # Int  |-> i)
+  **  ((( &( "k" ) )) # Int  |-> k)
+  **  ((( &( "spacelen" ) )) # Int  |-> spacelen)
+  **  (store_string text_pre input )
+  **  ((( &( "out" ) )) # Ptr  |-> out)
+  **  (CharArray.full out k output )
+  **  (CharArray.undef_seg out k (n + 1 ) )
+|--
+  “ (1 <= INT_MAX) ” 
+  &&  “ ((INT_MIN) <= 1) ”
+.
+
+Definition fix_spaces_safety_wit_11 := 
+forall (text_pre: Z) (input: (@list Z)) (out: Z) (output: (@list Z)) (spacelen: Z) (k: Z) (i: Z) (n: Z) (PreH1 : ((Znth i (c_string (input)) 0) <> 32)) (PreH2 : (i < n)) (PreH3 : (n = (string_length (input)))) (PreH4 : (0 <= i)) (PreH5 : (i <= n)) (PreH6 : (0 <= k)) (PreH7 : (0 <= spacelen)) (PreH8 : ((k + spacelen ) <= i)) (PreH9 : (k = (Zlength (output)))) (PreH10 : (fix_spaces_state_z_140 input output i spacelen )) (PreH11 : (valid_string input )) (PreH12 : (problem_140_pre_z input )) (PreH13 : (ascii_range_z input )) (PreH14 : ((string_length (input)) < INT_MAX)) ,
+  ((( &( "text" ) )) # Ptr  |-> text_pre)
+  **  ((( &( "n" ) )) # Int  |-> n)
+  **  ((( &( "i" ) )) # Int  |-> i)
+  **  ((( &( "k" ) )) # Int  |-> k)
+  **  ((( &( "spacelen" ) )) # Int  |-> spacelen)
+  **  (store_string text_pre input )
+  **  ((( &( "out" ) )) # Ptr  |-> out)
+  **  (CharArray.full out k output )
+  **  (CharArray.undef_seg out k (n + 1 ) )
+|--
+  “ (1 <= INT_MAX) ” 
+  &&  “ ((INT_MIN) <= 1) ”
+.
+
+Definition fix_spaces_safety_wit_12 := 
+forall (text_pre: Z) (input: (@list Z)) (out: Z) (output: (@list Z)) (spacelen: Z) (k: Z) (i: Z) (n: Z) (PreH1 : (spacelen = 1)) (PreH2 : ((Znth i (c_string (input)) 0) <> 32)) (PreH3 : (i < n)) (PreH4 : (n = (string_length (input)))) (PreH5 : (0 <= i)) (PreH6 : (i <= n)) (PreH7 : (0 <= k)) (PreH8 : (0 <= spacelen)) (PreH9 : ((k + spacelen ) <= i)) (PreH10 : (k = (Zlength (output)))) (PreH11 : (fix_spaces_state_z_140 input output i spacelen )) (PreH12 : (valid_string input )) (PreH13 : (problem_140_pre_z input )) (PreH14 : (ascii_range_z input )) (PreH15 : ((string_length (input)) < INT_MAX)) ,
+  ((( &( "text" ) )) # Ptr  |-> text_pre)
+  **  ((( &( "n" ) )) # Int  |-> n)
+  **  ((( &( "i" ) )) # Int  |-> i)
+  **  ((( &( "k" ) )) # Int  |-> k)
+  **  ((( &( "spacelen" ) )) # Int  |-> spacelen)
+  **  (store_string text_pre input )
+  **  ((( &( "out" ) )) # Ptr  |-> out)
+  **  (CharArray.full out k output )
+  **  (CharArray.undef_seg out k (n + 1 ) )
+|--
+  “ (95 <= INT_MAX) ” 
+  &&  “ ((INT_MIN) <= 95) ”
+.
+
+Definition fix_spaces_safety_wit_13 := 
+forall (text_pre: Z) (input: (@list Z)) (out: Z) (output: (@list Z)) (spacelen: Z) (k: Z) (i: Z) (n: Z) (PreH1 : (0 <= ((string_length (input)) + 1 ))) (PreH2 : (spacelen = 1)) (PreH3 : ((Znth i (c_string (input)) 0) <> 32)) (PreH4 : (i < n)) (PreH5 : (n = (string_length (input)))) (PreH6 : (0 <= i)) (PreH7 : (i <= n)) (PreH8 : (0 <= k)) (PreH9 : (0 <= spacelen)) (PreH10 : ((k + spacelen ) <= i)) (PreH11 : (k = (Zlength (output)))) (PreH12 : (fix_spaces_state_z_140 input output i spacelen )) (PreH13 : (valid_string input )) (PreH14 : (problem_140_pre_z input )) (PreH15 : (ascii_range_z input )) (PreH16 : ((string_length (input)) < INT_MAX)) ,
+  (CharArray.full out (k + 1 ) (app (output) ((cons (95) ((@nil Z))))) )
+  **  (CharArray.undef_seg out (k + 1 ) (n + 1 ) )
+  **  (CharArray.full text_pre ((string_length (input)) + 1 ) (c_string (input)) )
+  **  ((( &( "text" ) )) # Ptr  |-> text_pre)
+  **  ((( &( "n" ) )) # Int  |-> n)
+  **  ((( &( "i" ) )) # Int  |-> i)
+  **  ((( &( "k" ) )) # Int  |-> k)
+  **  ((( &( "spacelen" ) )) # Int  |-> spacelen)
+  **  ((( &( "out" ) )) # Ptr  |-> out)
+|--
+  “ ((k + 1 ) <= INT_MAX) ” 
+  &&  “ ((INT_MIN) <= (k + 1 )) ”
+.
+
+Definition fix_spaces_safety_wit_14 := 
+forall (text_pre: Z) (input: (@list Z)) (out: Z) (output: (@list Z)) (spacelen: Z) (k: Z) (i: Z) (n: Z) (PreH1 : (0 <= ((string_length (input)) + 1 ))) (PreH2 : (spacelen = 1)) (PreH3 : ((Znth i (c_string (input)) 0) <> 32)) (PreH4 : (i < n)) (PreH5 : (n = (string_length (input)))) (PreH6 : (0 <= i)) (PreH7 : (i <= n)) (PreH8 : (0 <= k)) (PreH9 : (0 <= spacelen)) (PreH10 : ((k + spacelen ) <= i)) (PreH11 : (k = (Zlength (output)))) (PreH12 : (fix_spaces_state_z_140 input output i spacelen )) (PreH13 : (valid_string input )) (PreH14 : (problem_140_pre_z input )) (PreH15 : (ascii_range_z input )) (PreH16 : ((string_length (input)) < INT_MAX)) ,
+  (CharArray.full out (k + 1 ) (app (output) ((cons (95) ((@nil Z))))) )
+  **  (CharArray.undef_seg out (k + 1 ) (n + 1 ) )
+  **  (CharArray.full text_pre ((string_length (input)) + 1 ) (c_string (input)) )
+  **  ((( &( "text" ) )) # Ptr  |-> text_pre)
+  **  ((( &( "n" ) )) # Int  |-> n)
+  **  ((( &( "i" ) )) # Int  |-> i)
+  **  ((( &( "k" ) )) # Int  |-> k)
+  **  ((( &( "spacelen" ) )) # Int  |-> spacelen)
+  **  ((( &( "out" ) )) # Ptr  |-> out)
+|--
+  “ (1 <= INT_MAX) ” 
+  &&  “ ((INT_MIN) <= 1) ”
+.
+
+Definition fix_spaces_safety_wit_15 := 
+forall (text_pre: Z) (input: (@list Z)) (out: Z) (output: (@list Z)) (spacelen: Z) (k: Z) (i: Z) (n: Z) (PreH1 : (0 <= ((string_length (input)) + 1 ))) (PreH2 : (spacelen = 1)) (PreH3 : ((Znth i (c_string (input)) 0) <> 32)) (PreH4 : (i < n)) (PreH5 : (n = (string_length (input)))) (PreH6 : (0 <= i)) (PreH7 : (i <= n)) (PreH8 : (0 <= k)) (PreH9 : (0 <= spacelen)) (PreH10 : ((k + spacelen ) <= i)) (PreH11 : (k = (Zlength (output)))) (PreH12 : (fix_spaces_state_z_140 input output i spacelen )) (PreH13 : (valid_string input )) (PreH14 : (problem_140_pre_z input )) (PreH15 : (ascii_range_z input )) (PreH16 : ((string_length (input)) < INT_MAX)) ,
+  (CharArray.full out (k + 1 ) (app (output) ((cons (95) ((@nil Z))))) )
+  **  (CharArray.undef_seg out (k + 1 ) (n + 1 ) )
+  **  (CharArray.full text_pre ((string_length (input)) + 1 ) (c_string (input)) )
+  **  ((( &( "text" ) )) # Ptr  |-> text_pre)
+  **  ((( &( "n" ) )) # Int  |-> n)
+  **  ((( &( "i" ) )) # Int  |-> i)
+  **  ((( &( "k" ) )) # Int  |-> (k + 1 ))
+  **  ((( &( "spacelen" ) )) # Int  |-> spacelen)
+  **  ((( &( "out" ) )) # Ptr  |-> out)
+|--
+  “ (2 <= INT_MAX) ” 
+  &&  “ ((INT_MIN) <= 2) ”
+.
+
+Definition fix_spaces_safety_wit_16 := 
+forall (text_pre: Z) (input: (@list Z)) (out: Z) (output: (@list Z)) (spacelen: Z) (k: Z) (i: Z) (n: Z) (PreH1 : (spacelen <> 1)) (PreH2 : ((Znth i (c_string (input)) 0) <> 32)) (PreH3 : (i < n)) (PreH4 : (n = (string_length (input)))) (PreH5 : (0 <= i)) (PreH6 : (i <= n)) (PreH7 : (0 <= k)) (PreH8 : (0 <= spacelen)) (PreH9 : ((k + spacelen ) <= i)) (PreH10 : (k = (Zlength (output)))) (PreH11 : (fix_spaces_state_z_140 input output i spacelen )) (PreH12 : (valid_string input )) (PreH13 : (problem_140_pre_z input )) (PreH14 : (ascii_range_z input )) (PreH15 : ((string_length (input)) < INT_MAX)) ,
+  ((( &( "text" ) )) # Ptr  |-> text_pre)
+  **  ((( &( "n" ) )) # Int  |-> n)
+  **  ((( &( "i" ) )) # Int  |-> i)
+  **  ((( &( "k" ) )) # Int  |-> k)
+  **  ((( &( "spacelen" ) )) # Int  |-> spacelen)
+  **  (store_string text_pre input )
+  **  ((( &( "out" ) )) # Ptr  |-> out)
+  **  (CharArray.full out k output )
+  **  (CharArray.undef_seg out k (n + 1 ) )
+|--
+  “ (2 <= INT_MAX) ” 
+  &&  “ ((INT_MIN) <= 2) ”
+.
+
+Definition fix_spaces_safety_wit_17 := 
+forall (text_pre: Z) (input: (@list Z)) (out: Z) (output: (@list Z)) (spacelen: Z) (k: Z) (i: Z) (n: Z) (PreH1 : (spacelen = 2)) (PreH2 : (0 <= ((string_length (input)) + 1 ))) (PreH3 : (spacelen = 1)) (PreH4 : ((Znth i (c_string (input)) 0) <> 32)) (PreH5 : (i < n)) (PreH6 : (n = (string_length (input)))) (PreH7 : (0 <= i)) (PreH8 : (i <= n)) (PreH9 : (0 <= k)) (PreH10 : (0 <= spacelen)) (PreH11 : ((k + spacelen ) <= i)) (PreH12 : (k = (Zlength (output)))) (PreH13 : (fix_spaces_state_z_140 input output i spacelen )) (PreH14 : (valid_string input )) (PreH15 : (problem_140_pre_z input )) (PreH16 : (ascii_range_z input )) (PreH17 : ((string_length (input)) < INT_MAX)) ,
+  (CharArray.full out (k + 1 ) (app (output) ((cons (95) ((@nil Z))))) )
+  **  (CharArray.undef_seg out (k + 1 ) (n + 1 ) )
+  **  (CharArray.full text_pre ((string_length (input)) + 1 ) (c_string (input)) )
+  **  ((( &( "text" ) )) # Ptr  |-> text_pre)
+  **  ((( &( "n" ) )) # Int  |-> n)
+  **  ((( &( "i" ) )) # Int  |-> i)
+  **  ((( &( "k" ) )) # Int  |-> (k + 1 ))
+  **  ((( &( "spacelen" ) )) # Int  |-> spacelen)
+  **  ((( &( "out" ) )) # Ptr  |-> out)
+|--
+  “ False ”
+.
+
+Definition fix_spaces_safety_wit_18 := 
+forall (text_pre: Z) (input: (@list Z)) (out: Z) (output: (@list Z)) (spacelen: Z) (k: Z) (i: Z) (n: Z) (PreH1 : (spacelen = 2)) (PreH2 : (spacelen <> 1)) (PreH3 : ((Znth i (c_string (input)) 0) <> 32)) (PreH4 : (i < n)) (PreH5 : (n = (string_length (input)))) (PreH6 : (0 <= i)) (PreH7 : (i <= n)) (PreH8 : (0 <= k)) (PreH9 : (0 <= spacelen)) (PreH10 : ((k + spacelen ) <= i)) (PreH11 : (k = (Zlength (output)))) (PreH12 : (fix_spaces_state_z_140 input output i spacelen )) (PreH13 : (valid_string input )) (PreH14 : (problem_140_pre_z input )) (PreH15 : (ascii_range_z input )) (PreH16 : ((string_length (input)) < INT_MAX)) ,
+  ((( &( "text" ) )) # Ptr  |-> text_pre)
+  **  ((( &( "n" ) )) # Int  |-> n)
+  **  ((( &( "i" ) )) # Int  |-> i)
+  **  ((( &( "k" ) )) # Int  |-> k)
+  **  ((( &( "spacelen" ) )) # Int  |-> spacelen)
+  **  (store_string text_pre input )
+  **  ((( &( "out" ) )) # Ptr  |-> out)
+  **  (CharArray.full out k output )
+  **  (CharArray.undef_seg out k (n + 1 ) )
+|--
+  “ (95 <= INT_MAX) ” 
+  &&  “ ((INT_MIN) <= 95) ”
+.
+
+Definition fix_spaces_safety_wit_19 := 
+forall (text_pre: Z) (input: (@list Z)) (out: Z) (output: (@list Z)) (spacelen: Z) (k: Z) (i: Z) (n: Z) (PreH1 : (0 <= ((string_length (input)) + 1 ))) (PreH2 : (spacelen = 2)) (PreH3 : (spacelen <> 1)) (PreH4 : ((Znth i (c_string (input)) 0) <> 32)) (PreH5 : (i < n)) (PreH6 : (n = (string_length (input)))) (PreH7 : (0 <= i)) (PreH8 : (i <= n)) (PreH9 : (0 <= k)) (PreH10 : (0 <= spacelen)) (PreH11 : ((k + spacelen ) <= i)) (PreH12 : (k = (Zlength (output)))) (PreH13 : (fix_spaces_state_z_140 input output i spacelen )) (PreH14 : (valid_string input )) (PreH15 : (problem_140_pre_z input )) (PreH16 : (ascii_range_z input )) (PreH17 : ((string_length (input)) < INT_MAX)) ,
+  (CharArray.full out (k + 1 ) (app (output) ((cons (95) ((@nil Z))))) )
+  **  (CharArray.undef_seg out (k + 1 ) (n + 1 ) )
+  **  (CharArray.full text_pre ((string_length (input)) + 1 ) (c_string (input)) )
+  **  ((( &( "text" ) )) # Ptr  |-> text_pre)
+  **  ((( &( "n" ) )) # Int  |-> n)
+  **  ((( &( "i" ) )) # Int  |-> i)
+  **  ((( &( "k" ) )) # Int  |-> k)
+  **  ((( &( "spacelen" ) )) # Int  |-> spacelen)
+  **  ((( &( "out" ) )) # Ptr  |-> out)
+|--
+  “ ((k + 1 ) <= INT_MAX) ” 
+  &&  “ ((INT_MIN) <= (k + 1 )) ”
+.
+
+Definition fix_spaces_safety_wit_20 := 
+forall (text_pre: Z) (input: (@list Z)) (out: Z) (output: (@list Z)) (spacelen: Z) (k: Z) (i: Z) (n: Z) (PreH1 : (0 <= ((string_length (input)) + 1 ))) (PreH2 : (spacelen = 2)) (PreH3 : (spacelen <> 1)) (PreH4 : ((Znth i (c_string (input)) 0) <> 32)) (PreH5 : (i < n)) (PreH6 : (n = (string_length (input)))) (PreH7 : (0 <= i)) (PreH8 : (i <= n)) (PreH9 : (0 <= k)) (PreH10 : (0 <= spacelen)) (PreH11 : ((k + spacelen ) <= i)) (PreH12 : (k = (Zlength (output)))) (PreH13 : (fix_spaces_state_z_140 input output i spacelen )) (PreH14 : (valid_string input )) (PreH15 : (problem_140_pre_z input )) (PreH16 : (ascii_range_z input )) (PreH17 : ((string_length (input)) < INT_MAX)) ,
+  (CharArray.full out (k + 1 ) (app (output) ((cons (95) ((@nil Z))))) )
+  **  (CharArray.undef_seg out (k + 1 ) (n + 1 ) )
+  **  (CharArray.full text_pre ((string_length (input)) + 1 ) (c_string (input)) )
+  **  ((( &( "text" ) )) # Ptr  |-> text_pre)
+  **  ((( &( "n" ) )) # Int  |-> n)
+  **  ((( &( "i" ) )) # Int  |-> i)
+  **  ((( &( "k" ) )) # Int  |-> k)
+  **  ((( &( "spacelen" ) )) # Int  |-> spacelen)
+  **  ((( &( "out" ) )) # Ptr  |-> out)
+|--
+  “ (1 <= INT_MAX) ” 
+  &&  “ ((INT_MIN) <= 1) ”
+.
+
+Definition fix_spaces_safety_wit_21 := 
+forall (text_pre: Z) (input: (@list Z)) (out: Z) (output: (@list Z)) (spacelen: Z) (k: Z) (i: Z) (n: Z) (PreH1 : (0 <= ((string_length (input)) + 1 ))) (PreH2 : (spacelen = 2)) (PreH3 : (spacelen <> 1)) (PreH4 : ((Znth i (c_string (input)) 0) <> 32)) (PreH5 : (i < n)) (PreH6 : (n = (string_length (input)))) (PreH7 : (0 <= i)) (PreH8 : (i <= n)) (PreH9 : (0 <= k)) (PreH10 : (0 <= spacelen)) (PreH11 : ((k + spacelen ) <= i)) (PreH12 : (k = (Zlength (output)))) (PreH13 : (fix_spaces_state_z_140 input output i spacelen )) (PreH14 : (valid_string input )) (PreH15 : (problem_140_pre_z input )) (PreH16 : (ascii_range_z input )) (PreH17 : ((string_length (input)) < INT_MAX)) ,
+  (CharArray.full out (k + 1 ) (app (output) ((cons (95) ((@nil Z))))) )
+  **  (CharArray.undef_seg out (k + 1 ) (n + 1 ) )
+  **  (CharArray.full text_pre ((string_length (input)) + 1 ) (c_string (input)) )
+  **  ((( &( "text" ) )) # Ptr  |-> text_pre)
+  **  ((( &( "n" ) )) # Int  |-> n)
+  **  ((( &( "i" ) )) # Int  |-> i)
+  **  ((( &( "k" ) )) # Int  |-> (k + 1 ))
+  **  ((( &( "spacelen" ) )) # Int  |-> spacelen)
+  **  ((( &( "out" ) )) # Ptr  |-> out)
+|--
+  “ (95 <= INT_MAX) ” 
+  &&  “ ((INT_MIN) <= 95) ”
+.
+
+Definition fix_spaces_safety_wit_22 := 
+forall (text_pre: Z) (input: (@list Z)) (out: Z) (output: (@list Z)) (spacelen: Z) (k: Z) (i: Z) (n: Z) (PreH1 : (0 <= (k + 1 ))) (PreH2 : (0 <= ((string_length (input)) + 1 ))) (PreH3 : (spacelen = 2)) (PreH4 : (spacelen <> 1)) (PreH5 : ((Znth i (c_string (input)) 0) <> 32)) (PreH6 : (i < n)) (PreH7 : (n = (string_length (input)))) (PreH8 : (0 <= i)) (PreH9 : (i <= n)) (PreH10 : (0 <= k)) (PreH11 : (0 <= spacelen)) (PreH12 : ((k + spacelen ) <= i)) (PreH13 : (k = (Zlength (output)))) (PreH14 : (fix_spaces_state_z_140 input output i spacelen )) (PreH15 : (valid_string input )) (PreH16 : (problem_140_pre_z input )) (PreH17 : (ascii_range_z input )) (PreH18 : ((string_length (input)) < INT_MAX)) ,
+  (CharArray.full out ((k + 1 ) + 1 ) (app ((app (output) ((cons (95) ((@nil Z)))))) ((cons (95) ((@nil Z))))) )
+  **  (CharArray.undef_seg out ((k + 1 ) + 1 ) (n + 1 ) )
+  **  (CharArray.full text_pre ((string_length (input)) + 1 ) (c_string (input)) )
+  **  ((( &( "text" ) )) # Ptr  |-> text_pre)
+  **  ((( &( "n" ) )) # Int  |-> n)
+  **  ((( &( "i" ) )) # Int  |-> i)
+  **  ((( &( "k" ) )) # Int  |-> (k + 1 ))
+  **  ((( &( "spacelen" ) )) # Int  |-> spacelen)
+  **  ((( &( "out" ) )) # Ptr  |-> out)
+|--
+  “ (((k + 1 ) + 1 ) <= INT_MAX) ” 
+  &&  “ ((INT_MIN) <= ((k + 1 ) + 1 )) ”
+.
+
+Definition fix_spaces_safety_wit_23 := 
+forall (text_pre: Z) (input: (@list Z)) (out: Z) (output: (@list Z)) (spacelen: Z) (k: Z) (i: Z) (n: Z) (PreH1 : (0 <= (k + 1 ))) (PreH2 : (0 <= ((string_length (input)) + 1 ))) (PreH3 : (spacelen = 2)) (PreH4 : (spacelen <> 1)) (PreH5 : ((Znth i (c_string (input)) 0) <> 32)) (PreH6 : (i < n)) (PreH7 : (n = (string_length (input)))) (PreH8 : (0 <= i)) (PreH9 : (i <= n)) (PreH10 : (0 <= k)) (PreH11 : (0 <= spacelen)) (PreH12 : ((k + spacelen ) <= i)) (PreH13 : (k = (Zlength (output)))) (PreH14 : (fix_spaces_state_z_140 input output i spacelen )) (PreH15 : (valid_string input )) (PreH16 : (problem_140_pre_z input )) (PreH17 : (ascii_range_z input )) (PreH18 : ((string_length (input)) < INT_MAX)) ,
+  (CharArray.full out ((k + 1 ) + 1 ) (app ((app (output) ((cons (95) ((@nil Z)))))) ((cons (95) ((@nil Z))))) )
+  **  (CharArray.undef_seg out ((k + 1 ) + 1 ) (n + 1 ) )
+  **  (CharArray.full text_pre ((string_length (input)) + 1 ) (c_string (input)) )
+  **  ((( &( "text" ) )) # Ptr  |-> text_pre)
+  **  ((( &( "n" ) )) # Int  |-> n)
+  **  ((( &( "i" ) )) # Int  |-> i)
+  **  ((( &( "k" ) )) # Int  |-> (k + 1 ))
+  **  ((( &( "spacelen" ) )) # Int  |-> spacelen)
+  **  ((( &( "out" ) )) # Ptr  |-> out)
+|--
+  “ (1 <= INT_MAX) ” 
+  &&  “ ((INT_MIN) <= 1) ”
+.
+
+Definition fix_spaces_safety_wit_24 := 
+forall (text_pre: Z) (input: (@list Z)) (out: Z) (output: (@list Z)) (spacelen: Z) (k: Z) (i: Z) (n: Z) (PreH1 : (0 <= (k + 1 ))) (PreH2 : (0 <= ((string_length (input)) + 1 ))) (PreH3 : (spacelen = 2)) (PreH4 : (spacelen <> 1)) (PreH5 : ((Znth i (c_string (input)) 0) <> 32)) (PreH6 : (i < n)) (PreH7 : (n = (string_length (input)))) (PreH8 : (0 <= i)) (PreH9 : (i <= n)) (PreH10 : (0 <= k)) (PreH11 : (0 <= spacelen)) (PreH12 : ((k + spacelen ) <= i)) (PreH13 : (k = (Zlength (output)))) (PreH14 : (fix_spaces_state_z_140 input output i spacelen )) (PreH15 : (valid_string input )) (PreH16 : (problem_140_pre_z input )) (PreH17 : (ascii_range_z input )) (PreH18 : ((string_length (input)) < INT_MAX)) ,
+  (CharArray.full out ((k + 1 ) + 1 ) (app ((app (output) ((cons (95) ((@nil Z)))))) ((cons (95) ((@nil Z))))) )
+  **  (CharArray.undef_seg out ((k + 1 ) + 1 ) (n + 1 ) )
+  **  (CharArray.full text_pre ((string_length (input)) + 1 ) (c_string (input)) )
+  **  ((( &( "text" ) )) # Ptr  |-> text_pre)
+  **  ((( &( "n" ) )) # Int  |-> n)
+  **  ((( &( "i" ) )) # Int  |-> i)
+  **  ((( &( "k" ) )) # Int  |-> ((k + 1 ) + 1 ))
+  **  ((( &( "spacelen" ) )) # Int  |-> spacelen)
+  **  ((( &( "out" ) )) # Ptr  |-> out)
+|--
+  “ (2 <= INT_MAX) ” 
+  &&  “ ((INT_MIN) <= 2) ”
+.
+
+Definition fix_spaces_safety_wit_25 := 
+forall (text_pre: Z) (input: (@list Z)) (out: Z) (output: (@list Z)) (spacelen: Z) (k: Z) (i: Z) (n: Z) (PreH1 : (spacelen <> 2)) (PreH2 : (0 <= ((string_length (input)) + 1 ))) (PreH3 : (spacelen = 1)) (PreH4 : ((Znth i (c_string (input)) 0) <> 32)) (PreH5 : (i < n)) (PreH6 : (n = (string_length (input)))) (PreH7 : (0 <= i)) (PreH8 : (i <= n)) (PreH9 : (0 <= k)) (PreH10 : (0 <= spacelen)) (PreH11 : ((k + spacelen ) <= i)) (PreH12 : (k = (Zlength (output)))) (PreH13 : (fix_spaces_state_z_140 input output i spacelen )) (PreH14 : (valid_string input )) (PreH15 : (problem_140_pre_z input )) (PreH16 : (ascii_range_z input )) (PreH17 : ((string_length (input)) < INT_MAX)) ,
+  (CharArray.full out (k + 1 ) (app (output) ((cons (95) ((@nil Z))))) )
+  **  (CharArray.undef_seg out (k + 1 ) (n + 1 ) )
+  **  (CharArray.full text_pre ((string_length (input)) + 1 ) (c_string (input)) )
+  **  ((( &( "text" ) )) # Ptr  |-> text_pre)
+  **  ((( &( "n" ) )) # Int  |-> n)
+  **  ((( &( "i" ) )) # Int  |-> i)
+  **  ((( &( "k" ) )) # Int  |-> (k + 1 ))
+  **  ((( &( "spacelen" ) )) # Int  |-> spacelen)
+  **  ((( &( "out" ) )) # Ptr  |-> out)
+|--
+  “ (2 <= INT_MAX) ” 
+  &&  “ ((INT_MIN) <= 2) ”
+.
+
+Definition fix_spaces_safety_wit_26 := 
+forall (text_pre: Z) (input: (@list Z)) (out: Z) (output: (@list Z)) (spacelen: Z) (k: Z) (i: Z) (n: Z) (PreH1 : (spacelen <> 2)) (PreH2 : (spacelen <> 1)) (PreH3 : ((Znth i (c_string (input)) 0) <> 32)) (PreH4 : (i < n)) (PreH5 : (n = (string_length (input)))) (PreH6 : (0 <= i)) (PreH7 : (i <= n)) (PreH8 : (0 <= k)) (PreH9 : (0 <= spacelen)) (PreH10 : ((k + spacelen ) <= i)) (PreH11 : (k = (Zlength (output)))) (PreH12 : (fix_spaces_state_z_140 input output i spacelen )) (PreH13 : (valid_string input )) (PreH14 : (problem_140_pre_z input )) (PreH15 : (ascii_range_z input )) (PreH16 : ((string_length (input)) < INT_MAX)) ,
+  ((( &( "text" ) )) # Ptr  |-> text_pre)
+  **  ((( &( "n" ) )) # Int  |-> n)
+  **  ((( &( "i" ) )) # Int  |-> i)
+  **  ((( &( "k" ) )) # Int  |-> k)
+  **  ((( &( "spacelen" ) )) # Int  |-> spacelen)
+  **  (store_string text_pre input )
+  **  ((( &( "out" ) )) # Ptr  |-> out)
+  **  (CharArray.full out k output )
+  **  (CharArray.undef_seg out k (n + 1 ) )
+|--
+  “ (2 <= INT_MAX) ” 
+  &&  “ ((INT_MIN) <= 2) ”
+.
+
+Definition fix_spaces_safety_wit_27 := 
+forall (text_pre: Z) (input: (@list Z)) (out: Z) (output: (@list Z)) (spacelen: Z) (k: Z) (i: Z) (n: Z) (PreH1 : (spacelen > 2)) (PreH2 : (0 <= (k + 1 ))) (PreH3 : (0 <= ((string_length (input)) + 1 ))) (PreH4 : (spacelen = 2)) (PreH5 : (spacelen <> 1)) (PreH6 : ((Znth i (c_string (input)) 0) <> 32)) (PreH7 : (i < n)) (PreH8 : (n = (string_length (input)))) (PreH9 : (0 <= i)) (PreH10 : (i <= n)) (PreH11 : (0 <= k)) (PreH12 : (0 <= spacelen)) (PreH13 : ((k + spacelen ) <= i)) (PreH14 : (k = (Zlength (output)))) (PreH15 : (fix_spaces_state_z_140 input output i spacelen )) (PreH16 : (valid_string input )) (PreH17 : (problem_140_pre_z input )) (PreH18 : (ascii_range_z input )) (PreH19 : ((string_length (input)) < INT_MAX)) ,
+  (CharArray.full out ((k + 1 ) + 1 ) (app ((app (output) ((cons (95) ((@nil Z)))))) ((cons (95) ((@nil Z))))) )
+  **  (CharArray.undef_seg out ((k + 1 ) + 1 ) (n + 1 ) )
+  **  (CharArray.full text_pre ((string_length (input)) + 1 ) (c_string (input)) )
+  **  ((( &( "text" ) )) # Ptr  |-> text_pre)
+  **  ((( &( "n" ) )) # Int  |-> n)
+  **  ((( &( "i" ) )) # Int  |-> i)
+  **  ((( &( "k" ) )) # Int  |-> ((k + 1 ) + 1 ))
+  **  ((( &( "spacelen" ) )) # Int  |-> spacelen)
+  **  ((( &( "out" ) )) # Ptr  |-> out)
+|--
+  “ False ”
+.
+
+Definition fix_spaces_safety_wit_28 := 
+forall (text_pre: Z) (input: (@list Z)) (out: Z) (output: (@list Z)) (spacelen: Z) (k: Z) (i: Z) (n: Z) (PreH1 : (spacelen > 2)) (PreH2 : (spacelen <> 2)) (PreH3 : (0 <= ((string_length (input)) + 1 ))) (PreH4 : (spacelen = 1)) (PreH5 : ((Znth i (c_string (input)) 0) <> 32)) (PreH6 : (i < n)) (PreH7 : (n = (string_length (input)))) (PreH8 : (0 <= i)) (PreH9 : (i <= n)) (PreH10 : (0 <= k)) (PreH11 : (0 <= spacelen)) (PreH12 : ((k + spacelen ) <= i)) (PreH13 : (k = (Zlength (output)))) (PreH14 : (fix_spaces_state_z_140 input output i spacelen )) (PreH15 : (valid_string input )) (PreH16 : (problem_140_pre_z input )) (PreH17 : (ascii_range_z input )) (PreH18 : ((string_length (input)) < INT_MAX)) ,
+  (CharArray.full out (k + 1 ) (app (output) ((cons (95) ((@nil Z))))) )
+  **  (CharArray.undef_seg out (k + 1 ) (n + 1 ) )
+  **  (CharArray.full text_pre ((string_length (input)) + 1 ) (c_string (input)) )
+  **  ((( &( "text" ) )) # Ptr  |-> text_pre)
+  **  ((( &( "n" ) )) # Int  |-> n)
+  **  ((( &( "i" ) )) # Int  |-> i)
+  **  ((( &( "k" ) )) # Int  |-> (k + 1 ))
+  **  ((( &( "spacelen" ) )) # Int  |-> spacelen)
+  **  ((( &( "out" ) )) # Ptr  |-> out)
+|--
+  “ False ”
+.
+
+Definition fix_spaces_safety_wit_29 := 
+forall (text_pre: Z) (input: (@list Z)) (out: Z) (output: (@list Z)) (spacelen: Z) (k: Z) (i: Z) (n: Z) (PreH1 : (spacelen > 2)) (PreH2 : (spacelen <> 2)) (PreH3 : (spacelen <> 1)) (PreH4 : ((Znth i (c_string (input)) 0) <> 32)) (PreH5 : (i < n)) (PreH6 : (n = (string_length (input)))) (PreH7 : (0 <= i)) (PreH8 : (i <= n)) (PreH9 : (0 <= k)) (PreH10 : (0 <= spacelen)) (PreH11 : ((k + spacelen ) <= i)) (PreH12 : (k = (Zlength (output)))) (PreH13 : (fix_spaces_state_z_140 input output i spacelen )) (PreH14 : (valid_string input )) (PreH15 : (problem_140_pre_z input )) (PreH16 : (ascii_range_z input )) (PreH17 : ((string_length (input)) < INT_MAX)) ,
+  ((( &( "text" ) )) # Ptr  |-> text_pre)
+  **  ((( &( "n" ) )) # Int  |-> n)
+  **  ((( &( "i" ) )) # Int  |-> i)
+  **  ((( &( "k" ) )) # Int  |-> k)
+  **  ((( &( "spacelen" ) )) # Int  |-> spacelen)
+  **  (store_string text_pre input )
+  **  ((( &( "out" ) )) # Ptr  |-> out)
+  **  (CharArray.full out k output )
+  **  (CharArray.undef_seg out k (n + 1 ) )
+|--
+  “ (45 <= INT_MAX) ” 
+  &&  “ ((INT_MIN) <= 45) ”
+.
+
+Definition fix_spaces_safety_wit_30 := 
+forall (text_pre: Z) (input: (@list Z)) (out: Z) (output: (@list Z)) (spacelen: Z) (k: Z) (i: Z) (n: Z) (PreH1 : (0 <= ((string_length (input)) + 1 ))) (PreH2 : (spacelen > 2)) (PreH3 : (spacelen <> 2)) (PreH4 : (spacelen <> 1)) (PreH5 : ((Znth i (c_string (input)) 0) <> 32)) (PreH6 : (i < n)) (PreH7 : (n = (string_length (input)))) (PreH8 : (0 <= i)) (PreH9 : (i <= n)) (PreH10 : (0 <= k)) (PreH11 : (0 <= spacelen)) (PreH12 : ((k + spacelen ) <= i)) (PreH13 : (k = (Zlength (output)))) (PreH14 : (fix_spaces_state_z_140 input output i spacelen )) (PreH15 : (valid_string input )) (PreH16 : (problem_140_pre_z input )) (PreH17 : (ascii_range_z input )) (PreH18 : ((string_length (input)) < INT_MAX)) ,
+  (CharArray.full out (k + 1 ) (app (output) ((cons (45) ((@nil Z))))) )
+  **  (CharArray.undef_seg out (k + 1 ) (n + 1 ) )
+  **  (CharArray.full text_pre ((string_length (input)) + 1 ) (c_string (input)) )
+  **  ((( &( "text" ) )) # Ptr  |-> text_pre)
+  **  ((( &( "n" ) )) # Int  |-> n)
+  **  ((( &( "i" ) )) # Int  |-> i)
+  **  ((( &( "k" ) )) # Int  |-> k)
+  **  ((( &( "spacelen" ) )) # Int  |-> spacelen)
+  **  ((( &( "out" ) )) # Ptr  |-> out)
+|--
+  “ ((k + 1 ) <= INT_MAX) ” 
+  &&  “ ((INT_MIN) <= (k + 1 )) ”
+.
+
+Definition fix_spaces_safety_wit_31 := 
+forall (text_pre: Z) (input: (@list Z)) (out: Z) (output: (@list Z)) (spacelen: Z) (k: Z) (i: Z) (n: Z) (PreH1 : (0 <= ((string_length (input)) + 1 ))) (PreH2 : (spacelen > 2)) (PreH3 : (spacelen <> 2)) (PreH4 : (spacelen <> 1)) (PreH5 : ((Znth i (c_string (input)) 0) <> 32)) (PreH6 : (i < n)) (PreH7 : (n = (string_length (input)))) (PreH8 : (0 <= i)) (PreH9 : (i <= n)) (PreH10 : (0 <= k)) (PreH11 : (0 <= spacelen)) (PreH12 : ((k + spacelen ) <= i)) (PreH13 : (k = (Zlength (output)))) (PreH14 : (fix_spaces_state_z_140 input output i spacelen )) (PreH15 : (valid_string input )) (PreH16 : (problem_140_pre_z input )) (PreH17 : (ascii_range_z input )) (PreH18 : ((string_length (input)) < INT_MAX)) ,
+  (CharArray.full out (k + 1 ) (app (output) ((cons (45) ((@nil Z))))) )
+  **  (CharArray.undef_seg out (k + 1 ) (n + 1 ) )
+  **  (CharArray.full text_pre ((string_length (input)) + 1 ) (c_string (input)) )
+  **  ((( &( "text" ) )) # Ptr  |-> text_pre)
+  **  ((( &( "n" ) )) # Int  |-> n)
+  **  ((( &( "i" ) )) # Int  |-> i)
+  **  ((( &( "k" ) )) # Int  |-> k)
+  **  ((( &( "spacelen" ) )) # Int  |-> spacelen)
+  **  ((( &( "out" ) )) # Ptr  |-> out)
+|--
+  “ (1 <= INT_MAX) ” 
+  &&  “ ((INT_MIN) <= 1) ”
+.
+
+Definition fix_spaces_safety_wit_32 := 
+forall (text_pre: Z) (input: (@list Z)) (out: Z) (output: (@list Z)) (spacelen: Z) (k: Z) (i: Z) (n: Z) (PreH1 : (0 <= ((string_length (input)) + 1 ))) (PreH2 : (spacelen > 2)) (PreH3 : (spacelen <> 2)) (PreH4 : (spacelen <> 1)) (PreH5 : ((Znth i (c_string (input)) 0) <> 32)) (PreH6 : (i < n)) (PreH7 : (n = (string_length (input)))) (PreH8 : (0 <= i)) (PreH9 : (i <= n)) (PreH10 : (0 <= k)) (PreH11 : (0 <= spacelen)) (PreH12 : ((k + spacelen ) <= i)) (PreH13 : (k = (Zlength (output)))) (PreH14 : (fix_spaces_state_z_140 input output i spacelen )) (PreH15 : (valid_string input )) (PreH16 : (problem_140_pre_z input )) (PreH17 : (ascii_range_z input )) (PreH18 : ((string_length (input)) < INT_MAX)) ,
+  (CharArray.full out (k + 1 ) (app (output) ((cons (45) ((@nil Z))))) )
+  **  (CharArray.undef_seg out (k + 1 ) (n + 1 ) )
+  **  (CharArray.full text_pre ((string_length (input)) + 1 ) (c_string (input)) )
+  **  ((( &( "text" ) )) # Ptr  |-> text_pre)
+  **  ((( &( "n" ) )) # Int  |-> n)
+  **  ((( &( "i" ) )) # Int  |-> i)
+  **  ((( &( "k" ) )) # Int  |-> (k + 1 ))
+  **  ((( &( "spacelen" ) )) # Int  |-> spacelen)
+  **  ((( &( "out" ) )) # Ptr  |-> out)
+|--
+  “ (0 <= INT_MAX) ” 
+  &&  “ ((INT_MIN) <= 0) ”
+.
+
+Definition fix_spaces_safety_wit_33 := 
+forall (text_pre: Z) (input: (@list Z)) (out: Z) (output: (@list Z)) (spacelen: Z) (k: Z) (i: Z) (n: Z) (PreH1 : (spacelen <= 2)) (PreH2 : (0 <= (k + 1 ))) (PreH3 : (0 <= ((string_length (input)) + 1 ))) (PreH4 : (spacelen = 2)) (PreH5 : (spacelen <> 1)) (PreH6 : ((Znth i (c_string (input)) 0) <> 32)) (PreH7 : (i < n)) (PreH8 : (n = (string_length (input)))) (PreH9 : (0 <= i)) (PreH10 : (i <= n)) (PreH11 : (0 <= k)) (PreH12 : (0 <= spacelen)) (PreH13 : ((k + spacelen ) <= i)) (PreH14 : (k = (Zlength (output)))) (PreH15 : (fix_spaces_state_z_140 input output i spacelen )) (PreH16 : (valid_string input )) (PreH17 : (problem_140_pre_z input )) (PreH18 : (ascii_range_z input )) (PreH19 : ((string_length (input)) < INT_MAX)) ,
+  (CharArray.full out ((k + 1 ) + 1 ) (app ((app (output) ((cons (95) ((@nil Z)))))) ((cons (95) ((@nil Z))))) )
+  **  (CharArray.undef_seg out ((k + 1 ) + 1 ) (n + 1 ) )
+  **  (CharArray.full text_pre ((string_length (input)) + 1 ) (c_string (input)) )
+  **  ((( &( "text" ) )) # Ptr  |-> text_pre)
+  **  ((( &( "n" ) )) # Int  |-> n)
+  **  ((( &( "i" ) )) # Int  |-> i)
+  **  ((( &( "k" ) )) # Int  |-> ((k + 1 ) + 1 ))
+  **  ((( &( "spacelen" ) )) # Int  |-> spacelen)
+  **  ((( &( "out" ) )) # Ptr  |-> out)
+|--
+  “ (0 <= INT_MAX) ” 
+  &&  “ ((INT_MIN) <= 0) ”
+.
+
+Definition fix_spaces_safety_wit_34 := 
+forall (text_pre: Z) (input: (@list Z)) (out: Z) (output: (@list Z)) (spacelen: Z) (k: Z) (i: Z) (n: Z) (PreH1 : (spacelen <= 2)) (PreH2 : (spacelen <> 2)) (PreH3 : (0 <= ((string_length (input)) + 1 ))) (PreH4 : (spacelen = 1)) (PreH5 : ((Znth i (c_string (input)) 0) <> 32)) (PreH6 : (i < n)) (PreH7 : (n = (string_length (input)))) (PreH8 : (0 <= i)) (PreH9 : (i <= n)) (PreH10 : (0 <= k)) (PreH11 : (0 <= spacelen)) (PreH12 : ((k + spacelen ) <= i)) (PreH13 : (k = (Zlength (output)))) (PreH14 : (fix_spaces_state_z_140 input output i spacelen )) (PreH15 : (valid_string input )) (PreH16 : (problem_140_pre_z input )) (PreH17 : (ascii_range_z input )) (PreH18 : ((string_length (input)) < INT_MAX)) ,
+  (CharArray.full out (k + 1 ) (app (output) ((cons (95) ((@nil Z))))) )
+  **  (CharArray.undef_seg out (k + 1 ) (n + 1 ) )
+  **  (CharArray.full text_pre ((string_length (input)) + 1 ) (c_string (input)) )
+  **  ((( &( "text" ) )) # Ptr  |-> text_pre)
+  **  ((( &( "n" ) )) # Int  |-> n)
+  **  ((( &( "i" ) )) # Int  |-> i)
+  **  ((( &( "k" ) )) # Int  |-> (k + 1 ))
+  **  ((( &( "spacelen" ) )) # Int  |-> spacelen)
+  **  ((( &( "out" ) )) # Ptr  |-> out)
+|--
+  “ (0 <= INT_MAX) ” 
+  &&  “ ((INT_MIN) <= 0) ”
+.
+
+Definition fix_spaces_safety_wit_35 := 
+forall (text_pre: Z) (input: (@list Z)) (out: Z) (output: (@list Z)) (spacelen: Z) (k: Z) (i: Z) (n: Z) (PreH1 : (spacelen <= 2)) (PreH2 : (spacelen <> 2)) (PreH3 : (spacelen <> 1)) (PreH4 : ((Znth i (c_string (input)) 0) <> 32)) (PreH5 : (i < n)) (PreH6 : (n = (string_length (input)))) (PreH7 : (0 <= i)) (PreH8 : (i <= n)) (PreH9 : (0 <= k)) (PreH10 : (0 <= spacelen)) (PreH11 : ((k + spacelen ) <= i)) (PreH12 : (k = (Zlength (output)))) (PreH13 : (fix_spaces_state_z_140 input output i spacelen )) (PreH14 : (valid_string input )) (PreH15 : (problem_140_pre_z input )) (PreH16 : (ascii_range_z input )) (PreH17 : ((string_length (input)) < INT_MAX)) ,
+  ((( &( "text" ) )) # Ptr  |-> text_pre)
+  **  ((( &( "n" ) )) # Int  |-> n)
+  **  ((( &( "i" ) )) # Int  |-> i)
+  **  ((( &( "k" ) )) # Int  |-> k)
+  **  ((( &( "spacelen" ) )) # Int  |-> spacelen)
+  **  (store_string text_pre input )
+  **  ((( &( "out" ) )) # Ptr  |-> out)
+  **  (CharArray.full out k output )
+  **  (CharArray.undef_seg out k (n + 1 ) )
+|--
+  “ (0 <= INT_MAX) ” 
+  &&  “ ((INT_MIN) <= 0) ”
+.
+
+Definition fix_spaces_safety_wit_36 := 
+forall (text_pre: Z) (input: (@list Z)) (out: Z) (output: (@list Z)) (spacelen: Z) (k: Z) (i: Z) (n: Z) (PreH1 : (0 <= (k + 1 ))) (PreH2 : (0 <= ((string_length (input)) + 1 ))) (PreH3 : (spacelen > 2)) (PreH4 : (spacelen <> 2)) (PreH5 : (spacelen <> 1)) (PreH6 : ((Znth i (c_string (input)) 0) <> 32)) (PreH7 : (i < n)) (PreH8 : (n = (string_length (input)))) (PreH9 : (0 <= i)) (PreH10 : (i <= n)) (PreH11 : (0 <= k)) (PreH12 : (0 <= spacelen)) (PreH13 : ((k + spacelen ) <= i)) (PreH14 : (k = (Zlength (output)))) (PreH15 : (fix_spaces_state_z_140 input output i spacelen )) (PreH16 : (valid_string input )) (PreH17 : (problem_140_pre_z input )) (PreH18 : (ascii_range_z input )) (PreH19 : ((string_length (input)) < INT_MAX)) ,
+  (CharArray.full out ((k + 1 ) + 1 ) (app ((app (output) ((cons (45) ((@nil Z)))))) ((cons ((Znth i (c_string (input)) 0)) ((@nil Z))))) )
+  **  (CharArray.undef_seg out ((k + 1 ) + 1 ) (n + 1 ) )
+  **  (CharArray.full text_pre ((string_length (input)) + 1 ) (c_string (input)) )
+  **  ((( &( "text" ) )) # Ptr  |-> text_pre)
+  **  ((( &( "n" ) )) # Int  |-> n)
+  **  ((( &( "i" ) )) # Int  |-> i)
+  **  ((( &( "k" ) )) # Int  |-> (k + 1 ))
+  **  ((( &( "spacelen" ) )) # Int  |-> 0)
+  **  ((( &( "out" ) )) # Ptr  |-> out)
+|--
+  “ (((k + 1 ) + 1 ) <= INT_MAX) ” 
+  &&  “ ((INT_MIN) <= ((k + 1 ) + 1 )) ”
+.
+
+Definition fix_spaces_safety_wit_37 := 
+forall (text_pre: Z) (input: (@list Z)) (out: Z) (output: (@list Z)) (spacelen: Z) (k: Z) (i: Z) (n: Z) (PreH1 : (0 <= (k + 1 ))) (PreH2 : (0 <= ((string_length (input)) + 1 ))) (PreH3 : (spacelen > 2)) (PreH4 : (spacelen <> 2)) (PreH5 : (spacelen <> 1)) (PreH6 : ((Znth i (c_string (input)) 0) <> 32)) (PreH7 : (i < n)) (PreH8 : (n = (string_length (input)))) (PreH9 : (0 <= i)) (PreH10 : (i <= n)) (PreH11 : (0 <= k)) (PreH12 : (0 <= spacelen)) (PreH13 : ((k + spacelen ) <= i)) (PreH14 : (k = (Zlength (output)))) (PreH15 : (fix_spaces_state_z_140 input output i spacelen )) (PreH16 : (valid_string input )) (PreH17 : (problem_140_pre_z input )) (PreH18 : (ascii_range_z input )) (PreH19 : ((string_length (input)) < INT_MAX)) ,
+  (CharArray.full out ((k + 1 ) + 1 ) (app ((app (output) ((cons (45) ((@nil Z)))))) ((cons ((Znth i (c_string (input)) 0)) ((@nil Z))))) )
+  **  (CharArray.undef_seg out ((k + 1 ) + 1 ) (n + 1 ) )
+  **  (CharArray.full text_pre ((string_length (input)) + 1 ) (c_string (input)) )
+  **  ((( &( "text" ) )) # Ptr  |-> text_pre)
+  **  ((( &( "n" ) )) # Int  |-> n)
+  **  ((( &( "i" ) )) # Int  |-> i)
+  **  ((( &( "k" ) )) # Int  |-> (k + 1 ))
+  **  ((( &( "spacelen" ) )) # Int  |-> 0)
+  **  ((( &( "out" ) )) # Ptr  |-> out)
+|--
+  “ (1 <= INT_MAX) ” 
+  &&  “ ((INT_MIN) <= 1) ”
+.
+
+Definition fix_spaces_safety_wit_38 := 
+forall (text_pre: Z) (input: (@list Z)) (out: Z) (output: (@list Z)) (spacelen: Z) (k: Z) (i: Z) (n: Z) (PreH1 : (0 <= ((k + 1 ) + 1 ))) (PreH2 : (spacelen <= 2)) (PreH3 : (0 <= (k + 1 ))) (PreH4 : (0 <= ((string_length (input)) + 1 ))) (PreH5 : (spacelen = 2)) (PreH6 : (spacelen <> 1)) (PreH7 : ((Znth i (c_string (input)) 0) <> 32)) (PreH8 : (i < n)) (PreH9 : (n = (string_length (input)))) (PreH10 : (0 <= i)) (PreH11 : (i <= n)) (PreH12 : (0 <= k)) (PreH13 : (0 <= spacelen)) (PreH14 : ((k + spacelen ) <= i)) (PreH15 : (k = (Zlength (output)))) (PreH16 : (fix_spaces_state_z_140 input output i spacelen )) (PreH17 : (valid_string input )) (PreH18 : (problem_140_pre_z input )) (PreH19 : (ascii_range_z input )) (PreH20 : ((string_length (input)) < INT_MAX)) ,
+  (CharArray.full out (((k + 1 ) + 1 ) + 1 ) (app ((app ((app (output) ((cons (95) ((@nil Z)))))) ((cons (95) ((@nil Z)))))) ((cons ((Znth i (c_string (input)) 0)) ((@nil Z))))) )
+  **  (CharArray.undef_seg out (((k + 1 ) + 1 ) + 1 ) (n + 1 ) )
+  **  (CharArray.full text_pre ((string_length (input)) + 1 ) (c_string (input)) )
+  **  ((( &( "text" ) )) # Ptr  |-> text_pre)
+  **  ((( &( "n" ) )) # Int  |-> n)
+  **  ((( &( "i" ) )) # Int  |-> i)
+  **  ((( &( "k" ) )) # Int  |-> ((k + 1 ) + 1 ))
+  **  ((( &( "spacelen" ) )) # Int  |-> 0)
+  **  ((( &( "out" ) )) # Ptr  |-> out)
+|--
+  “ ((((k + 1 ) + 1 ) + 1 ) <= INT_MAX) ” 
+  &&  “ ((INT_MIN) <= (((k + 1 ) + 1 ) + 1 )) ”
+.
+
+Definition fix_spaces_safety_wit_39 := 
+forall (text_pre: Z) (input: (@list Z)) (out: Z) (output: (@list Z)) (spacelen: Z) (k: Z) (i: Z) (n: Z) (PreH1 : (0 <= ((k + 1 ) + 1 ))) (PreH2 : (spacelen <= 2)) (PreH3 : (0 <= (k + 1 ))) (PreH4 : (0 <= ((string_length (input)) + 1 ))) (PreH5 : (spacelen = 2)) (PreH6 : (spacelen <> 1)) (PreH7 : ((Znth i (c_string (input)) 0) <> 32)) (PreH8 : (i < n)) (PreH9 : (n = (string_length (input)))) (PreH10 : (0 <= i)) (PreH11 : (i <= n)) (PreH12 : (0 <= k)) (PreH13 : (0 <= spacelen)) (PreH14 : ((k + spacelen ) <= i)) (PreH15 : (k = (Zlength (output)))) (PreH16 : (fix_spaces_state_z_140 input output i spacelen )) (PreH17 : (valid_string input )) (PreH18 : (problem_140_pre_z input )) (PreH19 : (ascii_range_z input )) (PreH20 : ((string_length (input)) < INT_MAX)) ,
+  (CharArray.full out (((k + 1 ) + 1 ) + 1 ) (app ((app ((app (output) ((cons (95) ((@nil Z)))))) ((cons (95) ((@nil Z)))))) ((cons ((Znth i (c_string (input)) 0)) ((@nil Z))))) )
+  **  (CharArray.undef_seg out (((k + 1 ) + 1 ) + 1 ) (n + 1 ) )
+  **  (CharArray.full text_pre ((string_length (input)) + 1 ) (c_string (input)) )
+  **  ((( &( "text" ) )) # Ptr  |-> text_pre)
+  **  ((( &( "n" ) )) # Int  |-> n)
+  **  ((( &( "i" ) )) # Int  |-> i)
+  **  ((( &( "k" ) )) # Int  |-> ((k + 1 ) + 1 ))
+  **  ((( &( "spacelen" ) )) # Int  |-> 0)
+  **  ((( &( "out" ) )) # Ptr  |-> out)
+|--
+  “ (1 <= INT_MAX) ” 
+  &&  “ ((INT_MIN) <= 1) ”
+.
+
+Definition fix_spaces_safety_wit_40 := 
+forall (text_pre: Z) (input: (@list Z)) (out: Z) (output: (@list Z)) (spacelen: Z) (k: Z) (i: Z) (n: Z) (PreH1 : (0 <= (k + 1 ))) (PreH2 : (spacelen <= 2)) (PreH3 : (spacelen <> 2)) (PreH4 : (0 <= ((string_length (input)) + 1 ))) (PreH5 : (spacelen = 1)) (PreH6 : ((Znth i (c_string (input)) 0) <> 32)) (PreH7 : (i < n)) (PreH8 : (n = (string_length (input)))) (PreH9 : (0 <= i)) (PreH10 : (i <= n)) (PreH11 : (0 <= k)) (PreH12 : (0 <= spacelen)) (PreH13 : ((k + spacelen ) <= i)) (PreH14 : (k = (Zlength (output)))) (PreH15 : (fix_spaces_state_z_140 input output i spacelen )) (PreH16 : (valid_string input )) (PreH17 : (problem_140_pre_z input )) (PreH18 : (ascii_range_z input )) (PreH19 : ((string_length (input)) < INT_MAX)) ,
+  (CharArray.full out ((k + 1 ) + 1 ) (app ((app (output) ((cons (95) ((@nil Z)))))) ((cons ((Znth i (c_string (input)) 0)) ((@nil Z))))) )
+  **  (CharArray.undef_seg out ((k + 1 ) + 1 ) (n + 1 ) )
+  **  (CharArray.full text_pre ((string_length (input)) + 1 ) (c_string (input)) )
+  **  ((( &( "text" ) )) # Ptr  |-> text_pre)
+  **  ((( &( "n" ) )) # Int  |-> n)
+  **  ((( &( "i" ) )) # Int  |-> i)
+  **  ((( &( "k" ) )) # Int  |-> (k + 1 ))
+  **  ((( &( "spacelen" ) )) # Int  |-> 0)
+  **  ((( &( "out" ) )) # Ptr  |-> out)
+|--
+  “ (((k + 1 ) + 1 ) <= INT_MAX) ” 
+  &&  “ ((INT_MIN) <= ((k + 1 ) + 1 )) ”
+.
+
+Definition fix_spaces_safety_wit_41 := 
+forall (text_pre: Z) (input: (@list Z)) (out: Z) (output: (@list Z)) (spacelen: Z) (k: Z) (i: Z) (n: Z) (PreH1 : (0 <= (k + 1 ))) (PreH2 : (spacelen <= 2)) (PreH3 : (spacelen <> 2)) (PreH4 : (0 <= ((string_length (input)) + 1 ))) (PreH5 : (spacelen = 1)) (PreH6 : ((Znth i (c_string (input)) 0) <> 32)) (PreH7 : (i < n)) (PreH8 : (n = (string_length (input)))) (PreH9 : (0 <= i)) (PreH10 : (i <= n)) (PreH11 : (0 <= k)) (PreH12 : (0 <= spacelen)) (PreH13 : ((k + spacelen ) <= i)) (PreH14 : (k = (Zlength (output)))) (PreH15 : (fix_spaces_state_z_140 input output i spacelen )) (PreH16 : (valid_string input )) (PreH17 : (problem_140_pre_z input )) (PreH18 : (ascii_range_z input )) (PreH19 : ((string_length (input)) < INT_MAX)) ,
+  (CharArray.full out ((k + 1 ) + 1 ) (app ((app (output) ((cons (95) ((@nil Z)))))) ((cons ((Znth i (c_string (input)) 0)) ((@nil Z))))) )
+  **  (CharArray.undef_seg out ((k + 1 ) + 1 ) (n + 1 ) )
+  **  (CharArray.full text_pre ((string_length (input)) + 1 ) (c_string (input)) )
+  **  ((( &( "text" ) )) # Ptr  |-> text_pre)
+  **  ((( &( "n" ) )) # Int  |-> n)
+  **  ((( &( "i" ) )) # Int  |-> i)
+  **  ((( &( "k" ) )) # Int  |-> (k + 1 ))
+  **  ((( &( "spacelen" ) )) # Int  |-> 0)
+  **  ((( &( "out" ) )) # Ptr  |-> out)
+|--
+  “ (1 <= INT_MAX) ” 
+  &&  “ ((INT_MIN) <= 1) ”
+.
+
+Definition fix_spaces_safety_wit_42 := 
+forall (text_pre: Z) (input: (@list Z)) (out: Z) (output: (@list Z)) (spacelen: Z) (k: Z) (i: Z) (n: Z) (PreH1 : (0 <= ((string_length (input)) + 1 ))) (PreH2 : (spacelen <= 2)) (PreH3 : (spacelen <> 2)) (PreH4 : (spacelen <> 1)) (PreH5 : ((Znth i (c_string (input)) 0) <> 32)) (PreH6 : (i < n)) (PreH7 : (n = (string_length (input)))) (PreH8 : (0 <= i)) (PreH9 : (i <= n)) (PreH10 : (0 <= k)) (PreH11 : (0 <= spacelen)) (PreH12 : ((k + spacelen ) <= i)) (PreH13 : (k = (Zlength (output)))) (PreH14 : (fix_spaces_state_z_140 input output i spacelen )) (PreH15 : (valid_string input )) (PreH16 : (problem_140_pre_z input )) (PreH17 : (ascii_range_z input )) (PreH18 : ((string_length (input)) < INT_MAX)) ,
+  (CharArray.full out (k + 1 ) (app (output) ((cons ((Znth i (c_string (input)) 0)) ((@nil Z))))) )
+  **  (CharArray.undef_seg out (k + 1 ) (n + 1 ) )
+  **  (CharArray.full text_pre ((string_length (input)) + 1 ) (c_string (input)) )
+  **  ((( &( "text" ) )) # Ptr  |-> text_pre)
+  **  ((( &( "n" ) )) # Int  |-> n)
+  **  ((( &( "i" ) )) # Int  |-> i)
+  **  ((( &( "k" ) )) # Int  |-> k)
+  **  ((( &( "spacelen" ) )) # Int  |-> 0)
+  **  ((( &( "out" ) )) # Ptr  |-> out)
+|--
+  “ ((k + 1 ) <= INT_MAX) ” 
+  &&  “ ((INT_MIN) <= (k + 1 )) ”
+.
+
+Definition fix_spaces_safety_wit_43 := 
+forall (text_pre: Z) (input: (@list Z)) (out: Z) (output: (@list Z)) (spacelen: Z) (k: Z) (i: Z) (n: Z) (PreH1 : (0 <= ((string_length (input)) + 1 ))) (PreH2 : (spacelen <= 2)) (PreH3 : (spacelen <> 2)) (PreH4 : (spacelen <> 1)) (PreH5 : ((Znth i (c_string (input)) 0) <> 32)) (PreH6 : (i < n)) (PreH7 : (n = (string_length (input)))) (PreH8 : (0 <= i)) (PreH9 : (i <= n)) (PreH10 : (0 <= k)) (PreH11 : (0 <= spacelen)) (PreH12 : ((k + spacelen ) <= i)) (PreH13 : (k = (Zlength (output)))) (PreH14 : (fix_spaces_state_z_140 input output i spacelen )) (PreH15 : (valid_string input )) (PreH16 : (problem_140_pre_z input )) (PreH17 : (ascii_range_z input )) (PreH18 : ((string_length (input)) < INT_MAX)) ,
+  (CharArray.full out (k + 1 ) (app (output) ((cons ((Znth i (c_string (input)) 0)) ((@nil Z))))) )
+  **  (CharArray.undef_seg out (k + 1 ) (n + 1 ) )
+  **  (CharArray.full text_pre ((string_length (input)) + 1 ) (c_string (input)) )
+  **  ((( &( "text" ) )) # Ptr  |-> text_pre)
+  **  ((( &( "n" ) )) # Int  |-> n)
+  **  ((( &( "i" ) )) # Int  |-> i)
+  **  ((( &( "k" ) )) # Int  |-> k)
+  **  ((( &( "spacelen" ) )) # Int  |-> 0)
+  **  ((( &( "out" ) )) # Ptr  |-> out)
+|--
+  “ (1 <= INT_MAX) ” 
+  &&  “ ((INT_MIN) <= 1) ”
+.
+
+Definition fix_spaces_safety_wit_44 := 
+forall (text_pre: Z) (input: (@list Z)) (output: (@list Z)) (n: Z) (i: Z) (k: Z) (spacelen: Z) (out: Z) (PreH1 : (n = (string_length (input)))) (PreH2 : (0 <= i)) (PreH3 : (i < n)) (PreH4 : (0 <= k)) (PreH5 : (0 <= spacelen)) (PreH6 : ((k + spacelen ) <= (i + 1 ))) (PreH7 : (k = (Zlength (output)))) (PreH8 : (fix_spaces_state_z_140 input output (i + 1 ) spacelen )) (PreH9 : (valid_string input )) (PreH10 : (problem_140_pre_z input )) (PreH11 : (ascii_range_z input )) (PreH12 : ((string_length (input)) < INT_MAX)) ,
+  ((( &( "text" ) )) # Ptr  |-> text_pre)
+  **  ((( &( "n" ) )) # Int  |-> n)
+  **  ((( &( "i" ) )) # Int  |-> i)
+  **  ((( &( "k" ) )) # Int  |-> k)
+  **  ((( &( "spacelen" ) )) # Int  |-> spacelen)
+  **  (store_string text_pre input )
+  **  ((( &( "out" ) )) # Ptr  |-> out)
+  **  (CharArray.full out k output )
+  **  (CharArray.undef_seg out k (n + 1 ) )
+|--
+  “ ((i + 1 ) <= INT_MAX) ” 
+  &&  “ ((INT_MIN) <= (i + 1 )) ”
+.
+
+Definition fix_spaces_safety_wit_45 := 
+forall (text_pre: Z) (input: (@list Z)) (out: Z) (output: (@list Z)) (spacelen: Z) (k: Z) (i: Z) (n: Z) (PreH1 : (i >= n)) (PreH2 : (n = (string_length (input)))) (PreH3 : (0 <= i)) (PreH4 : (i <= n)) (PreH5 : (0 <= k)) (PreH6 : (0 <= spacelen)) (PreH7 : ((k + spacelen ) <= i)) (PreH8 : (k = (Zlength (output)))) (PreH9 : (fix_spaces_state_z_140 input output i spacelen )) (PreH10 : (valid_string input )) (PreH11 : (problem_140_pre_z input )) (PreH12 : (ascii_range_z input )) (PreH13 : ((string_length (input)) < INT_MAX)) ,
+  ((( &( "text" ) )) # Ptr  |-> text_pre)
+  **  ((( &( "n" ) )) # Int  |-> n)
+  **  ((( &( "i" ) )) # Int  |-> i)
+  **  ((( &( "k" ) )) # Int  |-> k)
+  **  ((( &( "spacelen" ) )) # Int  |-> spacelen)
+  **  (store_string text_pre input )
+  **  ((( &( "out" ) )) # Ptr  |-> out)
+  **  (CharArray.full out k output )
+  **  (CharArray.undef_seg out k (n + 1 ) )
+|--
+  “ (1 <= INT_MAX) ” 
+  &&  “ ((INT_MIN) <= 1) ”
+.
+
+Definition fix_spaces_safety_wit_46 := 
+forall (text_pre: Z) (input: (@list Z)) (out: Z) (output: (@list Z)) (spacelen: Z) (k: Z) (i: Z) (n: Z) (PreH1 : (spacelen = 1)) (PreH2 : (i >= n)) (PreH3 : (n = (string_length (input)))) (PreH4 : (0 <= i)) (PreH5 : (i <= n)) (PreH6 : (0 <= k)) (PreH7 : (0 <= spacelen)) (PreH8 : ((k + spacelen ) <= i)) (PreH9 : (k = (Zlength (output)))) (PreH10 : (fix_spaces_state_z_140 input output i spacelen )) (PreH11 : (valid_string input )) (PreH12 : (problem_140_pre_z input )) (PreH13 : (ascii_range_z input )) (PreH14 : ((string_length (input)) < INT_MAX)) ,
+  ((( &( "text" ) )) # Ptr  |-> text_pre)
+  **  ((( &( "n" ) )) # Int  |-> n)
+  **  ((( &( "i" ) )) # Int  |-> i)
+  **  ((( &( "k" ) )) # Int  |-> k)
+  **  ((( &( "spacelen" ) )) # Int  |-> spacelen)
+  **  (store_string text_pre input )
+  **  ((( &( "out" ) )) # Ptr  |-> out)
+  **  (CharArray.full out k output )
+  **  (CharArray.undef_seg out k (n + 1 ) )
+|--
+  “ (95 <= INT_MAX) ” 
+  &&  “ ((INT_MIN) <= 95) ”
+.
+
+Definition fix_spaces_safety_wit_47 := 
+forall (text_pre: Z) (input: (@list Z)) (out: Z) (output: (@list Z)) (spacelen: Z) (k: Z) (i: Z) (n: Z) (PreH1 : (0 <= ((string_length (input)) + 1 ))) (PreH2 : (spacelen = 1)) (PreH3 : (i >= n)) (PreH4 : (n = (string_length (input)))) (PreH5 : (0 <= i)) (PreH6 : (i <= n)) (PreH7 : (0 <= k)) (PreH8 : (0 <= spacelen)) (PreH9 : ((k + spacelen ) <= i)) (PreH10 : (k = (Zlength (output)))) (PreH11 : (fix_spaces_state_z_140 input output i spacelen )) (PreH12 : (valid_string input )) (PreH13 : (problem_140_pre_z input )) (PreH14 : (ascii_range_z input )) (PreH15 : ((string_length (input)) < INT_MAX)) ,
+  (CharArray.full out (k + 1 ) (app (output) ((cons (95) ((@nil Z))))) )
+  **  (CharArray.undef_seg out (k + 1 ) (n + 1 ) )
+  **  (CharArray.full text_pre ((string_length (input)) + 1 ) (c_string (input)) )
+  **  ((( &( "text" ) )) # Ptr  |-> text_pre)
+  **  ((( &( "n" ) )) # Int  |-> n)
+  **  ((( &( "i" ) )) # Int  |-> i)
+  **  ((( &( "k" ) )) # Int  |-> k)
+  **  ((( &( "spacelen" ) )) # Int  |-> spacelen)
+  **  ((( &( "out" ) )) # Ptr  |-> out)
+|--
+  “ ((k + 1 ) <= INT_MAX) ” 
+  &&  “ ((INT_MIN) <= (k + 1 )) ”
+.
+
+Definition fix_spaces_safety_wit_48 := 
+forall (text_pre: Z) (input: (@list Z)) (out: Z) (output: (@list Z)) (spacelen: Z) (k: Z) (i: Z) (n: Z) (PreH1 : (0 <= ((string_length (input)) + 1 ))) (PreH2 : (spacelen = 1)) (PreH3 : (i >= n)) (PreH4 : (n = (string_length (input)))) (PreH5 : (0 <= i)) (PreH6 : (i <= n)) (PreH7 : (0 <= k)) (PreH8 : (0 <= spacelen)) (PreH9 : ((k + spacelen ) <= i)) (PreH10 : (k = (Zlength (output)))) (PreH11 : (fix_spaces_state_z_140 input output i spacelen )) (PreH12 : (valid_string input )) (PreH13 : (problem_140_pre_z input )) (PreH14 : (ascii_range_z input )) (PreH15 : ((string_length (input)) < INT_MAX)) ,
+  (CharArray.full out (k + 1 ) (app (output) ((cons (95) ((@nil Z))))) )
+  **  (CharArray.undef_seg out (k + 1 ) (n + 1 ) )
+  **  (CharArray.full text_pre ((string_length (input)) + 1 ) (c_string (input)) )
+  **  ((( &( "text" ) )) # Ptr  |-> text_pre)
+  **  ((( &( "n" ) )) # Int  |-> n)
+  **  ((( &( "i" ) )) # Int  |-> i)
+  **  ((( &( "k" ) )) # Int  |-> k)
+  **  ((( &( "spacelen" ) )) # Int  |-> spacelen)
+  **  ((( &( "out" ) )) # Ptr  |-> out)
+|--
+  “ (1 <= INT_MAX) ” 
+  &&  “ ((INT_MIN) <= 1) ”
+.
+
+Definition fix_spaces_safety_wit_49 := 
+forall (text_pre: Z) (input: (@list Z)) (out: Z) (output: (@list Z)) (spacelen: Z) (k: Z) (i: Z) (n: Z) (PreH1 : (0 <= ((string_length (input)) + 1 ))) (PreH2 : (spacelen = 1)) (PreH3 : (i >= n)) (PreH4 : (n = (string_length (input)))) (PreH5 : (0 <= i)) (PreH6 : (i <= n)) (PreH7 : (0 <= k)) (PreH8 : (0 <= spacelen)) (PreH9 : ((k + spacelen ) <= i)) (PreH10 : (k = (Zlength (output)))) (PreH11 : (fix_spaces_state_z_140 input output i spacelen )) (PreH12 : (valid_string input )) (PreH13 : (problem_140_pre_z input )) (PreH14 : (ascii_range_z input )) (PreH15 : ((string_length (input)) < INT_MAX)) ,
+  (CharArray.full out (k + 1 ) (app (output) ((cons (95) ((@nil Z))))) )
+  **  (CharArray.undef_seg out (k + 1 ) (n + 1 ) )
+  **  (CharArray.full text_pre ((string_length (input)) + 1 ) (c_string (input)) )
+  **  ((( &( "text" ) )) # Ptr  |-> text_pre)
+  **  ((( &( "n" ) )) # Int  |-> n)
+  **  ((( &( "i" ) )) # Int  |-> i)
+  **  ((( &( "k" ) )) # Int  |-> (k + 1 ))
+  **  ((( &( "spacelen" ) )) # Int  |-> spacelen)
+  **  ((( &( "out" ) )) # Ptr  |-> out)
+|--
+  “ (2 <= INT_MAX) ” 
+  &&  “ ((INT_MIN) <= 2) ”
+.
+
+Definition fix_spaces_safety_wit_50 := 
+forall (text_pre: Z) (input: (@list Z)) (out: Z) (output: (@list Z)) (spacelen: Z) (k: Z) (i: Z) (n: Z) (PreH1 : (spacelen <> 1)) (PreH2 : (i >= n)) (PreH3 : (n = (string_length (input)))) (PreH4 : (0 <= i)) (PreH5 : (i <= n)) (PreH6 : (0 <= k)) (PreH7 : (0 <= spacelen)) (PreH8 : ((k + spacelen ) <= i)) (PreH9 : (k = (Zlength (output)))) (PreH10 : (fix_spaces_state_z_140 input output i spacelen )) (PreH11 : (valid_string input )) (PreH12 : (problem_140_pre_z input )) (PreH13 : (ascii_range_z input )) (PreH14 : ((string_length (input)) < INT_MAX)) ,
+  ((( &( "text" ) )) # Ptr  |-> text_pre)
+  **  ((( &( "n" ) )) # Int  |-> n)
+  **  ((( &( "i" ) )) # Int  |-> i)
+  **  ((( &( "k" ) )) # Int  |-> k)
+  **  ((( &( "spacelen" ) )) # Int  |-> spacelen)
+  **  (store_string text_pre input )
+  **  ((( &( "out" ) )) # Ptr  |-> out)
+  **  (CharArray.full out k output )
+  **  (CharArray.undef_seg out k (n + 1 ) )
+|--
+  “ (2 <= INT_MAX) ” 
+  &&  “ ((INT_MIN) <= 2) ”
+.
+
+Definition fix_spaces_safety_wit_51 := 
+forall (text_pre: Z) (input: (@list Z)) (out: Z) (output: (@list Z)) (spacelen: Z) (k: Z) (i: Z) (n: Z) (PreH1 : (spacelen = 2)) (PreH2 : (0 <= ((string_length (input)) + 1 ))) (PreH3 : (spacelen = 1)) (PreH4 : (i >= n)) (PreH5 : (n = (string_length (input)))) (PreH6 : (0 <= i)) (PreH7 : (i <= n)) (PreH8 : (0 <= k)) (PreH9 : (0 <= spacelen)) (PreH10 : ((k + spacelen ) <= i)) (PreH11 : (k = (Zlength (output)))) (PreH12 : (fix_spaces_state_z_140 input output i spacelen )) (PreH13 : (valid_string input )) (PreH14 : (problem_140_pre_z input )) (PreH15 : (ascii_range_z input )) (PreH16 : ((string_length (input)) < INT_MAX)) ,
+  (CharArray.full out (k + 1 ) (app (output) ((cons (95) ((@nil Z))))) )
+  **  (CharArray.undef_seg out (k + 1 ) (n + 1 ) )
+  **  (CharArray.full text_pre ((string_length (input)) + 1 ) (c_string (input)) )
+  **  ((( &( "text" ) )) # Ptr  |-> text_pre)
+  **  ((( &( "n" ) )) # Int  |-> n)
+  **  ((( &( "i" ) )) # Int  |-> i)
+  **  ((( &( "k" ) )) # Int  |-> (k + 1 ))
+  **  ((( &( "spacelen" ) )) # Int  |-> spacelen)
+  **  ((( &( "out" ) )) # Ptr  |-> out)
+|--
+  “ False ”
+.
+
+Definition fix_spaces_safety_wit_52 := 
+forall (text_pre: Z) (input: (@list Z)) (out: Z) (output: (@list Z)) (spacelen: Z) (k: Z) (i: Z) (n: Z) (PreH1 : (spacelen = 2)) (PreH2 : (spacelen <> 1)) (PreH3 : (i >= n)) (PreH4 : (n = (string_length (input)))) (PreH5 : (0 <= i)) (PreH6 : (i <= n)) (PreH7 : (0 <= k)) (PreH8 : (0 <= spacelen)) (PreH9 : ((k + spacelen ) <= i)) (PreH10 : (k = (Zlength (output)))) (PreH11 : (fix_spaces_state_z_140 input output i spacelen )) (PreH12 : (valid_string input )) (PreH13 : (problem_140_pre_z input )) (PreH14 : (ascii_range_z input )) (PreH15 : ((string_length (input)) < INT_MAX)) ,
+  ((( &( "text" ) )) # Ptr  |-> text_pre)
+  **  ((( &( "n" ) )) # Int  |-> n)
+  **  ((( &( "i" ) )) # Int  |-> i)
+  **  ((( &( "k" ) )) # Int  |-> k)
+  **  ((( &( "spacelen" ) )) # Int  |-> spacelen)
+  **  (store_string text_pre input )
+  **  ((( &( "out" ) )) # Ptr  |-> out)
+  **  (CharArray.full out k output )
+  **  (CharArray.undef_seg out k (n + 1 ) )
+|--
+  “ (95 <= INT_MAX) ” 
+  &&  “ ((INT_MIN) <= 95) ”
+.
+
+Definition fix_spaces_safety_wit_53 := 
+forall (text_pre: Z) (input: (@list Z)) (out: Z) (output: (@list Z)) (spacelen: Z) (k: Z) (i: Z) (n: Z) (PreH1 : (0 <= ((string_length (input)) + 1 ))) (PreH2 : (spacelen = 2)) (PreH3 : (spacelen <> 1)) (PreH4 : (i >= n)) (PreH5 : (n = (string_length (input)))) (PreH6 : (0 <= i)) (PreH7 : (i <= n)) (PreH8 : (0 <= k)) (PreH9 : (0 <= spacelen)) (PreH10 : ((k + spacelen ) <= i)) (PreH11 : (k = (Zlength (output)))) (PreH12 : (fix_spaces_state_z_140 input output i spacelen )) (PreH13 : (valid_string input )) (PreH14 : (problem_140_pre_z input )) (PreH15 : (ascii_range_z input )) (PreH16 : ((string_length (input)) < INT_MAX)) ,
+  (CharArray.full out (k + 1 ) (app (output) ((cons (95) ((@nil Z))))) )
+  **  (CharArray.undef_seg out (k + 1 ) (n + 1 ) )
+  **  (CharArray.full text_pre ((string_length (input)) + 1 ) (c_string (input)) )
+  **  ((( &( "text" ) )) # Ptr  |-> text_pre)
+  **  ((( &( "n" ) )) # Int  |-> n)
+  **  ((( &( "i" ) )) # Int  |-> i)
+  **  ((( &( "k" ) )) # Int  |-> k)
+  **  ((( &( "spacelen" ) )) # Int  |-> spacelen)
+  **  ((( &( "out" ) )) # Ptr  |-> out)
+|--
+  “ ((k + 1 ) <= INT_MAX) ” 
+  &&  “ ((INT_MIN) <= (k + 1 )) ”
+.
+
+Definition fix_spaces_safety_wit_54 := 
+forall (text_pre: Z) (input: (@list Z)) (out: Z) (output: (@list Z)) (spacelen: Z) (k: Z) (i: Z) (n: Z) (PreH1 : (0 <= ((string_length (input)) + 1 ))) (PreH2 : (spacelen = 2)) (PreH3 : (spacelen <> 1)) (PreH4 : (i >= n)) (PreH5 : (n = (string_length (input)))) (PreH6 : (0 <= i)) (PreH7 : (i <= n)) (PreH8 : (0 <= k)) (PreH9 : (0 <= spacelen)) (PreH10 : ((k + spacelen ) <= i)) (PreH11 : (k = (Zlength (output)))) (PreH12 : (fix_spaces_state_z_140 input output i spacelen )) (PreH13 : (valid_string input )) (PreH14 : (problem_140_pre_z input )) (PreH15 : (ascii_range_z input )) (PreH16 : ((string_length (input)) < INT_MAX)) ,
+  (CharArray.full out (k + 1 ) (app (output) ((cons (95) ((@nil Z))))) )
+  **  (CharArray.undef_seg out (k + 1 ) (n + 1 ) )
+  **  (CharArray.full text_pre ((string_length (input)) + 1 ) (c_string (input)) )
+  **  ((( &( "text" ) )) # Ptr  |-> text_pre)
+  **  ((( &( "n" ) )) # Int  |-> n)
+  **  ((( &( "i" ) )) # Int  |-> i)
+  **  ((( &( "k" ) )) # Int  |-> k)
+  **  ((( &( "spacelen" ) )) # Int  |-> spacelen)
+  **  ((( &( "out" ) )) # Ptr  |-> out)
+|--
+  “ (1 <= INT_MAX) ” 
+  &&  “ ((INT_MIN) <= 1) ”
+.
+
+Definition fix_spaces_safety_wit_55 := 
+forall (text_pre: Z) (input: (@list Z)) (out: Z) (output: (@list Z)) (spacelen: Z) (k: Z) (i: Z) (n: Z) (PreH1 : (0 <= ((string_length (input)) + 1 ))) (PreH2 : (spacelen = 2)) (PreH3 : (spacelen <> 1)) (PreH4 : (i >= n)) (PreH5 : (n = (string_length (input)))) (PreH6 : (0 <= i)) (PreH7 : (i <= n)) (PreH8 : (0 <= k)) (PreH9 : (0 <= spacelen)) (PreH10 : ((k + spacelen ) <= i)) (PreH11 : (k = (Zlength (output)))) (PreH12 : (fix_spaces_state_z_140 input output i spacelen )) (PreH13 : (valid_string input )) (PreH14 : (problem_140_pre_z input )) (PreH15 : (ascii_range_z input )) (PreH16 : ((string_length (input)) < INT_MAX)) ,
+  (CharArray.full out (k + 1 ) (app (output) ((cons (95) ((@nil Z))))) )
+  **  (CharArray.undef_seg out (k + 1 ) (n + 1 ) )
+  **  (CharArray.full text_pre ((string_length (input)) + 1 ) (c_string (input)) )
+  **  ((( &( "text" ) )) # Ptr  |-> text_pre)
+  **  ((( &( "n" ) )) # Int  |-> n)
+  **  ((( &( "i" ) )) # Int  |-> i)
+  **  ((( &( "k" ) )) # Int  |-> (k + 1 ))
+  **  ((( &( "spacelen" ) )) # Int  |-> spacelen)
+  **  ((( &( "out" ) )) # Ptr  |-> out)
+|--
+  “ (95 <= INT_MAX) ” 
+  &&  “ ((INT_MIN) <= 95) ”
+.
+
+Definition fix_spaces_safety_wit_56 := 
+forall (text_pre: Z) (input: (@list Z)) (out: Z) (output: (@list Z)) (spacelen: Z) (k: Z) (i: Z) (n: Z) (PreH1 : (0 <= (k + 1 ))) (PreH2 : (0 <= ((string_length (input)) + 1 ))) (PreH3 : (spacelen = 2)) (PreH4 : (spacelen <> 1)) (PreH5 : (i >= n)) (PreH6 : (n = (string_length (input)))) (PreH7 : (0 <= i)) (PreH8 : (i <= n)) (PreH9 : (0 <= k)) (PreH10 : (0 <= spacelen)) (PreH11 : ((k + spacelen ) <= i)) (PreH12 : (k = (Zlength (output)))) (PreH13 : (fix_spaces_state_z_140 input output i spacelen )) (PreH14 : (valid_string input )) (PreH15 : (problem_140_pre_z input )) (PreH16 : (ascii_range_z input )) (PreH17 : ((string_length (input)) < INT_MAX)) ,
+  (CharArray.full out ((k + 1 ) + 1 ) (app ((app (output) ((cons (95) ((@nil Z)))))) ((cons (95) ((@nil Z))))) )
+  **  (CharArray.undef_seg out ((k + 1 ) + 1 ) (n + 1 ) )
+  **  (CharArray.full text_pre ((string_length (input)) + 1 ) (c_string (input)) )
+  **  ((( &( "text" ) )) # Ptr  |-> text_pre)
+  **  ((( &( "n" ) )) # Int  |-> n)
+  **  ((( &( "i" ) )) # Int  |-> i)
+  **  ((( &( "k" ) )) # Int  |-> (k + 1 ))
+  **  ((( &( "spacelen" ) )) # Int  |-> spacelen)
+  **  ((( &( "out" ) )) # Ptr  |-> out)
+|--
+  “ (((k + 1 ) + 1 ) <= INT_MAX) ” 
+  &&  “ ((INT_MIN) <= ((k + 1 ) + 1 )) ”
+.
+
+Definition fix_spaces_safety_wit_57 := 
+forall (text_pre: Z) (input: (@list Z)) (out: Z) (output: (@list Z)) (spacelen: Z) (k: Z) (i: Z) (n: Z) (PreH1 : (0 <= (k + 1 ))) (PreH2 : (0 <= ((string_length (input)) + 1 ))) (PreH3 : (spacelen = 2)) (PreH4 : (spacelen <> 1)) (PreH5 : (i >= n)) (PreH6 : (n = (string_length (input)))) (PreH7 : (0 <= i)) (PreH8 : (i <= n)) (PreH9 : (0 <= k)) (PreH10 : (0 <= spacelen)) (PreH11 : ((k + spacelen ) <= i)) (PreH12 : (k = (Zlength (output)))) (PreH13 : (fix_spaces_state_z_140 input output i spacelen )) (PreH14 : (valid_string input )) (PreH15 : (problem_140_pre_z input )) (PreH16 : (ascii_range_z input )) (PreH17 : ((string_length (input)) < INT_MAX)) ,
+  (CharArray.full out ((k + 1 ) + 1 ) (app ((app (output) ((cons (95) ((@nil Z)))))) ((cons (95) ((@nil Z))))) )
+  **  (CharArray.undef_seg out ((k + 1 ) + 1 ) (n + 1 ) )
+  **  (CharArray.full text_pre ((string_length (input)) + 1 ) (c_string (input)) )
+  **  ((( &( "text" ) )) # Ptr  |-> text_pre)
+  **  ((( &( "n" ) )) # Int  |-> n)
+  **  ((( &( "i" ) )) # Int  |-> i)
+  **  ((( &( "k" ) )) # Int  |-> (k + 1 ))
+  **  ((( &( "spacelen" ) )) # Int  |-> spacelen)
+  **  ((( &( "out" ) )) # Ptr  |-> out)
+|--
+  “ (1 <= INT_MAX) ” 
+  &&  “ ((INT_MIN) <= 1) ”
+.
+
+Definition fix_spaces_safety_wit_58 := 
+forall (text_pre: Z) (input: (@list Z)) (out: Z) (output: (@list Z)) (spacelen: Z) (k: Z) (i: Z) (n: Z) (PreH1 : (0 <= (k + 1 ))) (PreH2 : (0 <= ((string_length (input)) + 1 ))) (PreH3 : (spacelen = 2)) (PreH4 : (spacelen <> 1)) (PreH5 : (i >= n)) (PreH6 : (n = (string_length (input)))) (PreH7 : (0 <= i)) (PreH8 : (i <= n)) (PreH9 : (0 <= k)) (PreH10 : (0 <= spacelen)) (PreH11 : ((k + spacelen ) <= i)) (PreH12 : (k = (Zlength (output)))) (PreH13 : (fix_spaces_state_z_140 input output i spacelen )) (PreH14 : (valid_string input )) (PreH15 : (problem_140_pre_z input )) (PreH16 : (ascii_range_z input )) (PreH17 : ((string_length (input)) < INT_MAX)) ,
+  (CharArray.full out ((k + 1 ) + 1 ) (app ((app (output) ((cons (95) ((@nil Z)))))) ((cons (95) ((@nil Z))))) )
+  **  (CharArray.undef_seg out ((k + 1 ) + 1 ) (n + 1 ) )
+  **  (CharArray.full text_pre ((string_length (input)) + 1 ) (c_string (input)) )
+  **  ((( &( "text" ) )) # Ptr  |-> text_pre)
+  **  ((( &( "n" ) )) # Int  |-> n)
+  **  ((( &( "i" ) )) # Int  |-> i)
+  **  ((( &( "k" ) )) # Int  |-> ((k + 1 ) + 1 ))
+  **  ((( &( "spacelen" ) )) # Int  |-> spacelen)
+  **  ((( &( "out" ) )) # Ptr  |-> out)
+|--
+  “ (2 <= INT_MAX) ” 
+  &&  “ ((INT_MIN) <= 2) ”
+.
+
+Definition fix_spaces_safety_wit_59 := 
+forall (text_pre: Z) (input: (@list Z)) (out: Z) (output: (@list Z)) (spacelen: Z) (k: Z) (i: Z) (n: Z) (PreH1 : (spacelen <> 2)) (PreH2 : (0 <= ((string_length (input)) + 1 ))) (PreH3 : (spacelen = 1)) (PreH4 : (i >= n)) (PreH5 : (n = (string_length (input)))) (PreH6 : (0 <= i)) (PreH7 : (i <= n)) (PreH8 : (0 <= k)) (PreH9 : (0 <= spacelen)) (PreH10 : ((k + spacelen ) <= i)) (PreH11 : (k = (Zlength (output)))) (PreH12 : (fix_spaces_state_z_140 input output i spacelen )) (PreH13 : (valid_string input )) (PreH14 : (problem_140_pre_z input )) (PreH15 : (ascii_range_z input )) (PreH16 : ((string_length (input)) < INT_MAX)) ,
+  (CharArray.full out (k + 1 ) (app (output) ((cons (95) ((@nil Z))))) )
+  **  (CharArray.undef_seg out (k + 1 ) (n + 1 ) )
+  **  (CharArray.full text_pre ((string_length (input)) + 1 ) (c_string (input)) )
+  **  ((( &( "text" ) )) # Ptr  |-> text_pre)
+  **  ((( &( "n" ) )) # Int  |-> n)
+  **  ((( &( "i" ) )) # Int  |-> i)
+  **  ((( &( "k" ) )) # Int  |-> (k + 1 ))
+  **  ((( &( "spacelen" ) )) # Int  |-> spacelen)
+  **  ((( &( "out" ) )) # Ptr  |-> out)
+|--
+  “ (2 <= INT_MAX) ” 
+  &&  “ ((INT_MIN) <= 2) ”
+.
+
+Definition fix_spaces_safety_wit_60 := 
+forall (text_pre: Z) (input: (@list Z)) (out: Z) (output: (@list Z)) (spacelen: Z) (k: Z) (i: Z) (n: Z) (PreH1 : (spacelen <> 2)) (PreH2 : (spacelen <> 1)) (PreH3 : (i >= n)) (PreH4 : (n = (string_length (input)))) (PreH5 : (0 <= i)) (PreH6 : (i <= n)) (PreH7 : (0 <= k)) (PreH8 : (0 <= spacelen)) (PreH9 : ((k + spacelen ) <= i)) (PreH10 : (k = (Zlength (output)))) (PreH11 : (fix_spaces_state_z_140 input output i spacelen )) (PreH12 : (valid_string input )) (PreH13 : (problem_140_pre_z input )) (PreH14 : (ascii_range_z input )) (PreH15 : ((string_length (input)) < INT_MAX)) ,
+  ((( &( "text" ) )) # Ptr  |-> text_pre)
+  **  ((( &( "n" ) )) # Int  |-> n)
+  **  ((( &( "i" ) )) # Int  |-> i)
+  **  ((( &( "k" ) )) # Int  |-> k)
+  **  ((( &( "spacelen" ) )) # Int  |-> spacelen)
+  **  (store_string text_pre input )
+  **  ((( &( "out" ) )) # Ptr  |-> out)
+  **  (CharArray.full out k output )
+  **  (CharArray.undef_seg out k (n + 1 ) )
+|--
+  “ (2 <= INT_MAX) ” 
+  &&  “ ((INT_MIN) <= 2) ”
+.
+
+Definition fix_spaces_safety_wit_61 := 
+forall (text_pre: Z) (input: (@list Z)) (out: Z) (output: (@list Z)) (spacelen: Z) (k: Z) (i: Z) (n: Z) (PreH1 : (spacelen > 2)) (PreH2 : (0 <= (k + 1 ))) (PreH3 : (0 <= ((string_length (input)) + 1 ))) (PreH4 : (spacelen = 2)) (PreH5 : (spacelen <> 1)) (PreH6 : (i >= n)) (PreH7 : (n = (string_length (input)))) (PreH8 : (0 <= i)) (PreH9 : (i <= n)) (PreH10 : (0 <= k)) (PreH11 : (0 <= spacelen)) (PreH12 : ((k + spacelen ) <= i)) (PreH13 : (k = (Zlength (output)))) (PreH14 : (fix_spaces_state_z_140 input output i spacelen )) (PreH15 : (valid_string input )) (PreH16 : (problem_140_pre_z input )) (PreH17 : (ascii_range_z input )) (PreH18 : ((string_length (input)) < INT_MAX)) ,
+  (CharArray.full out ((k + 1 ) + 1 ) (app ((app (output) ((cons (95) ((@nil Z)))))) ((cons (95) ((@nil Z))))) )
+  **  (CharArray.undef_seg out ((k + 1 ) + 1 ) (n + 1 ) )
+  **  (CharArray.full text_pre ((string_length (input)) + 1 ) (c_string (input)) )
+  **  ((( &( "text" ) )) # Ptr  |-> text_pre)
+  **  ((( &( "n" ) )) # Int  |-> n)
+  **  ((( &( "i" ) )) # Int  |-> i)
+  **  ((( &( "k" ) )) # Int  |-> ((k + 1 ) + 1 ))
+  **  ((( &( "spacelen" ) )) # Int  |-> spacelen)
+  **  ((( &( "out" ) )) # Ptr  |-> out)
+|--
+  “ False ”
+.
+
+Definition fix_spaces_safety_wit_62 := 
+forall (text_pre: Z) (input: (@list Z)) (out: Z) (output: (@list Z)) (spacelen: Z) (k: Z) (i: Z) (n: Z) (PreH1 : (spacelen > 2)) (PreH2 : (spacelen <> 2)) (PreH3 : (0 <= ((string_length (input)) + 1 ))) (PreH4 : (spacelen = 1)) (PreH5 : (i >= n)) (PreH6 : (n = (string_length (input)))) (PreH7 : (0 <= i)) (PreH8 : (i <= n)) (PreH9 : (0 <= k)) (PreH10 : (0 <= spacelen)) (PreH11 : ((k + spacelen ) <= i)) (PreH12 : (k = (Zlength (output)))) (PreH13 : (fix_spaces_state_z_140 input output i spacelen )) (PreH14 : (valid_string input )) (PreH15 : (problem_140_pre_z input )) (PreH16 : (ascii_range_z input )) (PreH17 : ((string_length (input)) < INT_MAX)) ,
+  (CharArray.full out (k + 1 ) (app (output) ((cons (95) ((@nil Z))))) )
+  **  (CharArray.undef_seg out (k + 1 ) (n + 1 ) )
+  **  (CharArray.full text_pre ((string_length (input)) + 1 ) (c_string (input)) )
+  **  ((( &( "text" ) )) # Ptr  |-> text_pre)
+  **  ((( &( "n" ) )) # Int  |-> n)
+  **  ((( &( "i" ) )) # Int  |-> i)
+  **  ((( &( "k" ) )) # Int  |-> (k + 1 ))
+  **  ((( &( "spacelen" ) )) # Int  |-> spacelen)
+  **  ((( &( "out" ) )) # Ptr  |-> out)
+|--
+  “ False ”
+.
+
+Definition fix_spaces_safety_wit_63 := 
+forall (text_pre: Z) (input: (@list Z)) (out: Z) (output: (@list Z)) (spacelen: Z) (k: Z) (i: Z) (n: Z) (PreH1 : (spacelen > 2)) (PreH2 : (spacelen <> 2)) (PreH3 : (spacelen <> 1)) (PreH4 : (i >= n)) (PreH5 : (n = (string_length (input)))) (PreH6 : (0 <= i)) (PreH7 : (i <= n)) (PreH8 : (0 <= k)) (PreH9 : (0 <= spacelen)) (PreH10 : ((k + spacelen ) <= i)) (PreH11 : (k = (Zlength (output)))) (PreH12 : (fix_spaces_state_z_140 input output i spacelen )) (PreH13 : (valid_string input )) (PreH14 : (problem_140_pre_z input )) (PreH15 : (ascii_range_z input )) (PreH16 : ((string_length (input)) < INT_MAX)) ,
+  ((( &( "text" ) )) # Ptr  |-> text_pre)
+  **  ((( &( "n" ) )) # Int  |-> n)
+  **  ((( &( "i" ) )) # Int  |-> i)
+  **  ((( &( "k" ) )) # Int  |-> k)
+  **  ((( &( "spacelen" ) )) # Int  |-> spacelen)
+  **  (store_string text_pre input )
+  **  ((( &( "out" ) )) # Ptr  |-> out)
+  **  (CharArray.full out k output )
+  **  (CharArray.undef_seg out k (n + 1 ) )
+|--
+  “ (45 <= INT_MAX) ” 
+  &&  “ ((INT_MIN) <= 45) ”
+.
+
+Definition fix_spaces_safety_wit_64 := 
+forall (text_pre: Z) (input: (@list Z)) (out: Z) (output: (@list Z)) (spacelen: Z) (k: Z) (i: Z) (n: Z) (PreH1 : (0 <= ((string_length (input)) + 1 ))) (PreH2 : (spacelen > 2)) (PreH3 : (spacelen <> 2)) (PreH4 : (spacelen <> 1)) (PreH5 : (i >= n)) (PreH6 : (n = (string_length (input)))) (PreH7 : (0 <= i)) (PreH8 : (i <= n)) (PreH9 : (0 <= k)) (PreH10 : (0 <= spacelen)) (PreH11 : ((k + spacelen ) <= i)) (PreH12 : (k = (Zlength (output)))) (PreH13 : (fix_spaces_state_z_140 input output i spacelen )) (PreH14 : (valid_string input )) (PreH15 : (problem_140_pre_z input )) (PreH16 : (ascii_range_z input )) (PreH17 : ((string_length (input)) < INT_MAX)) ,
+  (CharArray.full out (k + 1 ) (app (output) ((cons (45) ((@nil Z))))) )
+  **  (CharArray.undef_seg out (k + 1 ) (n + 1 ) )
+  **  (CharArray.full text_pre ((string_length (input)) + 1 ) (c_string (input)) )
+  **  ((( &( "text" ) )) # Ptr  |-> text_pre)
+  **  ((( &( "n" ) )) # Int  |-> n)
+  **  ((( &( "i" ) )) # Int  |-> i)
+  **  ((( &( "k" ) )) # Int  |-> k)
+  **  ((( &( "spacelen" ) )) # Int  |-> spacelen)
+  **  ((( &( "out" ) )) # Ptr  |-> out)
+|--
+  “ ((k + 1 ) <= INT_MAX) ” 
+  &&  “ ((INT_MIN) <= (k + 1 )) ”
+.
+
+Definition fix_spaces_safety_wit_65 := 
+forall (text_pre: Z) (input: (@list Z)) (out: Z) (output: (@list Z)) (spacelen: Z) (k: Z) (i: Z) (n: Z) (PreH1 : (0 <= ((string_length (input)) + 1 ))) (PreH2 : (spacelen > 2)) (PreH3 : (spacelen <> 2)) (PreH4 : (spacelen <> 1)) (PreH5 : (i >= n)) (PreH6 : (n = (string_length (input)))) (PreH7 : (0 <= i)) (PreH8 : (i <= n)) (PreH9 : (0 <= k)) (PreH10 : (0 <= spacelen)) (PreH11 : ((k + spacelen ) <= i)) (PreH12 : (k = (Zlength (output)))) (PreH13 : (fix_spaces_state_z_140 input output i spacelen )) (PreH14 : (valid_string input )) (PreH15 : (problem_140_pre_z input )) (PreH16 : (ascii_range_z input )) (PreH17 : ((string_length (input)) < INT_MAX)) ,
+  (CharArray.full out (k + 1 ) (app (output) ((cons (45) ((@nil Z))))) )
+  **  (CharArray.undef_seg out (k + 1 ) (n + 1 ) )
+  **  (CharArray.full text_pre ((string_length (input)) + 1 ) (c_string (input)) )
+  **  ((( &( "text" ) )) # Ptr  |-> text_pre)
+  **  ((( &( "n" ) )) # Int  |-> n)
+  **  ((( &( "i" ) )) # Int  |-> i)
+  **  ((( &( "k" ) )) # Int  |-> k)
+  **  ((( &( "spacelen" ) )) # Int  |-> spacelen)
+  **  ((( &( "out" ) )) # Ptr  |-> out)
+|--
+  “ (1 <= INT_MAX) ” 
+  &&  “ ((INT_MIN) <= 1) ”
+.
+
+Definition fix_spaces_safety_wit_66 := 
+forall (text_pre: Z) (input: (@list Z)) (prefix: (@list Z)) (output: (@list Z)) (i: Z) (n: Z) (k: Z) (spacelen: Z) (out: Z) (PreH1 : (n = (string_length (input)))) (PreH2 : (0 <= k)) (PreH3 : (0 <= spacelen)) (PreH4 : (k <= n)) (PreH5 : (k = (Zlength (output)))) (PreH6 : (output = (app (prefix) ((flush_spaces_z_140 (spacelen)))))) (PreH7 : (fix_spaces_state_z_140 input prefix n spacelen )) (PreH8 : (valid_string input )) (PreH9 : (problem_140_pre_z input )) (PreH10 : (ascii_range_z input )) (PreH11 : ((string_length (input)) < INT_MAX)) ,
+  ((( &( "text" ) )) # Ptr  |-> text_pre)
+  **  ((( &( "i" ) )) # Int  |-> i)
+  **  ((( &( "n" ) )) # Int  |-> n)
+  **  ((( &( "k" ) )) # Int  |-> k)
+  **  ((( &( "spacelen" ) )) # Int  |-> spacelen)
+  **  (store_string text_pre input )
+  **  ((( &( "out" ) )) # Ptr  |-> out)
+  **  (CharArray.full out k output )
+  **  (CharArray.undef_seg out k (n + 1 ) )
+|--
+  “ (0 <= INT_MAX) ” 
+  &&  “ ((INT_MIN) <= 0) ”
+.
+
+Definition fix_spaces_entail_wit_1 := 
+(
+forall (text_pre: Z) (input: (@list Z)) (retval: Z) (retval_2: Z) (PreH1 : (retval_2 <> 0)) (PreH2 : (retval_2 <> 0)) (PreH3 : (retval = (string_length (input)))) (PreH4 : (0 <= ((string_length (input)) + 1 ))) (PreH5 : (valid_string input )) (PreH6 : (problem_140_pre_z input )) (PreH7 : (ascii_range_z input )) (PreH8 : ((string_length (input)) < INT_MAX)) ,
+  (CharArray.undef_full retval_2 (retval + 1 ) )
+  **  (CharArray.full text_pre ((string_length (input)) + 1 ) (c_string (input)) )
+|--
+  EX (output: (@list Z)) ,
+  “ (retval = (string_length (input))) ” 
+  &&  “ (0 <= 0) ” 
+  &&  “ (0 <= retval) ” 
+  &&  “ (0 <= 0) ” 
+  &&  “ (0 <= 0) ” 
+  &&  “ ((0 + 0 ) <= 0) ” 
+  &&  “ (0 = (Zlength (output))) ” 
+  &&  “ (fix_spaces_state_z_140 input output 0 0 ) ” 
+  &&  “ (valid_string input ) ” 
+  &&  “ (problem_140_pre_z input ) ” 
+  &&  “ (ascii_range_z input ) ” 
+  &&  “ ((string_length (input)) < INT_MAX) ”
+  &&  (store_string text_pre input )
+  **  (CharArray.full retval_2 0 output )
+  **  (CharArray.undef_seg retval_2 0 (retval + 1 ) )
+) \/
+(
+forall (input: (@list Z)) (retval: Z) (retval_2: Z) (PreH1 : (retval_2 <> 0)) (PreH2 : (retval_2 <> 0)) (PreH3 : (retval = (string_length (input)))) (PreH4 : (0 <= ((string_length (input)) + 1 ))) (PreH5 : (valid_string input )) (PreH6 : (problem_140_pre_z input )) (PreH7 : (ascii_range_z input )) (PreH8 : ((string_length (input)) < INT_MAX)) ,
+  (CharArray.undef_full retval_2 (retval + 1 ) )
+|--
+  “ (fix_spaces_state_z_140 input (@nil Z) 0 0 ) ” 
+  &&  “ (0 = (Zlength ((@nil Z)))) ” 
+  &&  “ (0 <= retval) ”
+  &&  (CharArray.undef_full retval_2 (retval + 1 ) )
+).
+
+Definition fix_spaces_entail_wit_1_split_goal_1 := 
+forall (input: (@list Z)) (retval: Z) (retval_2: Z) (PreH1 : (retval_2 <> 0)) (PreH2 : (retval_2 <> 0)) (PreH3 : (retval = (string_length (input)))) (PreH4 : (0 <= ((string_length (input)) + 1 ))) (PreH5 : (valid_string input )) (PreH6 : (problem_140_pre_z input )) (PreH7 : (ascii_range_z input )) (PreH8 : ((string_length (input)) < INT_MAX)) ,
+  (CharArray.undef_full retval_2 (retval + 1 ) )
+|--
+  “ (fix_spaces_state_z_140 input (@nil Z) 0 0 ) ”
+.
+
+Definition fix_spaces_entail_wit_1_split_goal_2 := 
+forall (input: (@list Z)) (retval: Z) (retval_2: Z) (PreH1 : (retval_2 <> 0)) (PreH2 : (retval_2 <> 0)) (PreH3 : (retval = (string_length (input)))) (PreH4 : (0 <= ((string_length (input)) + 1 ))) (PreH5 : (valid_string input )) (PreH6 : (problem_140_pre_z input )) (PreH7 : (ascii_range_z input )) (PreH8 : ((string_length (input)) < INT_MAX)) ,
+  (CharArray.undef_full retval_2 (retval + 1 ) )
+|--
+  “ (0 = (Zlength ((@nil Z)))) ”
+.
+
+Definition fix_spaces_entail_wit_1_split_goal_3 := 
+forall (input: (@list Z)) (retval: Z) (retval_2: Z) (PreH1 : (retval_2 <> 0)) (PreH2 : (retval_2 <> 0)) (PreH3 : (retval = (string_length (input)))) (PreH4 : (0 <= ((string_length (input)) + 1 ))) (PreH5 : (valid_string input )) (PreH6 : (problem_140_pre_z input )) (PreH7 : (ascii_range_z input )) (PreH8 : ((string_length (input)) < INT_MAX)) ,
+  (CharArray.undef_full retval_2 (retval + 1 ) )
+|--
+  “ (0 <= retval) ”
+.
+
+Definition fix_spaces_entail_wit_1_split_goal_spatial := 
+forall (input: (@list Z)) (retval: Z) (retval_2: Z) (PreH1 : (retval_2 <> 0)) (PreH2 : (retval_2 <> 0)) (PreH3 : (retval = (string_length (input)))) (PreH4 : (0 <= ((string_length (input)) + 1 ))) (PreH5 : (valid_string input )) (PreH6 : (problem_140_pre_z input )) (PreH7 : (ascii_range_z input )) (PreH8 : ((string_length (input)) < INT_MAX)) ,
+  (CharArray.undef_full retval_2 (retval + 1 ) )
+|--
+  (CharArray.undef_full retval_2 (retval + 1 ) )
+.
+
+Definition fix_spaces_entail_wit_2_1 := 
+(
+forall (text_pre: Z) (input: (@list Z)) (out: Z) (output_2: (@list Z)) (spacelen: Z) (k: Z) (i: Z) (n: Z) (PreH1 : (0 <= ((string_length (input)) + 1 ))) (PreH2 : (spacelen <= 2)) (PreH3 : (spacelen <> 2)) (PreH4 : (spacelen <> 1)) (PreH5 : ((Znth i (c_string (input)) 0) <> 32)) (PreH6 : (i < n)) (PreH7 : (n = (string_length (input)))) (PreH8 : (0 <= i)) (PreH9 : (i <= n)) (PreH10 : (0 <= k)) (PreH11 : (0 <= spacelen)) (PreH12 : ((k + spacelen ) <= i)) (PreH13 : (k = (Zlength (output_2)))) (PreH14 : (fix_spaces_state_z_140 input output_2 i spacelen )) (PreH15 : (valid_string input )) (PreH16 : (problem_140_pre_z input )) (PreH17 : (ascii_range_z input )) (PreH18 : ((string_length (input)) < INT_MAX)) ,
+  (CharArray.full out (k + 1 ) (app (output_2) ((cons ((Znth i (c_string (input)) 0)) ((@nil Z))))) )
+  **  (CharArray.undef_seg out (k + 1 ) (n + 1 ) )
+  **  (CharArray.full text_pre ((string_length (input)) + 1 ) (c_string (input)) )
+|--
+  EX (output: (@list Z)) ,
+  “ (n = (string_length (input))) ” 
+  &&  “ (0 <= i) ” 
+  &&  “ (i < n) ” 
+  &&  “ (0 <= (k + 1 )) ” 
+  &&  “ (0 <= 0) ” 
+  &&  “ (((k + 1 ) + 0 ) <= (i + 1 )) ” 
+  &&  “ ((k + 1 ) = (Zlength (output))) ” 
+  &&  “ (fix_spaces_state_z_140 input output (i + 1 ) 0 ) ” 
+  &&  “ (valid_string input ) ” 
+  &&  “ (problem_140_pre_z input ) ” 
+  &&  “ (ascii_range_z input ) ” 
+  &&  “ ((string_length (input)) < INT_MAX) ”
+  &&  (store_string text_pre input )
+  **  (CharArray.full out (k + 1 ) output )
+  **  (CharArray.undef_seg out (k + 1 ) (n + 1 ) )
+) \/
+(
+forall (input: (@list Z)) (output_2: (@list Z)) (spacelen: Z) (k: Z) (i: Z) (n: Z) (PreH1 : (0 <= ((string_length (input)) + 1 ))) (PreH2 : (spacelen <= 2)) (PreH3 : (spacelen <> 2)) (PreH4 : (spacelen <> 1)) (PreH5 : ((Znth i (c_string (input)) 0) <> 32)) (PreH6 : (i < n)) (PreH7 : (n = (string_length (input)))) (PreH8 : (0 <= i)) (PreH9 : (i <= n)) (PreH10 : (0 <= k)) (PreH11 : (0 <= spacelen)) (PreH12 : ((k + spacelen ) <= i)) (PreH13 : (k = (Zlength (output_2)))) (PreH14 : (fix_spaces_state_z_140 input output_2 i spacelen )) (PreH15 : (valid_string input )) (PreH16 : (problem_140_pre_z input )) (PreH17 : (ascii_range_z input )) (PreH18 : ((string_length (input)) < INT_MAX)) ,
+  TT && emp 
+|--
+  “ (fix_spaces_state_z_140 input (app (output_2) ((cons ((Znth i (c_string (input)) 0)) ((@nil Z))))) (i + 1 ) 0 ) ” 
+  &&  “ ((k + 1 ) = (Zlength ((app (output_2) ((cons ((Znth i (c_string (input)) 0)) ((@nil Z)))))))) ”
+  &&  emp
+).
+
+Definition fix_spaces_entail_wit_2_1_split_goal_1 := 
+forall (input: (@list Z)) (output_2: (@list Z)) (spacelen: Z) (k: Z) (i: Z) (n: Z) (PreH1 : (0 <= ((string_length (input)) + 1 ))) (PreH2 : (spacelen <= 2)) (PreH3 : (spacelen <> 2)) (PreH4 : (spacelen <> 1)) (PreH5 : ((Znth i (c_string (input)) 0) <> 32)) (PreH6 : (i < n)) (PreH7 : (n = (string_length (input)))) (PreH8 : (0 <= i)) (PreH9 : (i <= n)) (PreH10 : (0 <= k)) (PreH11 : (0 <= spacelen)) (PreH12 : ((k + spacelen ) <= i)) (PreH13 : (k = (Zlength (output_2)))) (PreH14 : (fix_spaces_state_z_140 input output_2 i spacelen )) (PreH15 : (valid_string input )) (PreH16 : (problem_140_pre_z input )) (PreH17 : (ascii_range_z input )) (PreH18 : ((string_length (input)) < INT_MAX)) ,
+  TT && emp 
+|--
+  “ (fix_spaces_state_z_140 input (app (output_2) ((cons ((Znth i (c_string (input)) 0)) ((@nil Z))))) (i + 1 ) 0 ) ”
+.
+
+Definition fix_spaces_entail_wit_2_1_split_goal_2 := 
+forall (input: (@list Z)) (output_2: (@list Z)) (spacelen: Z) (k: Z) (i: Z) (n: Z) (PreH1 : (0 <= ((string_length (input)) + 1 ))) (PreH2 : (spacelen <= 2)) (PreH3 : (spacelen <> 2)) (PreH4 : (spacelen <> 1)) (PreH5 : ((Znth i (c_string (input)) 0) <> 32)) (PreH6 : (i < n)) (PreH7 : (n = (string_length (input)))) (PreH8 : (0 <= i)) (PreH9 : (i <= n)) (PreH10 : (0 <= k)) (PreH11 : (0 <= spacelen)) (PreH12 : ((k + spacelen ) <= i)) (PreH13 : (k = (Zlength (output_2)))) (PreH14 : (fix_spaces_state_z_140 input output_2 i spacelen )) (PreH15 : (valid_string input )) (PreH16 : (problem_140_pre_z input )) (PreH17 : (ascii_range_z input )) (PreH18 : ((string_length (input)) < INT_MAX)) ,
+  TT && emp 
+|--
+  “ ((k + 1 ) = (Zlength ((app (output_2) ((cons ((Znth i (c_string (input)) 0)) ((@nil Z)))))))) ”
+.
+
+Definition fix_spaces_entail_wit_2_2 := 
+(
+forall (text_pre: Z) (input: (@list Z)) (out: Z) (output_2: (@list Z)) (spacelen: Z) (k: Z) (i: Z) (n: Z) (PreH1 : (0 <= (k + 1 ))) (PreH2 : (spacelen <= 2)) (PreH3 : (spacelen <> 2)) (PreH4 : (0 <= ((string_length (input)) + 1 ))) (PreH5 : (spacelen = 1)) (PreH6 : ((Znth i (c_string (input)) 0) <> 32)) (PreH7 : (i < n)) (PreH8 : (n = (string_length (input)))) (PreH9 : (0 <= i)) (PreH10 : (i <= n)) (PreH11 : (0 <= k)) (PreH12 : (0 <= spacelen)) (PreH13 : ((k + spacelen ) <= i)) (PreH14 : (k = (Zlength (output_2)))) (PreH15 : (fix_spaces_state_z_140 input output_2 i spacelen )) (PreH16 : (valid_string input )) (PreH17 : (problem_140_pre_z input )) (PreH18 : (ascii_range_z input )) (PreH19 : ((string_length (input)) < INT_MAX)) ,
+  (CharArray.full out ((k + 1 ) + 1 ) (app ((app (output_2) ((cons (95) ((@nil Z)))))) ((cons ((Znth i (c_string (input)) 0)) ((@nil Z))))) )
+  **  (CharArray.undef_seg out ((k + 1 ) + 1 ) (n + 1 ) )
+  **  (CharArray.full text_pre ((string_length (input)) + 1 ) (c_string (input)) )
+|--
+  EX (output: (@list Z)) ,
+  “ (n = (string_length (input))) ” 
+  &&  “ (0 <= i) ” 
+  &&  “ (i < n) ” 
+  &&  “ (0 <= ((k + 1 ) + 1 )) ” 
+  &&  “ (0 <= 0) ” 
+  &&  “ ((((k + 1 ) + 1 ) + 0 ) <= (i + 1 )) ” 
+  &&  “ (((k + 1 ) + 1 ) = (Zlength (output))) ” 
+  &&  “ (fix_spaces_state_z_140 input output (i + 1 ) 0 ) ” 
+  &&  “ (valid_string input ) ” 
+  &&  “ (problem_140_pre_z input ) ” 
+  &&  “ (ascii_range_z input ) ” 
+  &&  “ ((string_length (input)) < INT_MAX) ”
+  &&  (store_string text_pre input )
+  **  (CharArray.full out ((k + 1 ) + 1 ) output )
+  **  (CharArray.undef_seg out ((k + 1 ) + 1 ) (n + 1 ) )
+) \/
+(
+forall (input: (@list Z)) (output_2: (@list Z)) (spacelen: Z) (k: Z) (i: Z) (n: Z) (PreH1 : (0 <= (k + 1 ))) (PreH2 : (spacelen <= 2)) (PreH3 : (spacelen <> 2)) (PreH4 : (0 <= ((string_length (input)) + 1 ))) (PreH5 : (spacelen = 1)) (PreH6 : ((Znth i (c_string (input)) 0) <> 32)) (PreH7 : (i < n)) (PreH8 : (n = (string_length (input)))) (PreH9 : (0 <= i)) (PreH10 : (i <= n)) (PreH11 : (0 <= k)) (PreH12 : (0 <= spacelen)) (PreH13 : ((k + spacelen ) <= i)) (PreH14 : (k = (Zlength (output_2)))) (PreH15 : (fix_spaces_state_z_140 input output_2 i spacelen )) (PreH16 : (valid_string input )) (PreH17 : (problem_140_pre_z input )) (PreH18 : (ascii_range_z input )) (PreH19 : ((string_length (input)) < INT_MAX)) ,
+  TT && emp 
+|--
+  “ (fix_spaces_state_z_140 input (app ((app (output_2) ((cons (95) ((@nil Z)))))) ((cons ((Znth i (c_string (input)) 0)) ((@nil Z))))) (i + 1 ) 0 ) ” 
+  &&  “ (((k + 1 ) + 1 ) = (Zlength ((app ((app (output_2) ((cons (95) ((@nil Z)))))) ((cons ((Znth i (c_string (input)) 0)) ((@nil Z)))))))) ”
+  &&  emp
+).
+
+Definition fix_spaces_entail_wit_2_2_split_goal_1 := 
+forall (input: (@list Z)) (output_2: (@list Z)) (spacelen: Z) (k: Z) (i: Z) (n: Z) (PreH1 : (0 <= (k + 1 ))) (PreH2 : (spacelen <= 2)) (PreH3 : (spacelen <> 2)) (PreH4 : (0 <= ((string_length (input)) + 1 ))) (PreH5 : (spacelen = 1)) (PreH6 : ((Znth i (c_string (input)) 0) <> 32)) (PreH7 : (i < n)) (PreH8 : (n = (string_length (input)))) (PreH9 : (0 <= i)) (PreH10 : (i <= n)) (PreH11 : (0 <= k)) (PreH12 : (0 <= spacelen)) (PreH13 : ((k + spacelen ) <= i)) (PreH14 : (k = (Zlength (output_2)))) (PreH15 : (fix_spaces_state_z_140 input output_2 i spacelen )) (PreH16 : (valid_string input )) (PreH17 : (problem_140_pre_z input )) (PreH18 : (ascii_range_z input )) (PreH19 : ((string_length (input)) < INT_MAX)) ,
+  TT && emp 
+|--
+  “ (fix_spaces_state_z_140 input (app ((app (output_2) ((cons (95) ((@nil Z)))))) ((cons ((Znth i (c_string (input)) 0)) ((@nil Z))))) (i + 1 ) 0 ) ”
+.
+
+Definition fix_spaces_entail_wit_2_2_split_goal_2 := 
+forall (input: (@list Z)) (output_2: (@list Z)) (spacelen: Z) (k: Z) (i: Z) (n: Z) (PreH1 : (0 <= (k + 1 ))) (PreH2 : (spacelen <= 2)) (PreH3 : (spacelen <> 2)) (PreH4 : (0 <= ((string_length (input)) + 1 ))) (PreH5 : (spacelen = 1)) (PreH6 : ((Znth i (c_string (input)) 0) <> 32)) (PreH7 : (i < n)) (PreH8 : (n = (string_length (input)))) (PreH9 : (0 <= i)) (PreH10 : (i <= n)) (PreH11 : (0 <= k)) (PreH12 : (0 <= spacelen)) (PreH13 : ((k + spacelen ) <= i)) (PreH14 : (k = (Zlength (output_2)))) (PreH15 : (fix_spaces_state_z_140 input output_2 i spacelen )) (PreH16 : (valid_string input )) (PreH17 : (problem_140_pre_z input )) (PreH18 : (ascii_range_z input )) (PreH19 : ((string_length (input)) < INT_MAX)) ,
+  TT && emp 
+|--
+  “ (((k + 1 ) + 1 ) = (Zlength ((app ((app (output_2) ((cons (95) ((@nil Z)))))) ((cons ((Znth i (c_string (input)) 0)) ((@nil Z)))))))) ”
+.
+
+Definition fix_spaces_entail_wit_2_3 := 
+(
+forall (text_pre: Z) (input: (@list Z)) (out: Z) (output_2: (@list Z)) (spacelen: Z) (k: Z) (i: Z) (n: Z) (PreH1 : (0 <= ((k + 1 ) + 1 ))) (PreH2 : (spacelen <= 2)) (PreH3 : (0 <= (k + 1 ))) (PreH4 : (0 <= ((string_length (input)) + 1 ))) (PreH5 : (spacelen = 2)) (PreH6 : (spacelen <> 1)) (PreH7 : ((Znth i (c_string (input)) 0) <> 32)) (PreH8 : (i < n)) (PreH9 : (n = (string_length (input)))) (PreH10 : (0 <= i)) (PreH11 : (i <= n)) (PreH12 : (0 <= k)) (PreH13 : (0 <= spacelen)) (PreH14 : ((k + spacelen ) <= i)) (PreH15 : (k = (Zlength (output_2)))) (PreH16 : (fix_spaces_state_z_140 input output_2 i spacelen )) (PreH17 : (valid_string input )) (PreH18 : (problem_140_pre_z input )) (PreH19 : (ascii_range_z input )) (PreH20 : ((string_length (input)) < INT_MAX)) ,
+  (CharArray.full out (((k + 1 ) + 1 ) + 1 ) (app ((app ((app (output_2) ((cons (95) ((@nil Z)))))) ((cons (95) ((@nil Z)))))) ((cons ((Znth i (c_string (input)) 0)) ((@nil Z))))) )
+  **  (CharArray.undef_seg out (((k + 1 ) + 1 ) + 1 ) (n + 1 ) )
+  **  (CharArray.full text_pre ((string_length (input)) + 1 ) (c_string (input)) )
+|--
+  EX (output: (@list Z)) ,
+  “ (n = (string_length (input))) ” 
+  &&  “ (0 <= i) ” 
+  &&  “ (i < n) ” 
+  &&  “ (0 <= (((k + 1 ) + 1 ) + 1 )) ” 
+  &&  “ (0 <= 0) ” 
+  &&  “ (((((k + 1 ) + 1 ) + 1 ) + 0 ) <= (i + 1 )) ” 
+  &&  “ ((((k + 1 ) + 1 ) + 1 ) = (Zlength (output))) ” 
+  &&  “ (fix_spaces_state_z_140 input output (i + 1 ) 0 ) ” 
+  &&  “ (valid_string input ) ” 
+  &&  “ (problem_140_pre_z input ) ” 
+  &&  “ (ascii_range_z input ) ” 
+  &&  “ ((string_length (input)) < INT_MAX) ”
+  &&  (store_string text_pre input )
+  **  (CharArray.full out (((k + 1 ) + 1 ) + 1 ) output )
+  **  (CharArray.undef_seg out (((k + 1 ) + 1 ) + 1 ) (n + 1 ) )
+) \/
+(
+forall (input: (@list Z)) (output_2: (@list Z)) (spacelen: Z) (k: Z) (i: Z) (n: Z) (PreH1 : (0 <= ((k + 1 ) + 1 ))) (PreH2 : (spacelen <= 2)) (PreH3 : (0 <= (k + 1 ))) (PreH4 : (0 <= ((string_length (input)) + 1 ))) (PreH5 : (spacelen = 2)) (PreH6 : (spacelen <> 1)) (PreH7 : ((Znth i (c_string (input)) 0) <> 32)) (PreH8 : (i < n)) (PreH9 : (n = (string_length (input)))) (PreH10 : (0 <= i)) (PreH11 : (i <= n)) (PreH12 : (0 <= k)) (PreH13 : (0 <= spacelen)) (PreH14 : ((k + spacelen ) <= i)) (PreH15 : (k = (Zlength (output_2)))) (PreH16 : (fix_spaces_state_z_140 input output_2 i spacelen )) (PreH17 : (valid_string input )) (PreH18 : (problem_140_pre_z input )) (PreH19 : (ascii_range_z input )) (PreH20 : ((string_length (input)) < INT_MAX)) ,
+  TT && emp 
+|--
+  “ (fix_spaces_state_z_140 input (app ((app ((app (output_2) ((cons (95) ((@nil Z)))))) ((cons (95) ((@nil Z)))))) ((cons ((Znth i (c_string (input)) 0)) ((@nil Z))))) (i + 1 ) 0 ) ” 
+  &&  “ ((((k + 1 ) + 1 ) + 1 ) = (Zlength ((app ((app ((app (output_2) ((cons (95) ((@nil Z)))))) ((cons (95) ((@nil Z)))))) ((cons ((Znth i (c_string (input)) 0)) ((@nil Z)))))))) ”
+  &&  emp
+).
+
+Definition fix_spaces_entail_wit_2_3_split_goal_1 := 
+forall (input: (@list Z)) (output_2: (@list Z)) (spacelen: Z) (k: Z) (i: Z) (n: Z) (PreH1 : (0 <= ((k + 1 ) + 1 ))) (PreH2 : (spacelen <= 2)) (PreH3 : (0 <= (k + 1 ))) (PreH4 : (0 <= ((string_length (input)) + 1 ))) (PreH5 : (spacelen = 2)) (PreH6 : (spacelen <> 1)) (PreH7 : ((Znth i (c_string (input)) 0) <> 32)) (PreH8 : (i < n)) (PreH9 : (n = (string_length (input)))) (PreH10 : (0 <= i)) (PreH11 : (i <= n)) (PreH12 : (0 <= k)) (PreH13 : (0 <= spacelen)) (PreH14 : ((k + spacelen ) <= i)) (PreH15 : (k = (Zlength (output_2)))) (PreH16 : (fix_spaces_state_z_140 input output_2 i spacelen )) (PreH17 : (valid_string input )) (PreH18 : (problem_140_pre_z input )) (PreH19 : (ascii_range_z input )) (PreH20 : ((string_length (input)) < INT_MAX)) ,
+  TT && emp 
+|--
+  “ (fix_spaces_state_z_140 input (app ((app ((app (output_2) ((cons (95) ((@nil Z)))))) ((cons (95) ((@nil Z)))))) ((cons ((Znth i (c_string (input)) 0)) ((@nil Z))))) (i + 1 ) 0 ) ”
+.
+
+Definition fix_spaces_entail_wit_2_3_split_goal_2 := 
+forall (input: (@list Z)) (output_2: (@list Z)) (spacelen: Z) (k: Z) (i: Z) (n: Z) (PreH1 : (0 <= ((k + 1 ) + 1 ))) (PreH2 : (spacelen <= 2)) (PreH3 : (0 <= (k + 1 ))) (PreH4 : (0 <= ((string_length (input)) + 1 ))) (PreH5 : (spacelen = 2)) (PreH6 : (spacelen <> 1)) (PreH7 : ((Znth i (c_string (input)) 0) <> 32)) (PreH8 : (i < n)) (PreH9 : (n = (string_length (input)))) (PreH10 : (0 <= i)) (PreH11 : (i <= n)) (PreH12 : (0 <= k)) (PreH13 : (0 <= spacelen)) (PreH14 : ((k + spacelen ) <= i)) (PreH15 : (k = (Zlength (output_2)))) (PreH16 : (fix_spaces_state_z_140 input output_2 i spacelen )) (PreH17 : (valid_string input )) (PreH18 : (problem_140_pre_z input )) (PreH19 : (ascii_range_z input )) (PreH20 : ((string_length (input)) < INT_MAX)) ,
+  TT && emp 
+|--
+  “ ((((k + 1 ) + 1 ) + 1 ) = (Zlength ((app ((app ((app (output_2) ((cons (95) ((@nil Z)))))) ((cons (95) ((@nil Z)))))) ((cons ((Znth i (c_string (input)) 0)) ((@nil Z)))))))) ”
+.
+
+Definition fix_spaces_entail_wit_2_4 := 
+(
+forall (text_pre: Z) (input: (@list Z)) (out: Z) (output_2: (@list Z)) (spacelen: Z) (k: Z) (i: Z) (n: Z) (PreH1 : (0 <= (k + 1 ))) (PreH2 : (0 <= ((string_length (input)) + 1 ))) (PreH3 : (spacelen > 2)) (PreH4 : (spacelen <> 2)) (PreH5 : (spacelen <> 1)) (PreH6 : ((Znth i (c_string (input)) 0) <> 32)) (PreH7 : (i < n)) (PreH8 : (n = (string_length (input)))) (PreH9 : (0 <= i)) (PreH10 : (i <= n)) (PreH11 : (0 <= k)) (PreH12 : (0 <= spacelen)) (PreH13 : ((k + spacelen ) <= i)) (PreH14 : (k = (Zlength (output_2)))) (PreH15 : (fix_spaces_state_z_140 input output_2 i spacelen )) (PreH16 : (valid_string input )) (PreH17 : (problem_140_pre_z input )) (PreH18 : (ascii_range_z input )) (PreH19 : ((string_length (input)) < INT_MAX)) ,
+  (CharArray.full out ((k + 1 ) + 1 ) (app ((app (output_2) ((cons (45) ((@nil Z)))))) ((cons ((Znth i (c_string (input)) 0)) ((@nil Z))))) )
+  **  (CharArray.undef_seg out ((k + 1 ) + 1 ) (n + 1 ) )
+  **  (CharArray.full text_pre ((string_length (input)) + 1 ) (c_string (input)) )
+|--
+  EX (output: (@list Z)) ,
+  “ (n = (string_length (input))) ” 
+  &&  “ (0 <= i) ” 
+  &&  “ (i < n) ” 
+  &&  “ (0 <= ((k + 1 ) + 1 )) ” 
+  &&  “ (0 <= 0) ” 
+  &&  “ ((((k + 1 ) + 1 ) + 0 ) <= (i + 1 )) ” 
+  &&  “ (((k + 1 ) + 1 ) = (Zlength (output))) ” 
+  &&  “ (fix_spaces_state_z_140 input output (i + 1 ) 0 ) ” 
+  &&  “ (valid_string input ) ” 
+  &&  “ (problem_140_pre_z input ) ” 
+  &&  “ (ascii_range_z input ) ” 
+  &&  “ ((string_length (input)) < INT_MAX) ”
+  &&  (store_string text_pre input )
+  **  (CharArray.full out ((k + 1 ) + 1 ) output )
+  **  (CharArray.undef_seg out ((k + 1 ) + 1 ) (n + 1 ) )
+) \/
+(
+forall (input: (@list Z)) (output_2: (@list Z)) (spacelen: Z) (k: Z) (i: Z) (n: Z) (PreH1 : (0 <= (k + 1 ))) (PreH2 : (0 <= ((string_length (input)) + 1 ))) (PreH3 : (spacelen > 2)) (PreH4 : (spacelen <> 2)) (PreH5 : (spacelen <> 1)) (PreH6 : ((Znth i (c_string (input)) 0) <> 32)) (PreH7 : (i < n)) (PreH8 : (n = (string_length (input)))) (PreH9 : (0 <= i)) (PreH10 : (i <= n)) (PreH11 : (0 <= k)) (PreH12 : (0 <= spacelen)) (PreH13 : ((k + spacelen ) <= i)) (PreH14 : (k = (Zlength (output_2)))) (PreH15 : (fix_spaces_state_z_140 input output_2 i spacelen )) (PreH16 : (valid_string input )) (PreH17 : (problem_140_pre_z input )) (PreH18 : (ascii_range_z input )) (PreH19 : ((string_length (input)) < INT_MAX)) ,
+  TT && emp 
+|--
+  “ (fix_spaces_state_z_140 input (app ((app (output_2) ((cons (45) ((@nil Z)))))) ((cons ((Znth i (c_string (input)) 0)) ((@nil Z))))) (i + 1 ) 0 ) ” 
+  &&  “ (((k + 1 ) + 1 ) = (Zlength ((app ((app (output_2) ((cons (45) ((@nil Z)))))) ((cons ((Znth i (c_string (input)) 0)) ((@nil Z)))))))) ”
+  &&  emp
+).
+
+Definition fix_spaces_entail_wit_2_4_split_goal_1 := 
+forall (input: (@list Z)) (output_2: (@list Z)) (spacelen: Z) (k: Z) (i: Z) (n: Z) (PreH1 : (0 <= (k + 1 ))) (PreH2 : (0 <= ((string_length (input)) + 1 ))) (PreH3 : (spacelen > 2)) (PreH4 : (spacelen <> 2)) (PreH5 : (spacelen <> 1)) (PreH6 : ((Znth i (c_string (input)) 0) <> 32)) (PreH7 : (i < n)) (PreH8 : (n = (string_length (input)))) (PreH9 : (0 <= i)) (PreH10 : (i <= n)) (PreH11 : (0 <= k)) (PreH12 : (0 <= spacelen)) (PreH13 : ((k + spacelen ) <= i)) (PreH14 : (k = (Zlength (output_2)))) (PreH15 : (fix_spaces_state_z_140 input output_2 i spacelen )) (PreH16 : (valid_string input )) (PreH17 : (problem_140_pre_z input )) (PreH18 : (ascii_range_z input )) (PreH19 : ((string_length (input)) < INT_MAX)) ,
+  TT && emp 
+|--
+  “ (fix_spaces_state_z_140 input (app ((app (output_2) ((cons (45) ((@nil Z)))))) ((cons ((Znth i (c_string (input)) 0)) ((@nil Z))))) (i + 1 ) 0 ) ”
+.
+
+Definition fix_spaces_entail_wit_2_4_split_goal_2 := 
+forall (input: (@list Z)) (output_2: (@list Z)) (spacelen: Z) (k: Z) (i: Z) (n: Z) (PreH1 : (0 <= (k + 1 ))) (PreH2 : (0 <= ((string_length (input)) + 1 ))) (PreH3 : (spacelen > 2)) (PreH4 : (spacelen <> 2)) (PreH5 : (spacelen <> 1)) (PreH6 : ((Znth i (c_string (input)) 0) <> 32)) (PreH7 : (i < n)) (PreH8 : (n = (string_length (input)))) (PreH9 : (0 <= i)) (PreH10 : (i <= n)) (PreH11 : (0 <= k)) (PreH12 : (0 <= spacelen)) (PreH13 : ((k + spacelen ) <= i)) (PreH14 : (k = (Zlength (output_2)))) (PreH15 : (fix_spaces_state_z_140 input output_2 i spacelen )) (PreH16 : (valid_string input )) (PreH17 : (problem_140_pre_z input )) (PreH18 : (ascii_range_z input )) (PreH19 : ((string_length (input)) < INT_MAX)) ,
+  TT && emp 
+|--
+  “ (((k + 1 ) + 1 ) = (Zlength ((app ((app (output_2) ((cons (45) ((@nil Z)))))) ((cons ((Znth i (c_string (input)) 0)) ((@nil Z)))))))) ”
+.
+
+Definition fix_spaces_entail_wit_2_5 := 
+(
+forall (text_pre: Z) (input: (@list Z)) (out: Z) (output_2: (@list Z)) (spacelen: Z) (k: Z) (i: Z) (n: Z) (PreH1 : ((Znth i (c_string (input)) 0) = 32)) (PreH2 : (i < n)) (PreH3 : (n = (string_length (input)))) (PreH4 : (0 <= i)) (PreH5 : (i <= n)) (PreH6 : (0 <= k)) (PreH7 : (0 <= spacelen)) (PreH8 : ((k + spacelen ) <= i)) (PreH9 : (k = (Zlength (output_2)))) (PreH10 : (fix_spaces_state_z_140 input output_2 i spacelen )) (PreH11 : (valid_string input )) (PreH12 : (problem_140_pre_z input )) (PreH13 : (ascii_range_z input )) (PreH14 : ((string_length (input)) < INT_MAX)) ,
+  (store_string text_pre input )
+  **  (CharArray.full out k output_2 )
+  **  (CharArray.undef_seg out k (n + 1 ) )
+|--
+  EX (output: (@list Z)) ,
+  “ (n = (string_length (input))) ” 
+  &&  “ (0 <= i) ” 
+  &&  “ (i < n) ” 
+  &&  “ (0 <= k) ” 
+  &&  “ (0 <= (spacelen + 1 )) ” 
+  &&  “ ((k + (spacelen + 1 ) ) <= (i + 1 )) ” 
+  &&  “ (k = (Zlength (output))) ” 
+  &&  “ (fix_spaces_state_z_140 input output (i + 1 ) (spacelen + 1 ) ) ” 
+  &&  “ (valid_string input ) ” 
+  &&  “ (problem_140_pre_z input ) ” 
+  &&  “ (ascii_range_z input ) ” 
+  &&  “ ((string_length (input)) < INT_MAX) ”
+  &&  (store_string text_pre input )
+  **  (CharArray.full out k output )
+  **  (CharArray.undef_seg out k (n + 1 ) )
+) \/
+(
+forall (input: (@list Z)) (output_2: (@list Z)) (spacelen: Z) (k: Z) (i: Z) (n: Z) (PreH1 : (0 <= ((string_length (input)) + 1 ))) (PreH2 : ((Znth i (c_string (input)) 0) = 32)) (PreH3 : (i < n)) (PreH4 : (n = (string_length (input)))) (PreH5 : (0 <= i)) (PreH6 : (i <= n)) (PreH7 : (0 <= k)) (PreH8 : (0 <= spacelen)) (PreH9 : ((k + spacelen ) <= i)) (PreH10 : (k = (Zlength (output_2)))) (PreH11 : (fix_spaces_state_z_140 input output_2 i spacelen )) (PreH12 : (valid_string input )) (PreH13 : (problem_140_pre_z input )) (PreH14 : (ascii_range_z input )) (PreH15 : ((string_length (input)) < INT_MAX)) ,
+  TT && emp 
+|--
+  “ (fix_spaces_state_z_140 input output_2 (i + 1 ) (spacelen + 1 ) ) ”
+  &&  emp
+).
+
+Definition fix_spaces_entail_wit_2_5_split_goal_1 := 
+forall (input: (@list Z)) (output_2: (@list Z)) (spacelen: Z) (k: Z) (i: Z) (n: Z) (PreH1 : (0 <= ((string_length (input)) + 1 ))) (PreH2 : ((Znth i (c_string (input)) 0) = 32)) (PreH3 : (i < n)) (PreH4 : (n = (string_length (input)))) (PreH5 : (0 <= i)) (PreH6 : (i <= n)) (PreH7 : (0 <= k)) (PreH8 : (0 <= spacelen)) (PreH9 : ((k + spacelen ) <= i)) (PreH10 : (k = (Zlength (output_2)))) (PreH11 : (fix_spaces_state_z_140 input output_2 i spacelen )) (PreH12 : (valid_string input )) (PreH13 : (problem_140_pre_z input )) (PreH14 : (ascii_range_z input )) (PreH15 : ((string_length (input)) < INT_MAX)) ,
+  TT && emp 
+|--
+  “ (fix_spaces_state_z_140 input output_2 (i + 1 ) (spacelen + 1 ) ) ”
+.
+
+Definition fix_spaces_entail_wit_3 := 
+forall (text_pre: Z) (input: (@list Z)) (output_2: (@list Z)) (n: Z) (i: Z) (k: Z) (spacelen: Z) (out: Z) (PreH1 : (n = (string_length (input)))) (PreH2 : (0 <= i)) (PreH3 : (i < n)) (PreH4 : (0 <= k)) (PreH5 : (0 <= spacelen)) (PreH6 : ((k + spacelen ) <= (i + 1 ))) (PreH7 : (k = (Zlength (output_2)))) (PreH8 : (fix_spaces_state_z_140 input output_2 (i + 1 ) spacelen )) (PreH9 : (valid_string input )) (PreH10 : (problem_140_pre_z input )) (PreH11 : (ascii_range_z input )) (PreH12 : ((string_length (input)) < INT_MAX)) ,
+  (store_string text_pre input )
+  **  (CharArray.full out k output_2 )
+  **  (CharArray.undef_seg out k (n + 1 ) )
+|--
+  EX (output: (@list Z)) ,
+  “ (n = (string_length (input))) ” 
+  &&  “ (0 <= (i + 1 )) ” 
+  &&  “ ((i + 1 ) <= n) ” 
+  &&  “ (0 <= k) ” 
+  &&  “ (0 <= spacelen) ” 
+  &&  “ ((k + spacelen ) <= (i + 1 )) ” 
+  &&  “ (k = (Zlength (output))) ” 
+  &&  “ (fix_spaces_state_z_140 input output (i + 1 ) spacelen ) ” 
+  &&  “ (valid_string input ) ” 
+  &&  “ (problem_140_pre_z input ) ” 
+  &&  “ (ascii_range_z input ) ” 
+  &&  “ ((string_length (input)) < INT_MAX) ”
+  &&  (store_string text_pre input )
+  **  (CharArray.full out k output )
+  **  (CharArray.undef_seg out k (n + 1 ) )
+.
+
+Definition fix_spaces_entail_wit_4_1 := 
+(
+forall (text_pre: Z) (input: (@list Z)) (out: Z) (output_2: (@list Z)) (spacelen: Z) (k: Z) (i: Z) (n: Z) (PreH1 : (spacelen <= 2)) (PreH2 : (spacelen <> 2)) (PreH3 : (spacelen <> 1)) (PreH4 : (i >= n)) (PreH5 : (n = (string_length (input)))) (PreH6 : (0 <= i)) (PreH7 : (i <= n)) (PreH8 : (0 <= k)) (PreH9 : (0 <= spacelen)) (PreH10 : ((k + spacelen ) <= i)) (PreH11 : (k = (Zlength (output_2)))) (PreH12 : (fix_spaces_state_z_140 input output_2 i spacelen )) (PreH13 : (valid_string input )) (PreH14 : (problem_140_pre_z input )) (PreH15 : (ascii_range_z input )) (PreH16 : ((string_length (input)) < INT_MAX)) ,
+  (store_string text_pre input )
+  **  (CharArray.full out k output_2 )
+  **  (CharArray.undef_seg out k (n + 1 ) )
+|--
+  EX (prefix: (@list Z))  (output: (@list Z)) ,
+  “ (n = (string_length (input))) ” 
+  &&  “ (0 <= k) ” 
+  &&  “ (0 <= spacelen) ” 
+  &&  “ (k <= n) ” 
+  &&  “ (k = (Zlength (output))) ” 
+  &&  “ (output = (app (prefix) ((flush_spaces_z_140 (spacelen))))) ” 
+  &&  “ (fix_spaces_state_z_140 input prefix n spacelen ) ” 
+  &&  “ (valid_string input ) ” 
+  &&  “ (problem_140_pre_z input ) ” 
+  &&  “ (ascii_range_z input ) ” 
+  &&  “ ((string_length (input)) < INT_MAX) ”
+  &&  (store_string text_pre input )
+  **  (CharArray.full out k output )
+  **  (CharArray.undef_seg out k (n + 1 ) )
+) \/
+(
+forall (input: (@list Z)) (output_2: (@list Z)) (spacelen: Z) (k: Z) (i: Z) (n: Z) (PreH1 : (0 <= ((string_length (input)) + 1 ))) (PreH2 : (spacelen <= 2)) (PreH3 : (spacelen <> 2)) (PreH4 : (spacelen <> 1)) (PreH5 : (i >= n)) (PreH6 : (n = (string_length (input)))) (PreH7 : (0 <= i)) (PreH8 : (i <= n)) (PreH9 : (0 <= k)) (PreH10 : (0 <= spacelen)) (PreH11 : ((k + spacelen ) <= i)) (PreH12 : (k = (Zlength (output_2)))) (PreH13 : (fix_spaces_state_z_140 input output_2 i spacelen )) (PreH14 : (valid_string input )) (PreH15 : (problem_140_pre_z input )) (PreH16 : (ascii_range_z input )) (PreH17 : ((string_length (input)) < INT_MAX)) ,
+  TT && emp 
+|--
+  EX (prefix: (@list Z)) ,
+  “ (output_2 = (app (prefix) ((flush_spaces_z_140 (spacelen))))) ” 
+  &&  “ (n = (string_length (input))) ” 
+  &&  “ (0 <= k) ” 
+  &&  “ (0 <= spacelen) ” 
+  &&  “ (k <= n) ” 
+  &&  “ (k = (Zlength ((app (prefix) ((flush_spaces_z_140 (spacelen))))))) ” 
+  &&  “ (fix_spaces_state_z_140 input prefix n spacelen ) ” 
+  &&  “ (valid_string input ) ” 
+  &&  “ (problem_140_pre_z input ) ” 
+  &&  “ (ascii_range_z input ) ” 
+  &&  “ ((string_length (input)) < INT_MAX) ”
+  &&  emp
+).
+
+Definition fix_spaces_entail_wit_4_2 := 
+(
+forall (text_pre: Z) (input: (@list Z)) (out: Z) (output_2: (@list Z)) (spacelen: Z) (k: Z) (i: Z) (n: Z) (PreH1 : (spacelen <= 2)) (PreH2 : (spacelen <> 2)) (PreH3 : (0 <= ((string_length (input)) + 1 ))) (PreH4 : (spacelen = 1)) (PreH5 : (i >= n)) (PreH6 : (n = (string_length (input)))) (PreH7 : (0 <= i)) (PreH8 : (i <= n)) (PreH9 : (0 <= k)) (PreH10 : (0 <= spacelen)) (PreH11 : ((k + spacelen ) <= i)) (PreH12 : (k = (Zlength (output_2)))) (PreH13 : (fix_spaces_state_z_140 input output_2 i spacelen )) (PreH14 : (valid_string input )) (PreH15 : (problem_140_pre_z input )) (PreH16 : (ascii_range_z input )) (PreH17 : ((string_length (input)) < INT_MAX)) ,
+  (CharArray.full out (k + 1 ) (app (output_2) ((cons (95) ((@nil Z))))) )
+  **  (CharArray.undef_seg out (k + 1 ) (n + 1 ) )
+  **  (CharArray.full text_pre ((string_length (input)) + 1 ) (c_string (input)) )
+|--
+  EX (prefix: (@list Z))  (output: (@list Z)) ,
+  “ (n = (string_length (input))) ” 
+  &&  “ (0 <= (k + 1 )) ” 
+  &&  “ (0 <= spacelen) ” 
+  &&  “ ((k + 1 ) <= n) ” 
+  &&  “ ((k + 1 ) = (Zlength (output))) ” 
+  &&  “ (output = (app (prefix) ((flush_spaces_z_140 (spacelen))))) ” 
+  &&  “ (fix_spaces_state_z_140 input prefix n spacelen ) ” 
+  &&  “ (valid_string input ) ” 
+  &&  “ (problem_140_pre_z input ) ” 
+  &&  “ (ascii_range_z input ) ” 
+  &&  “ ((string_length (input)) < INT_MAX) ”
+  &&  (store_string text_pre input )
+  **  (CharArray.full out (k + 1 ) output )
+  **  (CharArray.undef_seg out (k + 1 ) (n + 1 ) )
+) \/
+(
+forall (input: (@list Z)) (output_2: (@list Z)) (spacelen: Z) (k: Z) (i: Z) (n: Z) (PreH1 : (spacelen <= 2)) (PreH2 : (spacelen <> 2)) (PreH3 : (0 <= ((string_length (input)) + 1 ))) (PreH4 : (spacelen = 1)) (PreH5 : (i >= n)) (PreH6 : (n = (string_length (input)))) (PreH7 : (0 <= i)) (PreH8 : (i <= n)) (PreH9 : (0 <= k)) (PreH10 : (0 <= spacelen)) (PreH11 : ((k + spacelen ) <= i)) (PreH12 : (k = (Zlength (output_2)))) (PreH13 : (fix_spaces_state_z_140 input output_2 i spacelen )) (PreH14 : (valid_string input )) (PreH15 : (problem_140_pre_z input )) (PreH16 : (ascii_range_z input )) (PreH17 : ((string_length (input)) < INT_MAX)) ,
+  TT && emp 
+|--
+  EX (prefix: (@list Z)) ,
+  “ ((app (output_2) ((cons (95) ((@nil Z))))) = (app (prefix) ((flush_spaces_z_140 (spacelen))))) ” 
+  &&  “ (n = (string_length (input))) ” 
+  &&  “ (0 <= (k + 1 )) ” 
+  &&  “ (0 <= spacelen) ” 
+  &&  “ ((k + 1 ) <= n) ” 
+  &&  “ ((k + 1 ) = (Zlength ((app (prefix) ((flush_spaces_z_140 (spacelen))))))) ” 
+  &&  “ (fix_spaces_state_z_140 input prefix n spacelen ) ” 
+  &&  “ (valid_string input ) ” 
+  &&  “ (problem_140_pre_z input ) ” 
+  &&  “ (ascii_range_z input ) ” 
+  &&  “ ((string_length (input)) < INT_MAX) ”
+  &&  emp
+).
+
+Definition fix_spaces_entail_wit_4_3 := 
+(
+forall (text_pre: Z) (input: (@list Z)) (out: Z) (output_2: (@list Z)) (spacelen: Z) (k: Z) (i: Z) (n: Z) (PreH1 : (spacelen <= 2)) (PreH2 : (0 <= (k + 1 ))) (PreH3 : (0 <= ((string_length (input)) + 1 ))) (PreH4 : (spacelen = 2)) (PreH5 : (spacelen <> 1)) (PreH6 : (i >= n)) (PreH7 : (n = (string_length (input)))) (PreH8 : (0 <= i)) (PreH9 : (i <= n)) (PreH10 : (0 <= k)) (PreH11 : (0 <= spacelen)) (PreH12 : ((k + spacelen ) <= i)) (PreH13 : (k = (Zlength (output_2)))) (PreH14 : (fix_spaces_state_z_140 input output_2 i spacelen )) (PreH15 : (valid_string input )) (PreH16 : (problem_140_pre_z input )) (PreH17 : (ascii_range_z input )) (PreH18 : ((string_length (input)) < INT_MAX)) ,
+  (CharArray.full out ((k + 1 ) + 1 ) (app ((app (output_2) ((cons (95) ((@nil Z)))))) ((cons (95) ((@nil Z))))) )
+  **  (CharArray.undef_seg out ((k + 1 ) + 1 ) (n + 1 ) )
+  **  (CharArray.full text_pre ((string_length (input)) + 1 ) (c_string (input)) )
+|--
+  EX (prefix: (@list Z))  (output: (@list Z)) ,
+  “ (n = (string_length (input))) ” 
+  &&  “ (0 <= ((k + 1 ) + 1 )) ” 
+  &&  “ (0 <= spacelen) ” 
+  &&  “ (((k + 1 ) + 1 ) <= n) ” 
+  &&  “ (((k + 1 ) + 1 ) = (Zlength (output))) ” 
+  &&  “ (output = (app (prefix) ((flush_spaces_z_140 (spacelen))))) ” 
+  &&  “ (fix_spaces_state_z_140 input prefix n spacelen ) ” 
+  &&  “ (valid_string input ) ” 
+  &&  “ (problem_140_pre_z input ) ” 
+  &&  “ (ascii_range_z input ) ” 
+  &&  “ ((string_length (input)) < INT_MAX) ”
+  &&  (store_string text_pre input )
+  **  (CharArray.full out ((k + 1 ) + 1 ) output )
+  **  (CharArray.undef_seg out ((k + 1 ) + 1 ) (n + 1 ) )
+) \/
+(
+forall (input: (@list Z)) (output_2: (@list Z)) (spacelen: Z) (k: Z) (i: Z) (n: Z) (PreH1 : (spacelen <= 2)) (PreH2 : (0 <= (k + 1 ))) (PreH3 : (0 <= ((string_length (input)) + 1 ))) (PreH4 : (spacelen = 2)) (PreH5 : (spacelen <> 1)) (PreH6 : (i >= n)) (PreH7 : (n = (string_length (input)))) (PreH8 : (0 <= i)) (PreH9 : (i <= n)) (PreH10 : (0 <= k)) (PreH11 : (0 <= spacelen)) (PreH12 : ((k + spacelen ) <= i)) (PreH13 : (k = (Zlength (output_2)))) (PreH14 : (fix_spaces_state_z_140 input output_2 i spacelen )) (PreH15 : (valid_string input )) (PreH16 : (problem_140_pre_z input )) (PreH17 : (ascii_range_z input )) (PreH18 : ((string_length (input)) < INT_MAX)) ,
+  TT && emp 
+|--
+  EX (prefix: (@list Z)) ,
+  “ ((app ((app (output_2) ((cons (95) ((@nil Z)))))) ((cons (95) ((@nil Z))))) = (app (prefix) ((flush_spaces_z_140 (spacelen))))) ” 
+  &&  “ (n = (string_length (input))) ” 
+  &&  “ (0 <= ((k + 1 ) + 1 )) ” 
+  &&  “ (0 <= spacelen) ” 
+  &&  “ (((k + 1 ) + 1 ) <= n) ” 
+  &&  “ (((k + 1 ) + 1 ) = (Zlength ((app (prefix) ((flush_spaces_z_140 (spacelen))))))) ” 
+  &&  “ (fix_spaces_state_z_140 input prefix n spacelen ) ” 
+  &&  “ (valid_string input ) ” 
+  &&  “ (problem_140_pre_z input ) ” 
+  &&  “ (ascii_range_z input ) ” 
+  &&  “ ((string_length (input)) < INT_MAX) ”
+  &&  emp
+).
+
+Definition fix_spaces_entail_wit_4_4 := 
+(
+forall (text_pre: Z) (input: (@list Z)) (out: Z) (output_2: (@list Z)) (spacelen: Z) (k: Z) (i: Z) (n: Z) (PreH1 : (0 <= ((string_length (input)) + 1 ))) (PreH2 : (spacelen > 2)) (PreH3 : (spacelen <> 2)) (PreH4 : (spacelen <> 1)) (PreH5 : (i >= n)) (PreH6 : (n = (string_length (input)))) (PreH7 : (0 <= i)) (PreH8 : (i <= n)) (PreH9 : (0 <= k)) (PreH10 : (0 <= spacelen)) (PreH11 : ((k + spacelen ) <= i)) (PreH12 : (k = (Zlength (output_2)))) (PreH13 : (fix_spaces_state_z_140 input output_2 i spacelen )) (PreH14 : (valid_string input )) (PreH15 : (problem_140_pre_z input )) (PreH16 : (ascii_range_z input )) (PreH17 : ((string_length (input)) < INT_MAX)) ,
+  (CharArray.full out (k + 1 ) (app (output_2) ((cons (45) ((@nil Z))))) )
+  **  (CharArray.undef_seg out (k + 1 ) (n + 1 ) )
+  **  (CharArray.full text_pre ((string_length (input)) + 1 ) (c_string (input)) )
+|--
+  EX (prefix: (@list Z))  (output: (@list Z)) ,
+  “ (n = (string_length (input))) ” 
+  &&  “ (0 <= (k + 1 )) ” 
+  &&  “ (0 <= spacelen) ” 
+  &&  “ ((k + 1 ) <= n) ” 
+  &&  “ ((k + 1 ) = (Zlength (output))) ” 
+  &&  “ (output = (app (prefix) ((flush_spaces_z_140 (spacelen))))) ” 
+  &&  “ (fix_spaces_state_z_140 input prefix n spacelen ) ” 
+  &&  “ (valid_string input ) ” 
+  &&  “ (problem_140_pre_z input ) ” 
+  &&  “ (ascii_range_z input ) ” 
+  &&  “ ((string_length (input)) < INT_MAX) ”
+  &&  (store_string text_pre input )
+  **  (CharArray.full out (k + 1 ) output )
+  **  (CharArray.undef_seg out (k + 1 ) (n + 1 ) )
+) \/
+(
+forall (input: (@list Z)) (output_2: (@list Z)) (spacelen: Z) (k: Z) (i: Z) (n: Z) (PreH1 : (0 <= ((string_length (input)) + 1 ))) (PreH2 : (spacelen > 2)) (PreH3 : (spacelen <> 2)) (PreH4 : (spacelen <> 1)) (PreH5 : (i >= n)) (PreH6 : (n = (string_length (input)))) (PreH7 : (0 <= i)) (PreH8 : (i <= n)) (PreH9 : (0 <= k)) (PreH10 : (0 <= spacelen)) (PreH11 : ((k + spacelen ) <= i)) (PreH12 : (k = (Zlength (output_2)))) (PreH13 : (fix_spaces_state_z_140 input output_2 i spacelen )) (PreH14 : (valid_string input )) (PreH15 : (problem_140_pre_z input )) (PreH16 : (ascii_range_z input )) (PreH17 : ((string_length (input)) < INT_MAX)) ,
+  TT && emp 
+|--
+  EX (prefix: (@list Z)) ,
+  “ ((app (output_2) ((cons (45) ((@nil Z))))) = (app (prefix) ((flush_spaces_z_140 (spacelen))))) ” 
+  &&  “ (n = (string_length (input))) ” 
+  &&  “ (0 <= (k + 1 )) ” 
+  &&  “ (0 <= spacelen) ” 
+  &&  “ ((k + 1 ) <= n) ” 
+  &&  “ ((k + 1 ) = (Zlength ((app (prefix) ((flush_spaces_z_140 (spacelen))))))) ” 
+  &&  “ (fix_spaces_state_z_140 input prefix n spacelen ) ” 
+  &&  “ (valid_string input ) ” 
+  &&  “ (problem_140_pre_z input ) ” 
+  &&  “ (ascii_range_z input ) ” 
+  &&  “ ((string_length (input)) < INT_MAX) ”
+  &&  emp
+).
+
+Definition fix_spaces_return_wit_1 := 
+(
+forall (text_pre: Z) (input: (@list Z)) (prefix: (@list Z)) (output_2: (@list Z)) (n: Z) (k: Z) (spacelen: Z) (out: Z) (PreH1 : (0 <= ((string_length (input)) + 1 ))) (PreH2 : (n = (string_length (input)))) (PreH3 : (0 <= k)) (PreH4 : (0 <= spacelen)) (PreH5 : (k <= n)) (PreH6 : (k = (Zlength (output_2)))) (PreH7 : (output_2 = (app (prefix) ((flush_spaces_z_140 (spacelen)))))) (PreH8 : (fix_spaces_state_z_140 input prefix n spacelen )) (PreH9 : (valid_string input )) (PreH10 : (problem_140_pre_z input )) (PreH11 : (ascii_range_z input )) (PreH12 : ((string_length (input)) < INT_MAX)) ,
+  (CharArray.full out (k + 1 ) (app (output_2) ((cons (0) ((@nil Z))))) )
+  **  (CharArray.undef_seg out (k + 1 ) (n + 1 ) )
+  **  (CharArray.full text_pre ((string_length (input)) + 1 ) (c_string (input)) )
+|--
+  EX (output: (@list Z)) ,
+  “ (problem_140_spec_z input output ) ”
+  &&  (store_string text_pre input )
+  **  (store_string out output )
+  **  (CharArray.undef_seg out ((string_length (output)) + 1 ) ((string_length (input)) + 1 ) )
+) \/
+(
+forall (input: (@list Z)) (prefix: (@list Z)) (output_2: (@list Z)) (n: Z) (k: Z) (spacelen: Z) (out: Z) (PreH1 : (0 <= (k + 1 ))) (PreH2 : (0 <= ((string_length (input)) + 1 ))) (PreH3 : (n = (string_length (input)))) (PreH4 : (0 <= k)) (PreH5 : (0 <= spacelen)) (PreH6 : (k <= n)) (PreH7 : (k = (Zlength (output_2)))) (PreH8 : (output_2 = (app (prefix) ((flush_spaces_z_140 (spacelen)))))) (PreH9 : (fix_spaces_state_z_140 input prefix n spacelen )) (PreH10 : (valid_string input )) (PreH11 : (problem_140_pre_z input )) (PreH12 : (ascii_range_z input )) (PreH13 : ((string_length (input)) < INT_MAX)) ,
+  (CharArray.full out (k + 1 ) (app (output_2) ((cons (0) ((@nil Z))))) )
+  **  (CharArray.undef_seg out (k + 1 ) (n + 1 ) )
+|--
+  EX (output: (@list Z)) ,
+  “ (problem_140_spec_z input output ) ”
+  &&  (CharArray.full out ((string_length (output)) + 1 ) (c_string (output)) )
+  **  (CharArray.undef_seg out ((string_length (output)) + 1 ) ((string_length (input)) + 1 ) )
+).
+
+Definition fix_spaces_partial_solve_wit_1_pure := 
+forall (text_pre: Z) (input: (@list Z)) (PreH1 : (valid_string input )) (PreH2 : (problem_140_pre_z input )) (PreH3 : (ascii_range_z input )) (PreH4 : ((string_length (input)) < INT_MAX)) ,
+  ((( &( "n" ) )) # Int  |->_)
+  **  ((( &( "text" ) )) # Ptr  |-> text_pre)
+  **  (store_string text_pre input )
+|--
+  “ (valid_string input ) ” 
+  &&  “ ((string_length (input)) < INT_MAX) ”
+.
+
+Definition fix_spaces_partial_solve_wit_1_aux := 
+forall (text_pre: Z) (input: (@list Z)) (PreH1 : (valid_string input )) (PreH2 : (problem_140_pre_z input )) (PreH3 : (ascii_range_z input )) (PreH4 : ((string_length (input)) < INT_MAX)) ,
+  (store_string text_pre input )
+|--
+  “ (valid_string input ) ” 
+  &&  “ ((string_length (input)) < INT_MAX) ” 
+  &&  “ (0 <= ((string_length (input)) + 1 )) ” 
+  &&  “ (valid_string input ) ” 
+  &&  “ (problem_140_pre_z input ) ” 
+  &&  “ (ascii_range_z input ) ” 
+  &&  “ ((string_length (input)) < INT_MAX) ”
+  &&  (store_string text_pre input )
+.
+
+Definition fix_spaces_partial_solve_wit_1 := fix_spaces_partial_solve_wit_1_pure -> fix_spaces_partial_solve_wit_1_aux.
+
+Definition fix_spaces_partial_solve_wit_2_pure := 
+(
+forall (text_pre: Z) (input: (@list Z)) (retval: Z) (PreH1 : (retval = (string_length (input)))) (PreH2 : (0 <= ((string_length (input)) + 1 ))) (PreH3 : (valid_string input )) (PreH4 : (problem_140_pre_z input )) (PreH5 : (ascii_range_z input )) (PreH6 : ((string_length (input)) < INT_MAX)) ,
+  ((( &( "out" ) )) # Ptr  |->_)
+  **  (store_string text_pre input )
+  **  ((( &( "n" ) )) # Int  |-> retval)
+  **  ((( &( "text" ) )) # Ptr  |-> text_pre)
+|--
+  “ ((retval + 1 ) <= INT_MAX) ” 
+  &&  “ ((retval + 1 ) > 0) ”
+) \/
+(
+forall (text_pre: Z) (input: (@list Z)) (retval: Z) (PreH1 : (retval <= INT_MAX)) (PreH2 : (retval >= INT_MIN)) (PreH3 : (retval = (string_length (input)))) (PreH4 : (0 <= ((string_length (input)) + 1 ))) (PreH5 : (valid_string input )) (PreH6 : (problem_140_pre_z input )) (PreH7 : (ascii_range_z input )) (PreH8 : ((string_length (input)) < INT_MAX)) ,
+  (CharArray.full text_pre ((string_length (input)) + 1 ) (c_string (input)) )
+  **  ((( &( "out" ) )) # Ptr  |->_)
+  **  ((( &( "n" ) )) # Int  |-> retval)
+  **  ((( &( "text" ) )) # Ptr  |-> text_pre)
+|--
+  “ ((retval + 1 ) > 0) ”
+).
+
+Definition fix_spaces_partial_solve_wit_2_pure_split_goal_1 := 
+forall (text_pre: Z) (input: (@list Z)) (retval: Z) (PreH1 : (retval <= INT_MAX)) (PreH2 : (retval >= INT_MIN)) (PreH3 : (retval = (string_length (input)))) (PreH4 : (0 <= ((string_length (input)) + 1 ))) (PreH5 : (valid_string input )) (PreH6 : (problem_140_pre_z input )) (PreH7 : (ascii_range_z input )) (PreH8 : ((string_length (input)) < INT_MAX)) ,
+  (CharArray.full text_pre ((string_length (input)) + 1 ) (c_string (input)) )
+  **  ((( &( "out" ) )) # Ptr  |->_)
+  **  ((( &( "n" ) )) # Int  |-> retval)
+  **  ((( &( "text" ) )) # Ptr  |-> text_pre)
+|--
+  “ ((retval + 1 ) > 0) ”
+.
+
+Definition fix_spaces_partial_solve_wit_2_aux := 
+forall (text_pre: Z) (input: (@list Z)) (retval: Z) (PreH1 : (retval = (string_length (input)))) (PreH2 : (0 <= ((string_length (input)) + 1 ))) (PreH3 : (valid_string input )) (PreH4 : (problem_140_pre_z input )) (PreH5 : (ascii_range_z input )) (PreH6 : ((string_length (input)) < INT_MAX)) ,
+  (store_string text_pre input )
+|--
+  “ ((retval + 1 ) <= INT_MAX) ” 
+  &&  “ ((retval + 1 ) > 0) ” 
+  &&  “ (retval = (string_length (input))) ” 
+  &&  “ (0 <= ((string_length (input)) + 1 )) ” 
+  &&  “ (valid_string input ) ” 
+  &&  “ (problem_140_pre_z input ) ” 
+  &&  “ (ascii_range_z input ) ” 
+  &&  “ ((string_length (input)) < INT_MAX) ”
+  &&  (CharArray.full text_pre ((string_length (input)) + 1 ) (c_string (input)) )
+.
+
+Definition fix_spaces_partial_solve_wit_2 := fix_spaces_partial_solve_wit_2_pure -> fix_spaces_partial_solve_wit_2_aux.
+
+Definition fix_spaces_partial_solve_wit_3 := 
+forall (text_pre: Z) (input: (@list Z)) (out: Z) (output: (@list Z)) (spacelen: Z) (k: Z) (i: Z) (n: Z) (PreH1 : (spacelen = 1)) (PreH2 : ((Znth i (c_string (input)) 0) <> 32)) (PreH3 : (i < n)) (PreH4 : (n = (string_length (input)))) (PreH5 : (0 <= i)) (PreH6 : (i <= n)) (PreH7 : (0 <= k)) (PreH8 : (0 <= spacelen)) (PreH9 : ((k + spacelen ) <= i)) (PreH10 : (k = (Zlength (output)))) (PreH11 : (fix_spaces_state_z_140 input output i spacelen )) (PreH12 : (valid_string input )) (PreH13 : (problem_140_pre_z input )) (PreH14 : (ascii_range_z input )) (PreH15 : ((string_length (input)) < INT_MAX)) ,
+  (store_string text_pre input )
+  **  (CharArray.full out k output )
+  **  (CharArray.undef_seg out k (n + 1 ) )
+|--
+  “ (0 <= ((string_length (input)) + 1 )) ” 
+  &&  “ (spacelen = 1) ” 
+  &&  “ ((Znth i (c_string (input)) 0) <> 32) ” 
+  &&  “ (i < n) ” 
+  &&  “ (n = (string_length (input))) ” 
+  &&  “ (0 <= i) ” 
+  &&  “ (i <= n) ” 
+  &&  “ (0 <= k) ” 
+  &&  “ (0 <= spacelen) ” 
+  &&  “ ((k + spacelen ) <= i) ” 
+  &&  “ (k = (Zlength (output))) ” 
+  &&  “ (fix_spaces_state_z_140 input output i spacelen ) ” 
+  &&  “ (valid_string input ) ” 
+  &&  “ (problem_140_pre_z input ) ” 
+  &&  “ (ascii_range_z input ) ” 
+  &&  “ ((string_length (input)) < INT_MAX) ”
+  &&  (((out + (k * sizeof(CHAR) ) )) # Char  |->_)
+  **  (CharArray.full text_pre ((string_length (input)) + 1 ) (c_string (input)) )
+  **  (CharArray.undef_missing_i out k k (n + 1 ) )
+  **  (CharArray.full out k output )
+.
+
+Definition fix_spaces_partial_solve_wit_4 := 
+forall (text_pre: Z) (input: (@list Z)) (out: Z) (output: (@list Z)) (spacelen: Z) (k: Z) (i: Z) (n: Z) (PreH1 : (spacelen = 2)) (PreH2 : (spacelen <> 1)) (PreH3 : ((Znth i (c_string (input)) 0) <> 32)) (PreH4 : (i < n)) (PreH5 : (n = (string_length (input)))) (PreH6 : (0 <= i)) (PreH7 : (i <= n)) (PreH8 : (0 <= k)) (PreH9 : (0 <= spacelen)) (PreH10 : ((k + spacelen ) <= i)) (PreH11 : (k = (Zlength (output)))) (PreH12 : (fix_spaces_state_z_140 input output i spacelen )) (PreH13 : (valid_string input )) (PreH14 : (problem_140_pre_z input )) (PreH15 : (ascii_range_z input )) (PreH16 : ((string_length (input)) < INT_MAX)) ,
+  (store_string text_pre input )
+  **  (CharArray.full out k output )
+  **  (CharArray.undef_seg out k (n + 1 ) )
+|--
+  “ (0 <= ((string_length (input)) + 1 )) ” 
+  &&  “ (spacelen = 2) ” 
+  &&  “ (spacelen <> 1) ” 
+  &&  “ ((Znth i (c_string (input)) 0) <> 32) ” 
+  &&  “ (i < n) ” 
+  &&  “ (n = (string_length (input))) ” 
+  &&  “ (0 <= i) ” 
+  &&  “ (i <= n) ” 
+  &&  “ (0 <= k) ” 
+  &&  “ (0 <= spacelen) ” 
+  &&  “ ((k + spacelen ) <= i) ” 
+  &&  “ (k = (Zlength (output))) ” 
+  &&  “ (fix_spaces_state_z_140 input output i spacelen ) ” 
+  &&  “ (valid_string input ) ” 
+  &&  “ (problem_140_pre_z input ) ” 
+  &&  “ (ascii_range_z input ) ” 
+  &&  “ ((string_length (input)) < INT_MAX) ”
+  &&  (((out + (k * sizeof(CHAR) ) )) # Char  |->_)
+  **  (CharArray.full text_pre ((string_length (input)) + 1 ) (c_string (input)) )
+  **  (CharArray.undef_missing_i out k k (n + 1 ) )
+  **  (CharArray.full out k output )
+.
+
+Definition fix_spaces_partial_solve_wit_5 := 
+forall (text_pre: Z) (input: (@list Z)) (out: Z) (output: (@list Z)) (spacelen: Z) (k: Z) (i: Z) (n: Z) (PreH1 : (0 <= ((string_length (input)) + 1 ))) (PreH2 : (spacelen = 2)) (PreH3 : (spacelen <> 1)) (PreH4 : ((Znth i (c_string (input)) 0) <> 32)) (PreH5 : (i < n)) (PreH6 : (n = (string_length (input)))) (PreH7 : (0 <= i)) (PreH8 : (i <= n)) (PreH9 : (0 <= k)) (PreH10 : (0 <= spacelen)) (PreH11 : ((k + spacelen ) <= i)) (PreH12 : (k = (Zlength (output)))) (PreH13 : (fix_spaces_state_z_140 input output i spacelen )) (PreH14 : (valid_string input )) (PreH15 : (problem_140_pre_z input )) (PreH16 : (ascii_range_z input )) (PreH17 : ((string_length (input)) < INT_MAX)) ,
+  (CharArray.full out (k + 1 ) (app (output) ((cons (95) ((@nil Z))))) )
+  **  (CharArray.undef_seg out (k + 1 ) (n + 1 ) )
+  **  (CharArray.full text_pre ((string_length (input)) + 1 ) (c_string (input)) )
+|--
+  “ (0 <= (k + 1 )) ” 
+  &&  “ (0 <= ((string_length (input)) + 1 )) ” 
+  &&  “ (spacelen = 2) ” 
+  &&  “ (spacelen <> 1) ” 
+  &&  “ ((Znth i (c_string (input)) 0) <> 32) ” 
+  &&  “ (i < n) ” 
+  &&  “ (n = (string_length (input))) ” 
+  &&  “ (0 <= i) ” 
+  &&  “ (i <= n) ” 
+  &&  “ (0 <= k) ” 
+  &&  “ (0 <= spacelen) ” 
+  &&  “ ((k + spacelen ) <= i) ” 
+  &&  “ (k = (Zlength (output))) ” 
+  &&  “ (fix_spaces_state_z_140 input output i spacelen ) ” 
+  &&  “ (valid_string input ) ” 
+  &&  “ (problem_140_pre_z input ) ” 
+  &&  “ (ascii_range_z input ) ” 
+  &&  “ ((string_length (input)) < INT_MAX) ”
+  &&  (((out + ((k + 1 ) * sizeof(CHAR) ) )) # Char  |->_)
+  **  (CharArray.undef_missing_i out (k + 1 ) (k + 1 ) (n + 1 ) )
+  **  (CharArray.full out (k + 1 ) (app (output) ((cons (95) ((@nil Z))))) )
+  **  (CharArray.full text_pre ((string_length (input)) + 1 ) (c_string (input)) )
+.
+
+Definition fix_spaces_partial_solve_wit_6 := 
+forall (text_pre: Z) (input: (@list Z)) (out: Z) (output: (@list Z)) (spacelen: Z) (k: Z) (i: Z) (n: Z) (PreH1 : (spacelen > 2)) (PreH2 : (spacelen <> 2)) (PreH3 : (spacelen <> 1)) (PreH4 : ((Znth i (c_string (input)) 0) <> 32)) (PreH5 : (i < n)) (PreH6 : (n = (string_length (input)))) (PreH7 : (0 <= i)) (PreH8 : (i <= n)) (PreH9 : (0 <= k)) (PreH10 : (0 <= spacelen)) (PreH11 : ((k + spacelen ) <= i)) (PreH12 : (k = (Zlength (output)))) (PreH13 : (fix_spaces_state_z_140 input output i spacelen )) (PreH14 : (valid_string input )) (PreH15 : (problem_140_pre_z input )) (PreH16 : (ascii_range_z input )) (PreH17 : ((string_length (input)) < INT_MAX)) ,
+  (store_string text_pre input )
+  **  (CharArray.full out k output )
+  **  (CharArray.undef_seg out k (n + 1 ) )
+|--
+  “ (0 <= ((string_length (input)) + 1 )) ” 
+  &&  “ (spacelen > 2) ” 
+  &&  “ (spacelen <> 2) ” 
+  &&  “ (spacelen <> 1) ” 
+  &&  “ ((Znth i (c_string (input)) 0) <> 32) ” 
+  &&  “ (i < n) ” 
+  &&  “ (n = (string_length (input))) ” 
+  &&  “ (0 <= i) ” 
+  &&  “ (i <= n) ” 
+  &&  “ (0 <= k) ” 
+  &&  “ (0 <= spacelen) ” 
+  &&  “ ((k + spacelen ) <= i) ” 
+  &&  “ (k = (Zlength (output))) ” 
+  &&  “ (fix_spaces_state_z_140 input output i spacelen ) ” 
+  &&  “ (valid_string input ) ” 
+  &&  “ (problem_140_pre_z input ) ” 
+  &&  “ (ascii_range_z input ) ” 
+  &&  “ ((string_length (input)) < INT_MAX) ”
+  &&  (((out + (k * sizeof(CHAR) ) )) # Char  |->_)
+  **  (CharArray.full text_pre ((string_length (input)) + 1 ) (c_string (input)) )
+  **  (CharArray.undef_missing_i out k k (n + 1 ) )
+  **  (CharArray.full out k output )
+.
+
+Definition fix_spaces_partial_solve_wit_7 := 
+forall (text_pre: Z) (input: (@list Z)) (out: Z) (output: (@list Z)) (spacelen: Z) (k: Z) (i: Z) (n: Z) (PreH1 : (0 <= ((string_length (input)) + 1 ))) (PreH2 : (spacelen > 2)) (PreH3 : (spacelen <> 2)) (PreH4 : (spacelen <> 1)) (PreH5 : ((Znth i (c_string (input)) 0) <> 32)) (PreH6 : (i < n)) (PreH7 : (n = (string_length (input)))) (PreH8 : (0 <= i)) (PreH9 : (i <= n)) (PreH10 : (0 <= k)) (PreH11 : (0 <= spacelen)) (PreH12 : ((k + spacelen ) <= i)) (PreH13 : (k = (Zlength (output)))) (PreH14 : (fix_spaces_state_z_140 input output i spacelen )) (PreH15 : (valid_string input )) (PreH16 : (problem_140_pre_z input )) (PreH17 : (ascii_range_z input )) (PreH18 : ((string_length (input)) < INT_MAX)) ,
+  (CharArray.full out (k + 1 ) (app (output) ((cons (45) ((@nil Z))))) )
+  **  (CharArray.undef_seg out (k + 1 ) (n + 1 ) )
+  **  (CharArray.full text_pre ((string_length (input)) + 1 ) (c_string (input)) )
+|--
+  “ (0 <= (k + 1 )) ” 
+  &&  “ (0 <= ((string_length (input)) + 1 )) ” 
+  &&  “ (spacelen > 2) ” 
+  &&  “ (spacelen <> 2) ” 
+  &&  “ (spacelen <> 1) ” 
+  &&  “ ((Znth i (c_string (input)) 0) <> 32) ” 
+  &&  “ (i < n) ” 
+  &&  “ (n = (string_length (input))) ” 
+  &&  “ (0 <= i) ” 
+  &&  “ (i <= n) ” 
+  &&  “ (0 <= k) ” 
+  &&  “ (0 <= spacelen) ” 
+  &&  “ ((k + spacelen ) <= i) ” 
+  &&  “ (k = (Zlength (output))) ” 
+  &&  “ (fix_spaces_state_z_140 input output i spacelen ) ” 
+  &&  “ (valid_string input ) ” 
+  &&  “ (problem_140_pre_z input ) ” 
+  &&  “ (ascii_range_z input ) ” 
+  &&  “ ((string_length (input)) < INT_MAX) ”
+  &&  (((text_pre + (i * sizeof(CHAR) ) )) # Char  |-> (Znth i (c_string (input)) 0))
+  **  (CharArray.missing_i text_pre i 0 ((string_length (input)) + 1 ) (c_string (input)) )
+  **  (CharArray.full out (k + 1 ) (app (output) ((cons (45) ((@nil Z))))) )
+  **  (CharArray.undef_seg out (k + 1 ) (n + 1 ) )
+.
+
+Definition fix_spaces_partial_solve_wit_8 := 
+forall (text_pre: Z) (input: (@list Z)) (out: Z) (output: (@list Z)) (spacelen: Z) (k: Z) (i: Z) (n: Z) (PreH1 : (0 <= (k + 1 ))) (PreH2 : (0 <= ((string_length (input)) + 1 ))) (PreH3 : (spacelen > 2)) (PreH4 : (spacelen <> 2)) (PreH5 : (spacelen <> 1)) (PreH6 : ((Znth i (c_string (input)) 0) <> 32)) (PreH7 : (i < n)) (PreH8 : (n = (string_length (input)))) (PreH9 : (0 <= i)) (PreH10 : (i <= n)) (PreH11 : (0 <= k)) (PreH12 : (0 <= spacelen)) (PreH13 : ((k + spacelen ) <= i)) (PreH14 : (k = (Zlength (output)))) (PreH15 : (fix_spaces_state_z_140 input output i spacelen )) (PreH16 : (valid_string input )) (PreH17 : (problem_140_pre_z input )) (PreH18 : (ascii_range_z input )) (PreH19 : ((string_length (input)) < INT_MAX)) ,
+  (CharArray.full text_pre ((string_length (input)) + 1 ) (c_string (input)) )
+  **  (CharArray.full out (k + 1 ) (app (output) ((cons (45) ((@nil Z))))) )
+  **  (CharArray.undef_seg out (k + 1 ) (n + 1 ) )
+|--
+  “ (0 <= (k + 1 )) ” 
+  &&  “ (0 <= ((string_length (input)) + 1 )) ” 
+  &&  “ (spacelen > 2) ” 
+  &&  “ (spacelen <> 2) ” 
+  &&  “ (spacelen <> 1) ” 
+  &&  “ ((Znth i (c_string (input)) 0) <> 32) ” 
+  &&  “ (i < n) ” 
+  &&  “ (n = (string_length (input))) ” 
+  &&  “ (0 <= i) ” 
+  &&  “ (i <= n) ” 
+  &&  “ (0 <= k) ” 
+  &&  “ (0 <= spacelen) ” 
+  &&  “ ((k + spacelen ) <= i) ” 
+  &&  “ (k = (Zlength (output))) ” 
+  &&  “ (fix_spaces_state_z_140 input output i spacelen ) ” 
+  &&  “ (valid_string input ) ” 
+  &&  “ (problem_140_pre_z input ) ” 
+  &&  “ (ascii_range_z input ) ” 
+  &&  “ ((string_length (input)) < INT_MAX) ”
+  &&  (((out + ((k + 1 ) * sizeof(CHAR) ) )) # Char  |->_)
+  **  (CharArray.undef_missing_i out (k + 1 ) (k + 1 ) (n + 1 ) )
+  **  (CharArray.full text_pre ((string_length (input)) + 1 ) (c_string (input)) )
+  **  (CharArray.full out (k + 1 ) (app (output) ((cons (45) ((@nil Z))))) )
+.
+
+Definition fix_spaces_partial_solve_wit_9 := 
+forall (text_pre: Z) (input: (@list Z)) (out: Z) (output: (@list Z)) (spacelen: Z) (k: Z) (i: Z) (n: Z) (PreH1 : (spacelen <= 2)) (PreH2 : (0 <= (k + 1 ))) (PreH3 : (0 <= ((string_length (input)) + 1 ))) (PreH4 : (spacelen = 2)) (PreH5 : (spacelen <> 1)) (PreH6 : ((Znth i (c_string (input)) 0) <> 32)) (PreH7 : (i < n)) (PreH8 : (n = (string_length (input)))) (PreH9 : (0 <= i)) (PreH10 : (i <= n)) (PreH11 : (0 <= k)) (PreH12 : (0 <= spacelen)) (PreH13 : ((k + spacelen ) <= i)) (PreH14 : (k = (Zlength (output)))) (PreH15 : (fix_spaces_state_z_140 input output i spacelen )) (PreH16 : (valid_string input )) (PreH17 : (problem_140_pre_z input )) (PreH18 : (ascii_range_z input )) (PreH19 : ((string_length (input)) < INT_MAX)) ,
+  (CharArray.full out ((k + 1 ) + 1 ) (app ((app (output) ((cons (95) ((@nil Z)))))) ((cons (95) ((@nil Z))))) )
+  **  (CharArray.undef_seg out ((k + 1 ) + 1 ) (n + 1 ) )
+  **  (CharArray.full text_pre ((string_length (input)) + 1 ) (c_string (input)) )
+|--
+  “ (0 <= ((k + 1 ) + 1 )) ” 
+  &&  “ (spacelen <= 2) ” 
+  &&  “ (0 <= (k + 1 )) ” 
+  &&  “ (0 <= ((string_length (input)) + 1 )) ” 
+  &&  “ (spacelen = 2) ” 
+  &&  “ (spacelen <> 1) ” 
+  &&  “ ((Znth i (c_string (input)) 0) <> 32) ” 
+  &&  “ (i < n) ” 
+  &&  “ (n = (string_length (input))) ” 
+  &&  “ (0 <= i) ” 
+  &&  “ (i <= n) ” 
+  &&  “ (0 <= k) ” 
+  &&  “ (0 <= spacelen) ” 
+  &&  “ ((k + spacelen ) <= i) ” 
+  &&  “ (k = (Zlength (output))) ” 
+  &&  “ (fix_spaces_state_z_140 input output i spacelen ) ” 
+  &&  “ (valid_string input ) ” 
+  &&  “ (problem_140_pre_z input ) ” 
+  &&  “ (ascii_range_z input ) ” 
+  &&  “ ((string_length (input)) < INT_MAX) ”
+  &&  (((text_pre + (i * sizeof(CHAR) ) )) # Char  |-> (Znth i (c_string (input)) 0))
+  **  (CharArray.missing_i text_pre i 0 ((string_length (input)) + 1 ) (c_string (input)) )
+  **  (CharArray.full out ((k + 1 ) + 1 ) (app ((app (output) ((cons (95) ((@nil Z)))))) ((cons (95) ((@nil Z))))) )
+  **  (CharArray.undef_seg out ((k + 1 ) + 1 ) (n + 1 ) )
+.
+
+Definition fix_spaces_partial_solve_wit_10 := 
+forall (text_pre: Z) (input: (@list Z)) (out: Z) (output: (@list Z)) (spacelen: Z) (k: Z) (i: Z) (n: Z) (PreH1 : (0 <= ((k + 1 ) + 1 ))) (PreH2 : (spacelen <= 2)) (PreH3 : (0 <= (k + 1 ))) (PreH4 : (0 <= ((string_length (input)) + 1 ))) (PreH5 : (spacelen = 2)) (PreH6 : (spacelen <> 1)) (PreH7 : ((Znth i (c_string (input)) 0) <> 32)) (PreH8 : (i < n)) (PreH9 : (n = (string_length (input)))) (PreH10 : (0 <= i)) (PreH11 : (i <= n)) (PreH12 : (0 <= k)) (PreH13 : (0 <= spacelen)) (PreH14 : ((k + spacelen ) <= i)) (PreH15 : (k = (Zlength (output)))) (PreH16 : (fix_spaces_state_z_140 input output i spacelen )) (PreH17 : (valid_string input )) (PreH18 : (problem_140_pre_z input )) (PreH19 : (ascii_range_z input )) (PreH20 : ((string_length (input)) < INT_MAX)) ,
+  (CharArray.full text_pre ((string_length (input)) + 1 ) (c_string (input)) )
+  **  (CharArray.full out ((k + 1 ) + 1 ) (app ((app (output) ((cons (95) ((@nil Z)))))) ((cons (95) ((@nil Z))))) )
+  **  (CharArray.undef_seg out ((k + 1 ) + 1 ) (n + 1 ) )
+|--
+  “ (0 <= ((k + 1 ) + 1 )) ” 
+  &&  “ (spacelen <= 2) ” 
+  &&  “ (0 <= (k + 1 )) ” 
+  &&  “ (0 <= ((string_length (input)) + 1 )) ” 
+  &&  “ (spacelen = 2) ” 
+  &&  “ (spacelen <> 1) ” 
+  &&  “ ((Znth i (c_string (input)) 0) <> 32) ” 
+  &&  “ (i < n) ” 
+  &&  “ (n = (string_length (input))) ” 
+  &&  “ (0 <= i) ” 
+  &&  “ (i <= n) ” 
+  &&  “ (0 <= k) ” 
+  &&  “ (0 <= spacelen) ” 
+  &&  “ ((k + spacelen ) <= i) ” 
+  &&  “ (k = (Zlength (output))) ” 
+  &&  “ (fix_spaces_state_z_140 input output i spacelen ) ” 
+  &&  “ (valid_string input ) ” 
+  &&  “ (problem_140_pre_z input ) ” 
+  &&  “ (ascii_range_z input ) ” 
+  &&  “ ((string_length (input)) < INT_MAX) ”
+  &&  (((out + (((k + 1 ) + 1 ) * sizeof(CHAR) ) )) # Char  |->_)
+  **  (CharArray.undef_missing_i out ((k + 1 ) + 1 ) ((k + 1 ) + 1 ) (n + 1 ) )
+  **  (CharArray.full text_pre ((string_length (input)) + 1 ) (c_string (input)) )
+  **  (CharArray.full out ((k + 1 ) + 1 ) (app ((app (output) ((cons (95) ((@nil Z)))))) ((cons (95) ((@nil Z))))) )
+.
+
+Definition fix_spaces_partial_solve_wit_11 := 
+forall (text_pre: Z) (input: (@list Z)) (out: Z) (output: (@list Z)) (spacelen: Z) (k: Z) (i: Z) (n: Z) (PreH1 : (spacelen <= 2)) (PreH2 : (spacelen <> 2)) (PreH3 : (0 <= ((string_length (input)) + 1 ))) (PreH4 : (spacelen = 1)) (PreH5 : ((Znth i (c_string (input)) 0) <> 32)) (PreH6 : (i < n)) (PreH7 : (n = (string_length (input)))) (PreH8 : (0 <= i)) (PreH9 : (i <= n)) (PreH10 : (0 <= k)) (PreH11 : (0 <= spacelen)) (PreH12 : ((k + spacelen ) <= i)) (PreH13 : (k = (Zlength (output)))) (PreH14 : (fix_spaces_state_z_140 input output i spacelen )) (PreH15 : (valid_string input )) (PreH16 : (problem_140_pre_z input )) (PreH17 : (ascii_range_z input )) (PreH18 : ((string_length (input)) < INT_MAX)) ,
+  (CharArray.full out (k + 1 ) (app (output) ((cons (95) ((@nil Z))))) )
+  **  (CharArray.undef_seg out (k + 1 ) (n + 1 ) )
+  **  (CharArray.full text_pre ((string_length (input)) + 1 ) (c_string (input)) )
+|--
+  “ (0 <= (k + 1 )) ” 
+  &&  “ (spacelen <= 2) ” 
+  &&  “ (spacelen <> 2) ” 
+  &&  “ (0 <= ((string_length (input)) + 1 )) ” 
+  &&  “ (spacelen = 1) ” 
+  &&  “ ((Znth i (c_string (input)) 0) <> 32) ” 
+  &&  “ (i < n) ” 
+  &&  “ (n = (string_length (input))) ” 
+  &&  “ (0 <= i) ” 
+  &&  “ (i <= n) ” 
+  &&  “ (0 <= k) ” 
+  &&  “ (0 <= spacelen) ” 
+  &&  “ ((k + spacelen ) <= i) ” 
+  &&  “ (k = (Zlength (output))) ” 
+  &&  “ (fix_spaces_state_z_140 input output i spacelen ) ” 
+  &&  “ (valid_string input ) ” 
+  &&  “ (problem_140_pre_z input ) ” 
+  &&  “ (ascii_range_z input ) ” 
+  &&  “ ((string_length (input)) < INT_MAX) ”
+  &&  (((text_pre + (i * sizeof(CHAR) ) )) # Char  |-> (Znth i (c_string (input)) 0))
+  **  (CharArray.missing_i text_pre i 0 ((string_length (input)) + 1 ) (c_string (input)) )
+  **  (CharArray.full out (k + 1 ) (app (output) ((cons (95) ((@nil Z))))) )
+  **  (CharArray.undef_seg out (k + 1 ) (n + 1 ) )
+.
+
+Definition fix_spaces_partial_solve_wit_12 := 
+forall (text_pre: Z) (input: (@list Z)) (out: Z) (output: (@list Z)) (spacelen: Z) (k: Z) (i: Z) (n: Z) (PreH1 : (0 <= (k + 1 ))) (PreH2 : (spacelen <= 2)) (PreH3 : (spacelen <> 2)) (PreH4 : (0 <= ((string_length (input)) + 1 ))) (PreH5 : (spacelen = 1)) (PreH6 : ((Znth i (c_string (input)) 0) <> 32)) (PreH7 : (i < n)) (PreH8 : (n = (string_length (input)))) (PreH9 : (0 <= i)) (PreH10 : (i <= n)) (PreH11 : (0 <= k)) (PreH12 : (0 <= spacelen)) (PreH13 : ((k + spacelen ) <= i)) (PreH14 : (k = (Zlength (output)))) (PreH15 : (fix_spaces_state_z_140 input output i spacelen )) (PreH16 : (valid_string input )) (PreH17 : (problem_140_pre_z input )) (PreH18 : (ascii_range_z input )) (PreH19 : ((string_length (input)) < INT_MAX)) ,
+  (CharArray.full text_pre ((string_length (input)) + 1 ) (c_string (input)) )
+  **  (CharArray.full out (k + 1 ) (app (output) ((cons (95) ((@nil Z))))) )
+  **  (CharArray.undef_seg out (k + 1 ) (n + 1 ) )
+|--
+  “ (0 <= (k + 1 )) ” 
+  &&  “ (spacelen <= 2) ” 
+  &&  “ (spacelen <> 2) ” 
+  &&  “ (0 <= ((string_length (input)) + 1 )) ” 
+  &&  “ (spacelen = 1) ” 
+  &&  “ ((Znth i (c_string (input)) 0) <> 32) ” 
+  &&  “ (i < n) ” 
+  &&  “ (n = (string_length (input))) ” 
+  &&  “ (0 <= i) ” 
+  &&  “ (i <= n) ” 
+  &&  “ (0 <= k) ” 
+  &&  “ (0 <= spacelen) ” 
+  &&  “ ((k + spacelen ) <= i) ” 
+  &&  “ (k = (Zlength (output))) ” 
+  &&  “ (fix_spaces_state_z_140 input output i spacelen ) ” 
+  &&  “ (valid_string input ) ” 
+  &&  “ (problem_140_pre_z input ) ” 
+  &&  “ (ascii_range_z input ) ” 
+  &&  “ ((string_length (input)) < INT_MAX) ”
+  &&  (((out + ((k + 1 ) * sizeof(CHAR) ) )) # Char  |->_)
+  **  (CharArray.undef_missing_i out (k + 1 ) (k + 1 ) (n + 1 ) )
+  **  (CharArray.full text_pre ((string_length (input)) + 1 ) (c_string (input)) )
+  **  (CharArray.full out (k + 1 ) (app (output) ((cons (95) ((@nil Z))))) )
+.
+
+Definition fix_spaces_partial_solve_wit_13 := 
+forall (text_pre: Z) (input: (@list Z)) (out: Z) (output: (@list Z)) (spacelen: Z) (k: Z) (i: Z) (n: Z) (PreH1 : (spacelen <= 2)) (PreH2 : (spacelen <> 2)) (PreH3 : (spacelen <> 1)) (PreH4 : ((Znth i (c_string (input)) 0) <> 32)) (PreH5 : (i < n)) (PreH6 : (n = (string_length (input)))) (PreH7 : (0 <= i)) (PreH8 : (i <= n)) (PreH9 : (0 <= k)) (PreH10 : (0 <= spacelen)) (PreH11 : ((k + spacelen ) <= i)) (PreH12 : (k = (Zlength (output)))) (PreH13 : (fix_spaces_state_z_140 input output i spacelen )) (PreH14 : (valid_string input )) (PreH15 : (problem_140_pre_z input )) (PreH16 : (ascii_range_z input )) (PreH17 : ((string_length (input)) < INT_MAX)) ,
+  (store_string text_pre input )
+  **  (CharArray.full out k output )
+  **  (CharArray.undef_seg out k (n + 1 ) )
+|--
+  “ (0 <= ((string_length (input)) + 1 )) ” 
+  &&  “ (spacelen <= 2) ” 
+  &&  “ (spacelen <> 2) ” 
+  &&  “ (spacelen <> 1) ” 
+  &&  “ ((Znth i (c_string (input)) 0) <> 32) ” 
+  &&  “ (i < n) ” 
+  &&  “ (n = (string_length (input))) ” 
+  &&  “ (0 <= i) ” 
+  &&  “ (i <= n) ” 
+  &&  “ (0 <= k) ” 
+  &&  “ (0 <= spacelen) ” 
+  &&  “ ((k + spacelen ) <= i) ” 
+  &&  “ (k = (Zlength (output))) ” 
+  &&  “ (fix_spaces_state_z_140 input output i spacelen ) ” 
+  &&  “ (valid_string input ) ” 
+  &&  “ (problem_140_pre_z input ) ” 
+  &&  “ (ascii_range_z input ) ” 
+  &&  “ ((string_length (input)) < INT_MAX) ”
+  &&  (((out + (k * sizeof(CHAR) ) )) # Char  |->_)
+  **  (CharArray.full text_pre ((string_length (input)) + 1 ) (c_string (input)) )
+  **  (CharArray.undef_missing_i out k k (n + 1 ) )
+  **  (CharArray.full out k output )
+.
+
+Definition fix_spaces_partial_solve_wit_14 := 
+forall (text_pre: Z) (input: (@list Z)) (out: Z) (output: (@list Z)) (spacelen: Z) (k: Z) (i: Z) (n: Z) (PreH1 : (spacelen = 1)) (PreH2 : (i >= n)) (PreH3 : (n = (string_length (input)))) (PreH4 : (0 <= i)) (PreH5 : (i <= n)) (PreH6 : (0 <= k)) (PreH7 : (0 <= spacelen)) (PreH8 : ((k + spacelen ) <= i)) (PreH9 : (k = (Zlength (output)))) (PreH10 : (fix_spaces_state_z_140 input output i spacelen )) (PreH11 : (valid_string input )) (PreH12 : (problem_140_pre_z input )) (PreH13 : (ascii_range_z input )) (PreH14 : ((string_length (input)) < INT_MAX)) ,
+  (store_string text_pre input )
+  **  (CharArray.full out k output )
+  **  (CharArray.undef_seg out k (n + 1 ) )
+|--
+  “ (0 <= ((string_length (input)) + 1 )) ” 
+  &&  “ (spacelen = 1) ” 
+  &&  “ (i >= n) ” 
+  &&  “ (n = (string_length (input))) ” 
+  &&  “ (0 <= i) ” 
+  &&  “ (i <= n) ” 
+  &&  “ (0 <= k) ” 
+  &&  “ (0 <= spacelen) ” 
+  &&  “ ((k + spacelen ) <= i) ” 
+  &&  “ (k = (Zlength (output))) ” 
+  &&  “ (fix_spaces_state_z_140 input output i spacelen ) ” 
+  &&  “ (valid_string input ) ” 
+  &&  “ (problem_140_pre_z input ) ” 
+  &&  “ (ascii_range_z input ) ” 
+  &&  “ ((string_length (input)) < INT_MAX) ”
+  &&  (((out + (k * sizeof(CHAR) ) )) # Char  |->_)
+  **  (CharArray.full text_pre ((string_length (input)) + 1 ) (c_string (input)) )
+  **  (CharArray.undef_missing_i out k k (n + 1 ) )
+  **  (CharArray.full out k output )
+.
+
+Definition fix_spaces_partial_solve_wit_15 := 
+forall (text_pre: Z) (input: (@list Z)) (out: Z) (output: (@list Z)) (spacelen: Z) (k: Z) (i: Z) (n: Z) (PreH1 : (spacelen = 2)) (PreH2 : (spacelen <> 1)) (PreH3 : (i >= n)) (PreH4 : (n = (string_length (input)))) (PreH5 : (0 <= i)) (PreH6 : (i <= n)) (PreH7 : (0 <= k)) (PreH8 : (0 <= spacelen)) (PreH9 : ((k + spacelen ) <= i)) (PreH10 : (k = (Zlength (output)))) (PreH11 : (fix_spaces_state_z_140 input output i spacelen )) (PreH12 : (valid_string input )) (PreH13 : (problem_140_pre_z input )) (PreH14 : (ascii_range_z input )) (PreH15 : ((string_length (input)) < INT_MAX)) ,
+  (store_string text_pre input )
+  **  (CharArray.full out k output )
+  **  (CharArray.undef_seg out k (n + 1 ) )
+|--
+  “ (0 <= ((string_length (input)) + 1 )) ” 
+  &&  “ (spacelen = 2) ” 
+  &&  “ (spacelen <> 1) ” 
+  &&  “ (i >= n) ” 
+  &&  “ (n = (string_length (input))) ” 
+  &&  “ (0 <= i) ” 
+  &&  “ (i <= n) ” 
+  &&  “ (0 <= k) ” 
+  &&  “ (0 <= spacelen) ” 
+  &&  “ ((k + spacelen ) <= i) ” 
+  &&  “ (k = (Zlength (output))) ” 
+  &&  “ (fix_spaces_state_z_140 input output i spacelen ) ” 
+  &&  “ (valid_string input ) ” 
+  &&  “ (problem_140_pre_z input ) ” 
+  &&  “ (ascii_range_z input ) ” 
+  &&  “ ((string_length (input)) < INT_MAX) ”
+  &&  (((out + (k * sizeof(CHAR) ) )) # Char  |->_)
+  **  (CharArray.full text_pre ((string_length (input)) + 1 ) (c_string (input)) )
+  **  (CharArray.undef_missing_i out k k (n + 1 ) )
+  **  (CharArray.full out k output )
+.
+
+Definition fix_spaces_partial_solve_wit_16 := 
+forall (text_pre: Z) (input: (@list Z)) (out: Z) (output: (@list Z)) (spacelen: Z) (k: Z) (i: Z) (n: Z) (PreH1 : (0 <= ((string_length (input)) + 1 ))) (PreH2 : (spacelen = 2)) (PreH3 : (spacelen <> 1)) (PreH4 : (i >= n)) (PreH5 : (n = (string_length (input)))) (PreH6 : (0 <= i)) (PreH7 : (i <= n)) (PreH8 : (0 <= k)) (PreH9 : (0 <= spacelen)) (PreH10 : ((k + spacelen ) <= i)) (PreH11 : (k = (Zlength (output)))) (PreH12 : (fix_spaces_state_z_140 input output i spacelen )) (PreH13 : (valid_string input )) (PreH14 : (problem_140_pre_z input )) (PreH15 : (ascii_range_z input )) (PreH16 : ((string_length (input)) < INT_MAX)) ,
+  (CharArray.full out (k + 1 ) (app (output) ((cons (95) ((@nil Z))))) )
+  **  (CharArray.undef_seg out (k + 1 ) (n + 1 ) )
+  **  (CharArray.full text_pre ((string_length (input)) + 1 ) (c_string (input)) )
+|--
+  “ (0 <= (k + 1 )) ” 
+  &&  “ (0 <= ((string_length (input)) + 1 )) ” 
+  &&  “ (spacelen = 2) ” 
+  &&  “ (spacelen <> 1) ” 
+  &&  “ (i >= n) ” 
+  &&  “ (n = (string_length (input))) ” 
+  &&  “ (0 <= i) ” 
+  &&  “ (i <= n) ” 
+  &&  “ (0 <= k) ” 
+  &&  “ (0 <= spacelen) ” 
+  &&  “ ((k + spacelen ) <= i) ” 
+  &&  “ (k = (Zlength (output))) ” 
+  &&  “ (fix_spaces_state_z_140 input output i spacelen ) ” 
+  &&  “ (valid_string input ) ” 
+  &&  “ (problem_140_pre_z input ) ” 
+  &&  “ (ascii_range_z input ) ” 
+  &&  “ ((string_length (input)) < INT_MAX) ”
+  &&  (((out + ((k + 1 ) * sizeof(CHAR) ) )) # Char  |->_)
+  **  (CharArray.undef_missing_i out (k + 1 ) (k + 1 ) (n + 1 ) )
+  **  (CharArray.full out (k + 1 ) (app (output) ((cons (95) ((@nil Z))))) )
+  **  (CharArray.full text_pre ((string_length (input)) + 1 ) (c_string (input)) )
+.
+
+Definition fix_spaces_partial_solve_wit_17 := 
+forall (text_pre: Z) (input: (@list Z)) (out: Z) (output: (@list Z)) (spacelen: Z) (k: Z) (i: Z) (n: Z) (PreH1 : (spacelen > 2)) (PreH2 : (spacelen <> 2)) (PreH3 : (spacelen <> 1)) (PreH4 : (i >= n)) (PreH5 : (n = (string_length (input)))) (PreH6 : (0 <= i)) (PreH7 : (i <= n)) (PreH8 : (0 <= k)) (PreH9 : (0 <= spacelen)) (PreH10 : ((k + spacelen ) <= i)) (PreH11 : (k = (Zlength (output)))) (PreH12 : (fix_spaces_state_z_140 input output i spacelen )) (PreH13 : (valid_string input )) (PreH14 : (problem_140_pre_z input )) (PreH15 : (ascii_range_z input )) (PreH16 : ((string_length (input)) < INT_MAX)) ,
+  (store_string text_pre input )
+  **  (CharArray.full out k output )
+  **  (CharArray.undef_seg out k (n + 1 ) )
+|--
+  “ (0 <= ((string_length (input)) + 1 )) ” 
+  &&  “ (spacelen > 2) ” 
+  &&  “ (spacelen <> 2) ” 
+  &&  “ (spacelen <> 1) ” 
+  &&  “ (i >= n) ” 
+  &&  “ (n = (string_length (input))) ” 
+  &&  “ (0 <= i) ” 
+  &&  “ (i <= n) ” 
+  &&  “ (0 <= k) ” 
+  &&  “ (0 <= spacelen) ” 
+  &&  “ ((k + spacelen ) <= i) ” 
+  &&  “ (k = (Zlength (output))) ” 
+  &&  “ (fix_spaces_state_z_140 input output i spacelen ) ” 
+  &&  “ (valid_string input ) ” 
+  &&  “ (problem_140_pre_z input ) ” 
+  &&  “ (ascii_range_z input ) ” 
+  &&  “ ((string_length (input)) < INT_MAX) ”
+  &&  (((out + (k * sizeof(CHAR) ) )) # Char  |->_)
+  **  (CharArray.full text_pre ((string_length (input)) + 1 ) (c_string (input)) )
+  **  (CharArray.undef_missing_i out k k (n + 1 ) )
+  **  (CharArray.full out k output )
+.
+
+Definition fix_spaces_partial_solve_wit_18 := 
+forall (text_pre: Z) (input: (@list Z)) (prefix: (@list Z)) (output: (@list Z)) (n: Z) (k: Z) (spacelen: Z) (out: Z) (PreH1 : (n = (string_length (input)))) (PreH2 : (0 <= k)) (PreH3 : (0 <= spacelen)) (PreH4 : (k <= n)) (PreH5 : (k = (Zlength (output)))) (PreH6 : (output = (app (prefix) ((flush_spaces_z_140 (spacelen)))))) (PreH7 : (fix_spaces_state_z_140 input prefix n spacelen )) (PreH8 : (valid_string input )) (PreH9 : (problem_140_pre_z input )) (PreH10 : (ascii_range_z input )) (PreH11 : ((string_length (input)) < INT_MAX)) ,
+  (store_string text_pre input )
+  **  (CharArray.full out k output )
+  **  (CharArray.undef_seg out k (n + 1 ) )
+|--
+  “ (0 <= ((string_length (input)) + 1 )) ” 
+  &&  “ (n = (string_length (input))) ” 
+  &&  “ (0 <= k) ” 
+  &&  “ (0 <= spacelen) ” 
+  &&  “ (k <= n) ” 
+  &&  “ (k = (Zlength (output))) ” 
+  &&  “ (output = (app (prefix) ((flush_spaces_z_140 (spacelen))))) ” 
+  &&  “ (fix_spaces_state_z_140 input prefix n spacelen ) ” 
+  &&  “ (valid_string input ) ” 
+  &&  “ (problem_140_pre_z input ) ” 
+  &&  “ (ascii_range_z input ) ” 
+  &&  “ ((string_length (input)) < INT_MAX) ”
+  &&  (((out + (k * sizeof(CHAR) ) )) # Char  |->_)
+  **  (CharArray.full text_pre ((string_length (input)) + 1 ) (c_string (input)) )
+  **  (CharArray.undef_missing_i out k k (n + 1 ) )
+  **  (CharArray.full out k output )
+.
+
+Module Type VC_Correct.
+
+Include char_array_Strategy_Correct.
+Include string_Strategy_Correct.
+
+Axiom proof_of_fix_spaces_safety_wit_1 : fix_spaces_safety_wit_1.
+Axiom proof_of_fix_spaces_safety_wit_2 : fix_spaces_safety_wit_2.
+Axiom proof_of_fix_spaces_safety_wit_3 : fix_spaces_safety_wit_3.
+Axiom proof_of_fix_spaces_safety_wit_4 : fix_spaces_safety_wit_4.
+Axiom proof_of_fix_spaces_safety_wit_5 : fix_spaces_safety_wit_5.
+Axiom proof_of_fix_spaces_safety_wit_6 : fix_spaces_safety_wit_6.
+Axiom proof_of_fix_spaces_safety_wit_7 : fix_spaces_safety_wit_7.
+Axiom proof_of_fix_spaces_safety_wit_8 : fix_spaces_safety_wit_8.
+Axiom proof_of_fix_spaces_safety_wit_9 : fix_spaces_safety_wit_9.
+Axiom proof_of_fix_spaces_safety_wit_10 : fix_spaces_safety_wit_10.
+Axiom proof_of_fix_spaces_safety_wit_11 : fix_spaces_safety_wit_11.
+Axiom proof_of_fix_spaces_safety_wit_12 : fix_spaces_safety_wit_12.
+Axiom proof_of_fix_spaces_safety_wit_13 : fix_spaces_safety_wit_13.
+Axiom proof_of_fix_spaces_safety_wit_14 : fix_spaces_safety_wit_14.
+Axiom proof_of_fix_spaces_safety_wit_15 : fix_spaces_safety_wit_15.
+Axiom proof_of_fix_spaces_safety_wit_16 : fix_spaces_safety_wit_16.
+Axiom proof_of_fix_spaces_safety_wit_17 : fix_spaces_safety_wit_17.
+Axiom proof_of_fix_spaces_safety_wit_18 : fix_spaces_safety_wit_18.
+Axiom proof_of_fix_spaces_safety_wit_19 : fix_spaces_safety_wit_19.
+Axiom proof_of_fix_spaces_safety_wit_20 : fix_spaces_safety_wit_20.
+Axiom proof_of_fix_spaces_safety_wit_21 : fix_spaces_safety_wit_21.
+Axiom proof_of_fix_spaces_safety_wit_22 : fix_spaces_safety_wit_22.
+Axiom proof_of_fix_spaces_safety_wit_23 : fix_spaces_safety_wit_23.
+Axiom proof_of_fix_spaces_safety_wit_24 : fix_spaces_safety_wit_24.
+Axiom proof_of_fix_spaces_safety_wit_25 : fix_spaces_safety_wit_25.
+Axiom proof_of_fix_spaces_safety_wit_26 : fix_spaces_safety_wit_26.
+Axiom proof_of_fix_spaces_safety_wit_27 : fix_spaces_safety_wit_27.
+Axiom proof_of_fix_spaces_safety_wit_28 : fix_spaces_safety_wit_28.
+Axiom proof_of_fix_spaces_safety_wit_29 : fix_spaces_safety_wit_29.
+Axiom proof_of_fix_spaces_safety_wit_30 : fix_spaces_safety_wit_30.
+Axiom proof_of_fix_spaces_safety_wit_31 : fix_spaces_safety_wit_31.
+Axiom proof_of_fix_spaces_safety_wit_32 : fix_spaces_safety_wit_32.
+Axiom proof_of_fix_spaces_safety_wit_33 : fix_spaces_safety_wit_33.
+Axiom proof_of_fix_spaces_safety_wit_34 : fix_spaces_safety_wit_34.
+Axiom proof_of_fix_spaces_safety_wit_35 : fix_spaces_safety_wit_35.
+Axiom proof_of_fix_spaces_safety_wit_36 : fix_spaces_safety_wit_36.
+Axiom proof_of_fix_spaces_safety_wit_37 : fix_spaces_safety_wit_37.
+Axiom proof_of_fix_spaces_safety_wit_38 : fix_spaces_safety_wit_38.
+Axiom proof_of_fix_spaces_safety_wit_39 : fix_spaces_safety_wit_39.
+Axiom proof_of_fix_spaces_safety_wit_40 : fix_spaces_safety_wit_40.
+Axiom proof_of_fix_spaces_safety_wit_41 : fix_spaces_safety_wit_41.
+Axiom proof_of_fix_spaces_safety_wit_42 : fix_spaces_safety_wit_42.
+Axiom proof_of_fix_spaces_safety_wit_43 : fix_spaces_safety_wit_43.
+Axiom proof_of_fix_spaces_safety_wit_44 : fix_spaces_safety_wit_44.
+Axiom proof_of_fix_spaces_safety_wit_45 : fix_spaces_safety_wit_45.
+Axiom proof_of_fix_spaces_safety_wit_46 : fix_spaces_safety_wit_46.
+Axiom proof_of_fix_spaces_safety_wit_47 : fix_spaces_safety_wit_47.
+Axiom proof_of_fix_spaces_safety_wit_48 : fix_spaces_safety_wit_48.
+Axiom proof_of_fix_spaces_safety_wit_49 : fix_spaces_safety_wit_49.
+Axiom proof_of_fix_spaces_safety_wit_50 : fix_spaces_safety_wit_50.
+Axiom proof_of_fix_spaces_safety_wit_51 : fix_spaces_safety_wit_51.
+Axiom proof_of_fix_spaces_safety_wit_52 : fix_spaces_safety_wit_52.
+Axiom proof_of_fix_spaces_safety_wit_53 : fix_spaces_safety_wit_53.
+Axiom proof_of_fix_spaces_safety_wit_54 : fix_spaces_safety_wit_54.
+Axiom proof_of_fix_spaces_safety_wit_55 : fix_spaces_safety_wit_55.
+Axiom proof_of_fix_spaces_safety_wit_56 : fix_spaces_safety_wit_56.
+Axiom proof_of_fix_spaces_safety_wit_57 : fix_spaces_safety_wit_57.
+Axiom proof_of_fix_spaces_safety_wit_58 : fix_spaces_safety_wit_58.
+Axiom proof_of_fix_spaces_safety_wit_59 : fix_spaces_safety_wit_59.
+Axiom proof_of_fix_spaces_safety_wit_60 : fix_spaces_safety_wit_60.
+Axiom proof_of_fix_spaces_safety_wit_61 : fix_spaces_safety_wit_61.
+Axiom proof_of_fix_spaces_safety_wit_62 : fix_spaces_safety_wit_62.
+Axiom proof_of_fix_spaces_safety_wit_63 : fix_spaces_safety_wit_63.
+Axiom proof_of_fix_spaces_safety_wit_64 : fix_spaces_safety_wit_64.
+Axiom proof_of_fix_spaces_safety_wit_65 : fix_spaces_safety_wit_65.
+Axiom proof_of_fix_spaces_safety_wit_66 : fix_spaces_safety_wit_66.
+Axiom proof_of_fix_spaces_entail_wit_1 : fix_spaces_entail_wit_1.
+Axiom proof_of_fix_spaces_entail_wit_2_1 : fix_spaces_entail_wit_2_1.
+Axiom proof_of_fix_spaces_entail_wit_2_2 : fix_spaces_entail_wit_2_2.
+Axiom proof_of_fix_spaces_entail_wit_2_3 : fix_spaces_entail_wit_2_3.
+Axiom proof_of_fix_spaces_entail_wit_2_4 : fix_spaces_entail_wit_2_4.
+Axiom proof_of_fix_spaces_entail_wit_2_5 : fix_spaces_entail_wit_2_5.
+Axiom proof_of_fix_spaces_entail_wit_3 : fix_spaces_entail_wit_3.
+Axiom proof_of_fix_spaces_entail_wit_4_1 : fix_spaces_entail_wit_4_1.
+Axiom proof_of_fix_spaces_entail_wit_4_2 : fix_spaces_entail_wit_4_2.
+Axiom proof_of_fix_spaces_entail_wit_4_3 : fix_spaces_entail_wit_4_3.
+Axiom proof_of_fix_spaces_entail_wit_4_4 : fix_spaces_entail_wit_4_4.
+Axiom proof_of_fix_spaces_return_wit_1 : fix_spaces_return_wit_1.
+Axiom proof_of_fix_spaces_partial_solve_wit_1_pure : fix_spaces_partial_solve_wit_1_pure.
+Axiom proof_of_fix_spaces_partial_solve_wit_1 : fix_spaces_partial_solve_wit_1.
+Axiom proof_of_fix_spaces_partial_solve_wit_2_pure : fix_spaces_partial_solve_wit_2_pure.
+Axiom proof_of_fix_spaces_partial_solve_wit_2 : fix_spaces_partial_solve_wit_2.
+Axiom proof_of_fix_spaces_partial_solve_wit_3 : fix_spaces_partial_solve_wit_3.
+Axiom proof_of_fix_spaces_partial_solve_wit_4 : fix_spaces_partial_solve_wit_4.
+Axiom proof_of_fix_spaces_partial_solve_wit_5 : fix_spaces_partial_solve_wit_5.
+Axiom proof_of_fix_spaces_partial_solve_wit_6 : fix_spaces_partial_solve_wit_6.
+Axiom proof_of_fix_spaces_partial_solve_wit_7 : fix_spaces_partial_solve_wit_7.
+Axiom proof_of_fix_spaces_partial_solve_wit_8 : fix_spaces_partial_solve_wit_8.
+Axiom proof_of_fix_spaces_partial_solve_wit_9 : fix_spaces_partial_solve_wit_9.
+Axiom proof_of_fix_spaces_partial_solve_wit_10 : fix_spaces_partial_solve_wit_10.
+Axiom proof_of_fix_spaces_partial_solve_wit_11 : fix_spaces_partial_solve_wit_11.
+Axiom proof_of_fix_spaces_partial_solve_wit_12 : fix_spaces_partial_solve_wit_12.
+Axiom proof_of_fix_spaces_partial_solve_wit_13 : fix_spaces_partial_solve_wit_13.
+Axiom proof_of_fix_spaces_partial_solve_wit_14 : fix_spaces_partial_solve_wit_14.
+Axiom proof_of_fix_spaces_partial_solve_wit_15 : fix_spaces_partial_solve_wit_15.
+Axiom proof_of_fix_spaces_partial_solve_wit_16 : fix_spaces_partial_solve_wit_16.
+Axiom proof_of_fix_spaces_partial_solve_wit_17 : fix_spaces_partial_solve_wit_17.
+Axiom proof_of_fix_spaces_partial_solve_wit_18 : fix_spaces_partial_solve_wit_18.
+
+End VC_Correct.
