QCP_examples/humaneval/spec_logic_rewrite_c_files/C_140_proof_auto.v
@@ -1,0 +1,281 @@
+Require Import Coq.ZArith.ZArith.
+Require Import Coq.Bool.Bool.
+Require Import Coq.Strings.String.
+Require Import Coq.Strings.Ascii.
+Require Import Coq.Lists.List.
+Require Import Coq.Classes.RelationClasses.
+Require Import Coq.Classes.Morphisms.
+Require Import Coq.micromega.Psatz.
+Require Import Coq.Sorting.Permutation.
+From AUXLib Require Import int_auto Axioms Feq Idents ListLib VMap.
+Require Import SetsClass.SetsClass. Import SetsNotation.
+From SimpleC.SL Require Import Mem SeparationLogic.
+From SimpleC.EE Require Import C_140_goal.
+Require Import Logic.LogicGenerator.demo932.Interface.
+Local Open Scope Z_scope.
+Local Open Scope sets.
+Local Open Scope string_scope.
+Local Open Scope list.
+Import naive_C_Rules.
+Require Import SimpleC.StdLib.string_lib.
+Require Import coins_140.
+Local Open Scope sac.
+
+Lemma proof_of_fix_spaces_safety_wit_1 : fix_spaces_safety_wit_1.
+Proof. Admitted. 
+
+Lemma proof_of_fix_spaces_safety_wit_2 : fix_spaces_safety_wit_2.
+Proof. Admitted. 
+
+Lemma proof_of_fix_spaces_safety_wit_3 : fix_spaces_safety_wit_3.
+Proof. Admitted. 
+
+Lemma proof_of_fix_spaces_safety_wit_4 : fix_spaces_safety_wit_4.
+Proof. Admitted. 
+
+Lemma proof_of_fix_spaces_safety_wit_5 : fix_spaces_safety_wit_5.
+Proof. Admitted. 
+
+Lemma proof_of_fix_spaces_safety_wit_6 : fix_spaces_safety_wit_6.
+Proof. Admitted. 
+
+Lemma proof_of_fix_spaces_safety_wit_7 : fix_spaces_safety_wit_7.
+Proof. Admitted. 
+
+Lemma proof_of_fix_spaces_safety_wit_8 : fix_spaces_safety_wit_8.
+Proof. Admitted. 
+
+Lemma proof_of_fix_spaces_safety_wit_9 : fix_spaces_safety_wit_9.
+Proof. Admitted. 
+
+Lemma proof_of_fix_spaces_safety_wit_10 : fix_spaces_safety_wit_10.
+Proof. Admitted. 
+
+Lemma proof_of_fix_spaces_safety_wit_11 : fix_spaces_safety_wit_11.
+Proof. Admitted. 
+
+Lemma proof_of_fix_spaces_safety_wit_12 : fix_spaces_safety_wit_12.
+Proof. Admitted. 
+
+Lemma proof_of_fix_spaces_safety_wit_13 : fix_spaces_safety_wit_13.
+Proof. Admitted. 
+
+Lemma proof_of_fix_spaces_safety_wit_14 : fix_spaces_safety_wit_14.
+Proof. Admitted. 
+
+Lemma proof_of_fix_spaces_safety_wit_15 : fix_spaces_safety_wit_15.
+Proof. Admitted. 
+
+Lemma proof_of_fix_spaces_safety_wit_16 : fix_spaces_safety_wit_16.
+Proof. Admitted. 
+
+Lemma proof_of_fix_spaces_safety_wit_17 : fix_spaces_safety_wit_17.
+Proof. Admitted. 
+
+Lemma proof_of_fix_spaces_safety_wit_18 : fix_spaces_safety_wit_18.
+Proof. Admitted. 
+
+Lemma proof_of_fix_spaces_safety_wit_19 : fix_spaces_safety_wit_19.
+Proof. Admitted. 
+
+Lemma proof_of_fix_spaces_safety_wit_20 : fix_spaces_safety_wit_20.
+Proof. Admitted. 
+
+Lemma proof_of_fix_spaces_safety_wit_21 : fix_spaces_safety_wit_21.
+Proof. Admitted. 
+
+Lemma proof_of_fix_spaces_safety_wit_22 : fix_spaces_safety_wit_22.
+Proof. Admitted. 
+
+Lemma proof_of_fix_spaces_safety_wit_23 : fix_spaces_safety_wit_23.
+Proof. Admitted. 
+
+Lemma proof_of_fix_spaces_safety_wit_24 : fix_spaces_safety_wit_24.
+Proof. Admitted. 
+
+Lemma proof_of_fix_spaces_safety_wit_25 : fix_spaces_safety_wit_25.
+Proof. Admitted. 
+
+Lemma proof_of_fix_spaces_safety_wit_26 : fix_spaces_safety_wit_26.
+Proof. Admitted. 
+
+Lemma proof_of_fix_spaces_safety_wit_27 : fix_spaces_safety_wit_27.
+Proof. Admitted. 
+
+Lemma proof_of_fix_spaces_safety_wit_28 : fix_spaces_safety_wit_28.
+Proof. Admitted. 
+
+Lemma proof_of_fix_spaces_safety_wit_29 : fix_spaces_safety_wit_29.
+Proof. Admitted. 
+
+Lemma proof_of_fix_spaces_safety_wit_30 : fix_spaces_safety_wit_30.
+Proof. Admitted. 
+
+Lemma proof_of_fix_spaces_safety_wit_31 : fix_spaces_safety_wit_31.
+Proof. Admitted. 
+
+Lemma proof_of_fix_spaces_safety_wit_32 : fix_spaces_safety_wit_32.
+Proof. Admitted. 
+
+Lemma proof_of_fix_spaces_safety_wit_33 : fix_spaces_safety_wit_33.
+Proof. Admitted. 
+
+Lemma proof_of_fix_spaces_safety_wit_34 : fix_spaces_safety_wit_34.
+Proof. Admitted. 
+
+Lemma proof_of_fix_spaces_safety_wit_35 : fix_spaces_safety_wit_35.
+Proof. Admitted. 
+
+Lemma proof_of_fix_spaces_safety_wit_36 : fix_spaces_safety_wit_36.
+Proof. Admitted. 
+
+Lemma proof_of_fix_spaces_safety_wit_37 : fix_spaces_safety_wit_37.
+Proof. Admitted. 
+
+Lemma proof_of_fix_spaces_safety_wit_38 : fix_spaces_safety_wit_38.
+Proof. Admitted. 
+
+Lemma proof_of_fix_spaces_safety_wit_39 : fix_spaces_safety_wit_39.
+Proof. Admitted. 
+
+Lemma proof_of_fix_spaces_safety_wit_40 : fix_spaces_safety_wit_40.
+Proof. Admitted. 
+
+Lemma proof_of_fix_spaces_safety_wit_41 : fix_spaces_safety_wit_41.
+Proof. Admitted. 
+
+Lemma proof_of_fix_spaces_safety_wit_42 : fix_spaces_safety_wit_42.
+Proof. Admitted. 
+
+Lemma proof_of_fix_spaces_safety_wit_43 : fix_spaces_safety_wit_43.
+Proof. Admitted. 
+
+Lemma proof_of_fix_spaces_safety_wit_44 : fix_spaces_safety_wit_44.
+Proof. Admitted. 
+
+Lemma proof_of_fix_spaces_safety_wit_45 : fix_spaces_safety_wit_45.
+Proof. Admitted. 
+
+Lemma proof_of_fix_spaces_safety_wit_46 : fix_spaces_safety_wit_46.
+Proof. Admitted. 
+
+Lemma proof_of_fix_spaces_safety_wit_47 : fix_spaces_safety_wit_47.
+Proof. Admitted. 
+
+Lemma proof_of_fix_spaces_safety_wit_48 : fix_spaces_safety_wit_48.
+Proof. Admitted. 
+
+Lemma proof_of_fix_spaces_safety_wit_49 : fix_spaces_safety_wit_49.
+Proof. Admitted. 
+
+Lemma proof_of_fix_spaces_safety_wit_50 : fix_spaces_safety_wit_50.
+Proof. Admitted. 
+
+Lemma proof_of_fix_spaces_safety_wit_51 : fix_spaces_safety_wit_51.
+Proof. Admitted. 
+
+Lemma proof_of_fix_spaces_safety_wit_52 : fix_spaces_safety_wit_52.
+Proof. Admitted. 
+
+Lemma proof_of_fix_spaces_safety_wit_53 : fix_spaces_safety_wit_53.
+Proof. Admitted. 
+
+Lemma proof_of_fix_spaces_safety_wit_54 : fix_spaces_safety_wit_54.
+Proof. Admitted. 
+
+Lemma proof_of_fix_spaces_safety_wit_55 : fix_spaces_safety_wit_55.
+Proof. Admitted. 
+
+Lemma proof_of_fix_spaces_safety_wit_56 : fix_spaces_safety_wit_56.
+Proof. Admitted. 
+
+Lemma proof_of_fix_spaces_safety_wit_57 : fix_spaces_safety_wit_57.
+Proof. Admitted. 
+
+Lemma proof_of_fix_spaces_safety_wit_58 : fix_spaces_safety_wit_58.
+Proof. Admitted. 
+
+Lemma proof_of_fix_spaces_safety_wit_59 : fix_spaces_safety_wit_59.
+Proof. Admitted. 
+
+Lemma proof_of_fix_spaces_safety_wit_60 : fix_spaces_safety_wit_60.
+Proof. Admitted. 
+
+Lemma proof_of_fix_spaces_safety_wit_61 : fix_spaces_safety_wit_61.
+Proof. Admitted. 
+
+Lemma proof_of_fix_spaces_safety_wit_62 : fix_spaces_safety_wit_62.
+Proof. Admitted. 
+
+Lemma proof_of_fix_spaces_safety_wit_63 : fix_spaces_safety_wit_63.
+Proof. Admitted. 
+
+Lemma proof_of_fix_spaces_safety_wit_64 : fix_spaces_safety_wit_64.
+Proof. Admitted. 
+
+Lemma proof_of_fix_spaces_safety_wit_65 : fix_spaces_safety_wit_65.
+Proof. Admitted. 
+
+Lemma proof_of_fix_spaces_safety_wit_66 : fix_spaces_safety_wit_66.
+Proof. Admitted. 
+
+Lemma proof_of_fix_spaces_entail_wit_3 : fix_spaces_entail_wit_3.
+Proof. Admitted. 
+
+Lemma proof_of_fix_spaces_partial_solve_wit_1_pure : fix_spaces_partial_solve_wit_1_pure.
+Proof. Admitted. 
+
+Lemma proof_of_fix_spaces_partial_solve_wit_1 : fix_spaces_partial_solve_wit_1.
+Proof. Admitted. 
+
+Lemma proof_of_fix_spaces_partial_solve_wit_2 : fix_spaces_partial_solve_wit_2.
+Proof. Admitted. 
+
+Lemma proof_of_fix_spaces_partial_solve_wit_3 : fix_spaces_partial_solve_wit_3.
+Proof. Admitted. 
+
+Lemma proof_of_fix_spaces_partial_solve_wit_4 : fix_spaces_partial_solve_wit_4.
+Proof. Admitted. 
+
+Lemma proof_of_fix_spaces_partial_solve_wit_5 : fix_spaces_partial_solve_wit_5.
+Proof. Admitted. 
+
+Lemma proof_of_fix_spaces_partial_solve_wit_6 : fix_spaces_partial_solve_wit_6.
+Proof. Admitted. 
+
+Lemma proof_of_fix_spaces_partial_solve_wit_7 : fix_spaces_partial_solve_wit_7.
+Proof. Admitted. 
+
+Lemma proof_of_fix_spaces_partial_solve_wit_8 : fix_spaces_partial_solve_wit_8.
+Proof. Admitted. 
+
+Lemma proof_of_fix_spaces_partial_solve_wit_9 : fix_spaces_partial_solve_wit_9.
+Proof. Admitted. 
+
+Lemma proof_of_fix_spaces_partial_solve_wit_10 : fix_spaces_partial_solve_wit_10.
+Proof. Admitted. 
+
+Lemma proof_of_fix_spaces_partial_solve_wit_11 : fix_spaces_partial_solve_wit_11.
+Proof. Admitted. 
+
+Lemma proof_of_fix_spaces_partial_solve_wit_12 : fix_spaces_partial_solve_wit_12.
+Proof. Admitted. 
+
+Lemma proof_of_fix_spaces_partial_solve_wit_13 : fix_spaces_partial_solve_wit_13.
+Proof. Admitted. 
+
+Lemma proof_of_fix_spaces_partial_solve_wit_14 : fix_spaces_partial_solve_wit_14.
+Proof. Admitted. 
+
+Lemma proof_of_fix_spaces_partial_solve_wit_15 : fix_spaces_partial_solve_wit_15.
+Proof. Admitted. 
+
+Lemma proof_of_fix_spaces_partial_solve_wit_16 : fix_spaces_partial_solve_wit_16.
+Proof. Admitted. 
+
+Lemma proof_of_fix_spaces_partial_solve_wit_17 : fix_spaces_partial_solve_wit_17.
+Proof. Admitted. 
+
+Lemma proof_of_fix_spaces_partial_solve_wit_18 : fix_spaces_partial_solve_wit_18.
+Proof. Admitted. 
+
