QCP_examples/humaneval/spec_logic_rewrite_c_files/C_140_proof_manual.v
@@ -1,0 +1,158 @@
+Require Import Coq.ZArith.ZArith.
+Require Import Coq.Bool.Bool.
+Require Import Coq.Strings.String.
+Require Import Coq.Strings.Ascii.
+Require Import Coq.Lists.List.
+Require Import Coq.Classes.RelationClasses.
+Require Import Coq.Classes.Morphisms.
+Require Import Coq.micromega.Psatz.
+Require Import Coq.Sorting.Permutation.
+From AUXLib Require Import int_auto Axioms Feq Idents ListLib VMap.
+Require Import SetsClass.SetsClass. Import SetsNotation.
+From SimpleC.SL Require Import Mem SeparationLogic.
+From SimpleC.EE Require Import C_140_goal.
+From SimpleC.EE Require Import C_140_proof_auto.
+Require Import Logic.LogicGenerator.demo932.Interface.
+Local Open Scope Z_scope.
+Local Open Scope sets.
+Local Open Scope string_scope.
+Local Open Scope list.
+Import naive_C_Rules.
+Require Import SimpleC.StdLib.string_lib.
+Require Import coins_140.
+Local Open Scope sac.
+
+Lemma proof_of_fix_spaces_entail_wit_1 : fix_spaces_entail_wit_1.
+Proof.
+  right; intros.
+  entailer!.
+  - subst retval. apply string_length_nonneg.
+  - apply fix_spaces_state_z_140_init.
+Qed.
+
+Lemma proof_of_fix_spaces_entail_wit_2_1 : fix_spaces_entail_wit_2_1.
+Proof.
+  right; intros.
+  assert (spacelen = 0) by lia; subst spacelen.
+  pose proof (fix_spaces_state_z_140_char input output_2 i 0
+    ltac:(unfold string_length in *; lia) PreH5 PreH14) as Hstep.
+  unfold flush_spaces_z_140 in Hstep. simpl in Hstep.
+  entailer!.
+  rewrite Zlength_app, Zlength_cons, Zlength_nil. lia.
+Qed.
+
+Lemma proof_of_fix_spaces_entail_wit_2_2 : fix_spaces_entail_wit_2_2.
+Proof.
+  right; intros. subst spacelen.
+  pose proof (fix_spaces_state_z_140_char input output_2 i 1
+    ltac:(unfold string_length in *; lia) PreH6 PreH15) as Hstep.
+  unfold flush_spaces_z_140 in Hstep. simpl in Hstep.
+  entailer!.
+  - rewrite !Zlength_app, !Zlength_cons, Zlength_nil. lia.
+  - rewrite <- app_assoc. exact Hstep.
+Qed.
+
+Lemma proof_of_fix_spaces_entail_wit_2_3 : fix_spaces_entail_wit_2_3.
+Proof.
+  right; intros. subst spacelen.
+  pose proof (fix_spaces_state_z_140_char input output_2 i 2
+    ltac:(unfold string_length in *; lia) PreH7 PreH16) as Hstep.
+  unfold flush_spaces_z_140 in Hstep. simpl in Hstep.
+  entailer!.
+  - rewrite !Zlength_app, !Zlength_cons, Zlength_nil. lia.
+  - repeat rewrite <- app_assoc. exact Hstep.
+Qed.
+
+Lemma proof_of_fix_spaces_entail_wit_2_4 : fix_spaces_entail_wit_2_4.
+Proof.
+  right; intros.
+  pose proof (fix_spaces_state_z_140_char input output_2 i spacelen
+    ltac:(unfold string_length in *; lia) PreH6 PreH15) as Hstep.
+  unfold flush_spaces_z_140 in Hstep.
+  destruct (Z.eq_dec spacelen 0); [lia |].
+  destruct (Z.eq_dec spacelen 1); [lia |].
+  destruct (Z.eq_dec spacelen 2); [lia |].
+  entailer!.
+  - rewrite !Zlength_app, !Zlength_cons, Zlength_nil. lia.
+  - rewrite <- app_assoc. exact Hstep.
+Qed.
+
+Lemma proof_of_fix_spaces_entail_wit_2_5 : fix_spaces_entail_wit_2_5.
+Proof.
+  right; intros.
+  pose proof (fix_spaces_state_z_140_space input output_2 i spacelen
+    ltac:(unfold string_length in *; lia) PreH2 PreH11) as Hstep.
+  entailer!.
+Qed.
+
+Lemma proof_of_fix_spaces_entail_wit_4_1 : fix_spaces_entail_wit_4_1.
+Proof.
+  right; intros.
+  assert (i = n) by lia; subst i.
+  assert (spacelen = 0) by lia; subst spacelen.
+  Exists output_2.
+  unfold flush_spaces_z_140. simpl.
+  entailer!.
+  - rewrite app_nil_r. exact PreH12.
+  - rewrite app_nil_r. reflexivity.
+Qed.
+
+Lemma proof_of_fix_spaces_entail_wit_4_2 : fix_spaces_entail_wit_4_2.
+Proof.
+  right; intros.
+  assert (i = n) by lia; subst i. subst spacelen.
+  Exists output_2.
+  unfold flush_spaces_z_140. simpl.
+  entailer!.
+  rewrite Zlength_app, Zlength_cons, Zlength_nil. lia.
+Qed.
+
+Lemma proof_of_fix_spaces_entail_wit_4_3 : fix_spaces_entail_wit_4_3.
+Proof.
+  right; intros.
+  assert (i = n) by lia; subst i. subst spacelen.
+  Exists output_2.
+  unfold flush_spaces_z_140. simpl.
+  entailer!.
+  rewrite !Zlength_app, !Zlength_cons, Zlength_nil. lia.
+  symmetry.
+  change (output_2 ++ (95 :: nil) ++ (95 :: nil) =
+    (output_2 ++ (95 :: nil)) ++ (95 :: nil)).
+  apply app_assoc.
+Qed.
+
+Lemma proof_of_fix_spaces_entail_wit_4_4 : fix_spaces_entail_wit_4_4.
+Proof.
+  right; intros.
+  assert (i = n) by lia; subst i.
+  Exists output_2.
+  unfold flush_spaces_z_140.
+  destruct (Z.eq_dec spacelen 0); [lia |].
+  destruct (Z.eq_dec spacelen 1); [lia |].
+  destruct (Z.eq_dec spacelen 2); [lia |].
+  entailer!.
+  rewrite Zlength_app, Zlength_cons, Zlength_nil. lia.
+Qed.
+
+Lemma proof_of_fix_spaces_return_wit_1 : fix_spaces_return_wit_1.
+Proof.
+  right; intros.
+  Exists output_2.
+  assert (Hspec : problem_140_spec_z input output_2).
+  { eapply problem_140_spec_z_from_state.
+    - exact PreH10.
+    - subst n. unfold string_length in PreH9. exact PreH9.
+    - exact PreH8. }
+  unfold string_length in PreH3.
+  subst n. subst k.
+  unfold store_string, string_length, c_string.
+  entailer!.
+Qed.
+
+Lemma proof_of_fix_spaces_partial_solve_wit_2_pure : fix_spaces_partial_solve_wit_2_pure.
+Proof.
+  right; intros.
+  subst retval.
+  pose proof (string_length_nonneg input).
+  entailer!; lia.
+Qed.
